refactoring

src/drf/DRF_PF.v
@@ -33,14 +33,251 @@ Require Import PredStep.
 
 Set Implicit Arguments.
 
-Inductive unchanged_on (P: Loc.t -> Time.t -> Prop) m0 m1 : Prop :=
-| unchanged_on_intro
-    (NCOV: forall l t (IN: P l t) (COV: covered l t m1), covered l t m0)
-    (FUTURE : Memory.le m0 m1)
-.
-Global Program Instance le_PreOrder P: PreOrder (unchanged_on P).
-Next Obligation. ii. econs; eauto. refl. Qed.
-Next Obligation. ii. inv H. inv H0. econs; eauto. etrans; eauto. Qed.
+
+Section FORGETMEMORY.
+
+  Inductive forget_memory P msrc mtgt : Prop :=
+  | forget_memory_intro
+      (COMPLETE: forall l t (NPROMS: ~ P l t),
+          Memory.get l t msrc = Memory.get l t mtgt)
+      (FORGET: forall l t (PROMS: P l t), Memory.get l t msrc = None)
+  .
+
+  Lemma forget_compose P0 P1 m0 m1 m2
+        (FORGET0: forget_memory P0 m0 m1)
+        (FORGET1: forget_memory P1 m1 m2)
+    :
+      forget_memory (P0 \2/ P1) m0 m2.
+  Proof.
+    inv FORGET0. inv FORGET1. econs; eauto.
+    - ii. apply not_or_and in NPROMS. des.
+      erewrite COMPLETE; eauto.
+    - i. destruct (classic (P0 l t)); auto.
+      des; clarify. erewrite COMPLETE; eauto.
+  Qed.
+
+  Lemma forget_compose_middle P0 P1 m0 m1 m2
+        (FORGET: forget_memory (P0 \2/ P1) m0 m2)
+        (FORGET1: forget_memory P1 m1 m2)
+    :
+      forget_memory P0 m0 m1.
+  Proof.
+    inv FORGET. inv FORGET1. econs; eauto.
+    ii. destruct (classic (P1 l t)).
+    - erewrite FORGET; eauto.
+    - erewrite COMPLETE; eauto.
+      + erewrite COMPLETE0; eauto.
+      + ii. des; clarify.
+  Qed.
+
+  Lemma forget_memory_le P msrc mtgt
+        (FORGET: forget_memory P msrc mtgt)
+    :
+      Memory.le msrc mtgt.
+  Proof.
+    inv FORGET. ii.
+    destruct (classic (P loc to)).
+    - exploit FORGET0; eauto.
+      i. clarify.
+    - exploit COMPLETE; eauto.
+      i. rewrite LHS in *. auto.
+  Qed.
+
+  Lemma list_filter_exists A (P: A -> Prop) (l: list A)
+    :
+      exists l',
+        (<<COMPLETE: forall a, ((<<IN: List.In a l>>) /\ (<<SAT: P a>>))
+                               <-> (<<IN: List.In a l'>>)>>).
+  Proof.
+    induction l.
+    - exists []. ii. split; i; des.
+      + inv IN.
+      + inv H.
+    - des. destruct (classic (P a)).
+      + exists (a :: l'). split; i; ss; des; clarify; eauto.
+        * right. eapply COMPLETE; eauto.
+        * eapply COMPLETE in H0. des. eauto.
+      + exists l'. split; i; ss; des; clarify; eauto.
+        * eapply COMPLETE; eauto.
+        * eapply COMPLETE in H0. des; eauto.
+  Qed.
+
+  Lemma forget_exists_list l mem_tgt:
+    exists mem_src, <<FORGET: forget_memory (fun loc to => List.In (loc, to) l)
+                                            mem_src mem_tgt>>.
+  Proof.
+    induction l; ss.
+    - exists mem_tgt. econs; ss.
+    - i. destruct a as [loc to]. des.
+      destruct (Memory.get loc to mem_src) as [[from msg]|] eqn:GET.
+      + exploit Memory.remove_exists; eauto. i. des. exists mem2.
+        inv FORGET. econs; i.
+        * erewrite Memory.remove_o; eauto. des_ifs; eauto.
+          ss; des; clarify. exfalso. eauto.
+        * erewrite Memory.remove_o; eauto. des_ifs; clarify.
+          eapply FORGET0; eauto. ss. des; clarify; eauto.
+      + exists mem_src. inv FORGET.
+        econs; eauto. i. des; clarify; eauto.
+  Qed.
+
+  Lemma forget_exists P mem_tgt:
+    exists mem_src, <<FORGET: forget_memory P mem_src mem_tgt>>.
+  Proof.
+    hexploit (Memory.finite_sound_exists mem_tgt); eauto. i. des.
+    hexploit (list_filter_exists (fun locto => P (fst locto) (snd locto)) dom). i. des.
+    hexploit (forget_exists_list l' mem_tgt). i. des.
+    exists mem_src. inv FORGET. econs; eauto.
+    - i. eapply COMPLETE0. ii. eapply COMPLETE in H1. des; eauto.
+    - i. destruct (classic (List.In (l, t) dom)).
+      + eapply FORGET0; eauto. eapply COMPLETE; eauto.
+      + rewrite COMPLETE0; eauto.
+        * destruct (Memory.get l t mem_tgt) as [[from msg]|] eqn:GET; auto.
+          exfalso. exploit H; eauto.
+        * ii. eapply COMPLETE in H2. des; clarify.
+  Qed.
+
+  Lemma forget_unique P mem_tgt mem_src0 mem_src1
+        (FORGET0: forget_memory P mem_src0 mem_tgt)
+        (FORGET1: forget_memory P mem_src1 mem_tgt)
+    :
+      mem_src0 = mem_src1.
+  Proof.
+    inv FORGET0. inv FORGET1.
+    eapply Memory.ext. i. destruct (classic (P loc ts)).
+    - erewrite FORGET; auto. erewrite FORGET0; auto.
+    - erewrite COMPLETE; auto. erewrite COMPLETE0; auto.
+  Qed.
+
+End FORGETMEMORY.
+
+
+
+Section MEMORYLEMMAS.
+
+  Lemma inhabited_future mem1 mem2
+        (FUTURE: Memory.future mem1 mem2)
+        (INHABITED: Memory.inhabited mem1)
+  :
+    Memory.inhabited mem2.
+  Proof.
+    induction FUTURE; auto. apply IHFUTURE.
+    inv H. hexploit Memory.op_inhabited; eauto.
+  Qed.
+
+  Lemma memory_le_get_none msrc mtgt loc to
+        (MLE: Memory.le msrc mtgt)
+        (NONE: Memory.get loc to mtgt = None)
+    :
+      Memory.get loc to msrc = None.
+  Proof.
+    destruct (Memory.get loc to msrc) eqn:GET; auto.
+    destruct p. eapply MLE in GET. clarify.
+  Qed.
+
+  Lemma memory_le_covered msrc mtgt loc to
+        (MLE: Memory.le msrc mtgt)
+        (COVERED: covered loc to msrc)
+    :
+      covered loc to mtgt.
+  Proof.
+    inv COVERED. econs; eauto.
+  Qed.
+
+  Lemma memory_add_cover_disjoint mem0 loc from to msg mem1
+        (ADD: Memory.add mem0 loc from to msg mem1)
+        t
+        (IN: Interval.mem (from, to) t)
+    :
+      ~ covered loc t mem0.
+  Proof.
+    ii. inv H. dup ADD. eapply Memory.add_get0 in ADD. des.
+    exploit Memory.get_disjoint.
+    + eapply Memory.add_get1; eauto.
+    + eauto.
+    + i. des; clarify. eauto.
+  Qed.
+
+  Lemma write_succeed mem1 loc from1 to1 val released
+        (NCOVER: forall t (COVER: covered loc t mem1),
+            ~ Interval.mem (from1, to1) t)
+        (TO: Time.le (View.rlx (View.unwrap released) loc) to1)
+        (FROMTO: Time.lt from1 to1)
+        (MSGWF: Message.wf (Message.full val released))
+    :
+      exists mem2,
+        (<<WRITE: Memory.write Memory.bot mem1 loc from1 to1 val released Memory.bot mem2 Memory.op_kind_add>>).
+  Proof.
+    exploit Memory.add_exists; eauto.
+    { instantiate (1:=mem1). instantiate (1:=loc).
+      ii. eapply NCOVER; eauto. econs; eauto. }
+    i. des. exists mem2.
+    exploit Memory.add_exists; eauto.
+    { instantiate (1:=Memory.bot). instantiate (1:=loc).
+      ii. rewrite Memory.bot_get in *. clarify. } i. des.
+    econs.
+    - econs; eauto; ss.
+    - exploit Memory.remove_exists; eauto.
+      { eapply Memory.add_get0 in x1. des. eauto. } i. des.
+      exploit MemoryFacts.MemoryFacts.add_remove_eq; eauto.
+      i. clarify.
+  Qed.
+
+  Lemma write_disjoint promises1 mem1 loc from1 to1 val released promises3 mem2 kind
+        (MLE: Memory.le promises1 mem1)
+        (WRITE: Memory.write
+                  promises1 mem1 loc from1 to1 val released promises3 mem2 kind)
+        to
+        (INT: Interval.mem (from1, to1) to)
+    :
+      (<<PROMISED: covered loc to promises1>>) \/
+      (<<NEWMSG: ~ covered loc to mem1>>).
+  Proof.
+    inv WRITE. inv PROMISE.
+    - right. ii. inv H. inv MEM. inv ADD.
+      exploit DISJOINT; eauto.
+    - left. dup PROMISES. eapply Memory.split_get0 in PROMISES. des.
+      econs; eauto.
+      inv INT. inv PROMISES0. inv SPLIT. econs; ss.
+      etrans; eauto. left. auto.
+    - left. dup PROMISES. eapply Memory.lower_get0 in PROMISES. des.
+      econs; eauto.
+  Qed.
+
+  Lemma write_msg_wf v prom v' prom'
+        loc from to val releasedm released ord sc sc' mem_tgt mem_tgt' kind
+        (WRITE: Local.write_step
+                  (Local.mk v prom) sc mem_tgt
+                  loc from to val releasedm released ord
+                  (Local.mk v' prom') sc' mem_tgt' kind)
+    :
+      (<<TLE: Time.le
+                (View.rlx (View.unwrap (TView.write_released v sc loc to releasedm ord)) loc) to>>) /\
+      (<<FROMTO: Time.lt from to>>) /\
+      (<<MSGWF: Message.wf (Message.full val (TView.write_released v sc loc to releasedm ord))>>)
+  .
+  Proof.
+    inv WRITE. inv WRITE0. inv PROMISE.
+    - inv TS. inv MEM. inv ADD. esplits; eauto.
+    - inv TS. inv MEM. inv SPLIT. esplits; eauto.
+    - inv TS. inv MEM. inv LOWER. esplits; eauto.
+  Qed.
+
+  Lemma memory_write_bot_add
+        mem1 loc from1 to1 val released promises3 mem2 kind
+        (WRITE: Memory.write
+                  Memory.bot mem1 loc from1 to1 val released promises3 mem2 kind)
+    :
+      kind = Memory.op_kind_add.
+  Proof.
+    inv WRITE. inv PROMISE; auto.
+    - exfalso. eapply Memory.split_get0 in PROMISES. des.
+      rewrite Memory.bot_get in *. clarify.
+    - exfalso. eapply Memory.lower_get0 in PROMISES. des.
+      rewrite Memory.bot_get in *. clarify.
+  Qed.
+
+End MEMORYLEMMAS.
+
 
 Inductive promised (mem: Memory.t) (loc: Loc.t) (to: Time.t) : Prop :=
 | promised_intro
@@ -49,60 +286,6 @@ Inductive promised (mem: Memory.t) (loc: Loc.t) (to: Time.t) : Prop :=
   :
     promised mem loc to
 .
-
-Inductive forget_memory P msrc mtgt : Prop :=
-| forget_memory_intro
-    (* (FUTURE: Memory.le msrc mtgt) *)
-    (COMPLETE: forall l t (NPROMS: ~ P l t),
-        Memory.get l t msrc = Memory.get l t mtgt)
-    (FORGET: forall l t (PROMS: P l t), Memory.get l t msrc = None)
-.
-
-Lemma forget_memory_le P msrc mtgt
-      (FORGET: forget_memory P msrc mtgt)
-  :
-    Memory.le msrc mtgt.
-Proof.
-  inv FORGET. ii.
-  destruct (classic (P loc to)).
-  - exploit FORGET0; eauto.
-    i. clarify.
-  - exploit COMPLETE; eauto.
-    i. rewrite LHS in *. auto.
-Qed.
-
-Lemma memory_le_get_none msrc mtgt loc to
-      (MLE: Memory.le msrc mtgt)
-      (NONE: Memory.get loc to mtgt = None)
-  :
-    Memory.get loc to msrc = None.
-Proof.
-  destruct (Memory.get loc to msrc) eqn:GET; auto.
-  destruct p. eapply MLE in GET. clarify.
-Qed.
-
-Lemma memory_le_covered msrc mtgt loc to
-      (MLE: Memory.le msrc mtgt)
-      (COVERED: covered loc to msrc)
-  :
-    covered loc to mtgt.
-Proof.
-  inv COVERED. econs; eauto.
-Qed.
-
-Lemma memory_add_cover_disjoint mem0 loc from to msg mem1
-      (ADD: Memory.add mem0 loc from to msg mem1)
-      t
-      (IN: Interval.mem (from, to) t)
-  :
-    ~ covered loc t mem0.
-Proof.
-  ii. inv H. dup ADD. eapply Memory.add_get0 in ADD. des.
-  exploit Memory.get_disjoint.
-  + eapply Memory.add_get1; eauto.
-  + eauto.
-  + i. des; clarify. eauto.
-Qed.
 
 Inductive opt_pred_step P (lang : Language.t)
   : ThreadEvent.t -> Thread.t lang -> Thread.t lang -> Prop :=
@@ -114,2066 +297,1952 @@ Inductive opt_pred_step P (lang : Language.t)
     opt_pred_step P e t0 t1.
 Hint Constructors opt_pred_step.
 
-Definition promise_view_consistent (prom: Loc.t -> Time.t -> Prop) (view: TimeMap.t) : Prop :=
-  forall
-    loc to
-    (GET: prom loc to),
-    Time.lt (view loc) to.
 
-Definition local_consistent (lc: Local.t): Prop :=
-  promise_view_consistent (promised lc.(Local.promises)) lc.(Local.tview).(TView.cur).(View.rlx).
+Section VIEWCONSISTENT.
 
-Lemma promise_view_consistent_le v0 v1 prm
-      (VLE: TimeMap.le v0 v1)
-      (CONS: promise_view_consistent prm v1)
-  :
-    promise_view_consistent prm v0.
-Proof.
-  ii. exploit CONS; eauto. i.
-  eapply DenseOrder.DenseOrderFacts.le_lt_lt; eauto.
-Qed.
+  Definition promise_view_consistent (prom: Loc.t -> Time.t -> Prop) (view: TimeMap.t) : Prop :=
+    forall
+      loc to
+      (GET: prom loc to),
+      Time.lt (view loc) to.
 
-Lemma local_consistent_le tv0 tv1 prm
-      (VLE: TView.le tv0 tv1)
-      (CONS: local_consistent (Local.mk tv1 prm))
-  :
-    local_consistent (Local.mk tv0 prm).
-Proof.
-  inv VLE. inv CUR. unfold local_consistent in *. ss.
-  eapply promise_view_consistent_le; eauto.
-Qed.
+  Definition local_consistent (lc: Local.t): Prop :=
+    promise_view_consistent (promised lc.(Local.promises)) lc.(Local.tview).(TView.cur).(View.rlx).
 
-Lemma local_consistent_write lang (st0 st1: Language.state lang) lc0 lc1
-      sc0 sc1 m0 m1 loc tsr tsw valw releasedr releasedw ordw kind
-      (STEP: Local.write_step
-               lc0 sc0 m0 loc
-               tsr tsw valw releasedr releasedw ordw lc1 sc1 m1 kind)
-      (WF1: Local.wf lc0 m0)
-      (SC1: Memory.closed_timemap sc0 m0)
-      (RVwF: View.opt_wf releasedr)
-      (RVCLOSED: Memory.closed_opt_view releasedr m0)
-      (CLOSED1: Memory.closed m0)
-      (CONSISTENT: local_consistent lc1)
-  :
-    local_consistent lc0.
-Proof.
-  exploit Local.write_step_future; eauto. i. des.
-  inv STEP. inv WRITE. inv PROMISE; ss.
-  - exploit MemoryFacts.MemoryFacts.add_remove_eq.
-    { eapply PROMISES. }
-    { eapply REMOVE. }
-    i. clarify. eapply local_consistent_le; eauto.
-  - ii. destruct (loc_ts_eq_dec (loc0, to) (loc, tsw)).
-    + des. ss. clarify. inv WRITABLE. eauto.
-    + destruct (TimeSet.Facts.eq_dec to tsw).
-      * inv GET. exploit CONSISTENT; ss; eauto.
-        { econs. instantiate (1:=msg). instantiate (1:=tsw). instantiate (1:=loc0).
+  Lemma promise_view_consistent_le v0 v1 prm
+        (VLE: TimeMap.le v0 v1)
+        (CONS: promise_view_consistent prm v1)
+    :
+      promise_view_consistent prm v0.
+  Proof.
+    ii. exploit CONS; eauto. i.
+    eapply DenseOrder.DenseOrderFacts.le_lt_lt; eauto.
+  Qed.
+
+  Lemma local_consistent_le tv0 tv1 prm
+        (VLE: TView.le tv0 tv1)
+        (CONS: local_consistent (Local.mk tv1 prm))
+    :
+      local_consistent (Local.mk tv0 prm).
+  Proof.
+    inv VLE. inv CUR. unfold local_consistent in *. ss.
+    eapply promise_view_consistent_le; eauto.
+  Qed.
+
+  Lemma local_consistent_write lang (st0 st1: Language.state lang) lc0 lc1
+        sc0 sc1 m0 m1 loc tsr tsw valw releasedr releasedw ordw kind
+        (STEP: Local.write_step
+                 lc0 sc0 m0 loc
+                 tsr tsw valw releasedr releasedw ordw lc1 sc1 m1 kind)
+        (WF1: Local.wf lc0 m0)
+        (SC1: Memory.closed_timemap sc0 m0)
+        (RVwF: View.opt_wf releasedr)
+        (RVCLOSED: Memory.closed_opt_view releasedr m0)
+        (CLOSED1: Memory.closed m0)
+        (CONSISTENT: local_consistent lc1)
+    :
+      local_consistent lc0.
+  Proof.
+    exploit Local.write_step_future; eauto. i. des.
+    inv STEP. inv WRITE. inv PROMISE; ss.
+    - exploit MemoryFacts.MemoryFacts.add_remove_eq.
+      { eapply PROMISES. }
+      { eapply REMOVE. }
+      i. clarify. eapply local_consistent_le; eauto.
+    - ii. destruct (loc_ts_eq_dec (loc0, to) (loc, tsw)).
+      + des. ss. clarify. inv WRITABLE. eauto.
+      + destruct (TimeSet.Facts.eq_dec to tsw).
+        * inv GET. exploit CONSISTENT; ss; eauto.
+          { econs. instantiate (1:=msg). instantiate (1:=tsw). instantiate (1:=loc0).
+            erewrite Memory.remove_o; eauto.
+            erewrite Memory.split_o; eauto. des_ifs; ss; des; clarify. }
+          { i. eapply TimeFacts.le_lt_lt; eauto. eapply TimeMap.join_l. }
+        * destruct (loc_ts_eq_dec (loc0, to) (loc, ts3)).
+          { inv GET. exploit CONSISTENT; ss; eauto.
+            - econs. instantiate (2:=to). instantiate (2:=loc0).
+              erewrite Memory.remove_o; eauto.
+              erewrite Memory.split_o; eauto. des_ifs; ss; des; clarify.
+            - i. eapply TimeFacts.le_lt_lt; eauto. eapply TimeMap.join_l. }
+          { inv GET. exploit CONSISTENT; ss; eauto.
+            - econs. instantiate (2:=to). instantiate (2:=loc0).
+              erewrite Memory.remove_o; eauto.
+              erewrite Memory.split_o; eauto. des_if.
+              + ss. des; clarify.
+              + simpl in *. des_if; cycle 1.
+                * eauto.
+                * des; ss; clarify.
+            - i. eapply TimeFacts.le_lt_lt; eauto. eapply TimeMap.join_l. }
+    - ii. destruct (loc_ts_eq_dec (loc0, to) (loc, tsw)).
+      + des. ss. clarify. inv WRITABLE. eauto.
+      + inv GET. exploit CONSISTENT; ss; eauto.
+        * econs. instantiate (1:=msg). instantiate (1:=to). instantiate (1:=loc0).
           erewrite Memory.remove_o; eauto.
-          erewrite Memory.split_o; eauto. des_ifs; ss; des; clarify. }
-        { i. eapply TimeFacts.le_lt_lt; eauto. eapply TimeMap.join_l. }
-      * destruct (loc_ts_eq_dec (loc0, to) (loc, ts3)).
-        { inv GET. exploit CONSISTENT; ss; eauto.
-          - econs. instantiate (2:=to). instantiate (2:=loc0).
-            erewrite Memory.remove_o; eauto.
-            erewrite Memory.split_o; eauto. des_ifs; ss; des; clarify.
-          - i. eapply TimeFacts.le_lt_lt; eauto. eapply TimeMap.join_l. }
-        { inv GET. exploit CONSISTENT; ss; eauto.
-          - econs. instantiate (2:=to). instantiate (2:=loc0).
-            erewrite Memory.remove_o; eauto.
-            erewrite Memory.split_o; eauto. des_if.
-            + ss. des; clarify.
-            + simpl in *. des_if; cycle 1.
-              * eauto.
-              * des; ss; clarify.
-          - i. eapply TimeFacts.le_lt_lt; eauto. eapply TimeMap.join_l. }
-  - ii. destruct (loc_ts_eq_dec (loc0, to) (loc, tsw)).
-    + des. ss. clarify. inv WRITABLE. eauto.
-    + inv GET. exploit CONSISTENT; ss; eauto.
-      * econs. instantiate (1:=msg). instantiate (1:=to). instantiate (1:=loc0).
-        erewrite Memory.remove_o; eauto.
-        erewrite Memory.lower_o; eauto. des_ifs; ss; des; clarify.
-      * i. eapply TimeFacts.le_lt_lt; eauto. eapply TimeMap.join_l.
-Qed.
+          erewrite Memory.lower_o; eauto. des_ifs; ss; des; clarify.
+        * i. eapply TimeFacts.le_lt_lt; eauto. eapply TimeMap.join_l.
+  Qed.
 
-Lemma local_consistent_step lang (st0 st1: Language.state lang) lc0 lc1
-      sc0 sc1 m0 m1 pf e
-      (WF1: Local.wf lc0 m0)
-      (SC1: Memory.closed_timemap sc0 m0)
-      (CLOSED1: Memory.closed m0)
-      (CONSISTENT: local_consistent lc1)
-      (STEP: Thread.step pf e (Thread.mk _ st0 lc0 sc0 m0) (Thread.mk _ st1 lc1 sc1 m1))
-  :
-    local_consistent lc0.
-Proof.
-  exploit Thread.step_future; eauto; ss. i. des.
-  inv STEP; ss.
-  - inv STEP0. inv LOCAL. ii. inv GET. destruct msg0.
-    exploit Memory.promise_get1_promise; eauto. i. des.
-    exploit CONSISTENT; ss; eauto. econs; eauto.
-  - inv STEP0. destruct lc0, lc1. inv LOCAL; ss; eauto.
-    + inv LOCAL0; ss. clarify.
-      eapply local_consistent_le; eauto.
-    + eapply local_consistent_write; eauto.
-    + exploit Local.read_step_future; eauto. i. des.
-      hexploit local_consistent_write; eauto.
-      inv LOCAL1. ss. i.
-      eapply local_consistent_le; eauto.
-    + inv LOCAL0; ss. clarify.
-      eapply local_consistent_le; eauto.
-    + inv LOCAL0; ss. clarify.
-      eapply local_consistent_le; eauto.
-Qed.
+  Lemma local_consistent_step lang (st0 st1: Language.state lang) lc0 lc1
+        sc0 sc1 m0 m1 pf e
+        (WF1: Local.wf lc0 m0)
+        (SC1: Memory.closed_timemap sc0 m0)
+        (CLOSED1: Memory.closed m0)
+        (CONSISTENT: local_consistent lc1)
+        (STEP: Thread.step pf e (Thread.mk _ st0 lc0 sc0 m0) (Thread.mk _ st1 lc1 sc1 m1))
+    :
+      local_consistent lc0.
+  Proof.
+    exploit Thread.step_future; eauto; ss. i. des.
+    inv STEP; ss.
+    - inv STEP0. inv LOCAL. ii. inv GET. destruct msg0.
+      exploit Memory.promise_get1_promise; eauto. i. des.
+      exploit CONSISTENT; ss; eauto. econs; eauto.
+    - inv STEP0. destruct lc0, lc1. inv LOCAL; ss; eauto.
+      + inv LOCAL0; ss. clarify.
+        eapply local_consistent_le; eauto.
+      + eapply local_consistent_write; eauto.
+      + exploit Local.read_step_future; eauto. i. des.
+        hexploit local_consistent_write; eauto.
+        inv LOCAL1. ss. i.
+        eapply local_consistent_le; eauto.
+      + inv LOCAL0; ss. clarify.
+        eapply local_consistent_le; eauto.
+      + inv LOCAL0; ss. clarify.
+        eapply local_consistent_le; eauto.
+  Qed.
 
-Lemma inhabited_future mem1 mem2
-      (FUTURE: Memory.future mem1 mem2)
-      (INHABITED: Memory.inhabited mem1)
-  :
-    Memory.inhabited mem2.
-Proof.
-  induction FUTURE; auto. apply IHFUTURE.
-  inv H. hexploit Memory.op_inhabited; eauto.
-Qed.
+  Lemma thread_consistent_view_consistent lang st lc sc mem
+        (CLOSED: Memory.closed mem)
+        (INHABITED: Memory.inhabited mem)
+        (LCWF: Local.wf lc mem)
+        (SC: Memory.closed_timemap sc mem)
+        (CONSISTENT: Thread.consistent (Thread.mk lang st lc sc mem))
+    :
+      local_consistent lc.
+  Proof.
+    hexploit Memory.cap_exists; eauto. instantiate (1:=lc.(Local.promises)). i. des.
+    hexploit inhabited_future; eauto. i.
+    exploit Memory.max_full_timemap_exists; eauto. i. des.
+    exploit CONSISTENT; eauto. i. des. ss.
+    assert (CONSISTENT1: local_consistent (Thread.local e2)).
+    { ii. inv GET. rewrite PROMISES in *. rewrite Memory.bot_get in *. clarify. }
+    eapply Local.cap_wf in LCWF; eauto.
+    eapply Memory.cap_closed_timemap in SC; eauto.
+    eapply Memory.cap_closed in CLOSED; eauto.
+    eapply Memory.max_full_timemap_closed in x0; eauto.
+    clear - LCWF x0 CLOSED LCWF CONSISTENT1 STEPS. rename x0 into SC.
+    remember (Thread.mk _ st lc tm mem2) as e1.
+    replace mem2 with e1.(Thread.memory) in *; [| rewrite Heqe1; ss].
+    replace tm with e1.(Thread.sc) in *; [| rewrite Heqe1; ss].
+    replace lc with e1.(Thread.local) in *; [| rewrite Heqe1; ss].
+    clear Heqe1 st lc tm mem2.
+    revert LCWF SC CLOSED.
 
-Lemma thread_consistent_view_consistent lang st lc sc mem
-      (CLOSED: Memory.closed mem)
-      (INHABITED: Memory.inhabited mem)
-      (LCWF: Local.wf lc mem)
-      (SC: Memory.closed_timemap sc mem)
-      (CONSISTENT: Thread.consistent (Thread.mk lang st lc sc mem))
-  :
-    local_consistent lc.
-Proof.
-  hexploit Memory.cap_exists; eauto. instantiate (1:=lc.(Local.promises)). i. des.
-  hexploit inhabited_future; eauto. i.
-  exploit Memory.max_full_timemap_exists; eauto. i. des.
-  exploit CONSISTENT; eauto. i. des. ss.
-  assert (CONSISTENT1: local_consistent (Thread.local e2)).
-  { ii. inv GET. rewrite PROMISES in *. rewrite Memory.bot_get in *. clarify. }
-  eapply Local.cap_wf in LCWF; eauto.
-  eapply Memory.cap_closed_timemap in SC; eauto.
-  eapply Memory.cap_closed in CLOSED; eauto.
-  eapply Memory.max_full_timemap_closed in x0; eauto.
-  clear - LCWF x0 CLOSED LCWF CONSISTENT1 STEPS. rename x0 into SC.
-  remember (Thread.mk _ st lc tm mem2) as e1.
-  replace mem2 with e1.(Thread.memory) in *; [| rewrite Heqe1; ss].
-  replace tm with e1.(Thread.sc) in *; [| rewrite Heqe1; ss].
-  replace lc with e1.(Thread.local) in *; [| rewrite Heqe1; ss].
-  clear Heqe1 st lc tm mem2.
-  revert LCWF SC CLOSED.
+    eapply Operators_Properties.rt1n_ind_right with
+        (P := fun e1 =>
+                Local.wf (Thread.local e1) (Thread.memory e1) ->
+                Memory.closed_timemap (Thread.sc e1) (Thread.memory e1) ->
+                Memory.closed (Thread.memory e1) -> local_consistent (Thread.local e1)); eauto.
+    i. inv H. inv TSTEP.
+    hexploit Thread.step_future; eauto. i. des.
+    hexploit H1; eauto. i.
+    destruct x, y. ss. eapply local_consistent_step; eauto.
+  Qed.
 
-  eapply Operators_Properties.rt1n_ind_right with
-      (P := fun e1 =>
-              Local.wf (Thread.local e1) (Thread.memory e1) ->
-              Memory.closed_timemap (Thread.sc e1) (Thread.memory e1) ->
-              Memory.closed (Thread.memory e1) -> local_consistent (Thread.local e1)); eauto.
-  i. inv H. inv TSTEP.
-  hexploit Thread.step_future; eauto. i. des.
-  hexploit H1; eauto. i.
-  destruct x, y. ss. eapply local_consistent_step; eauto.
-Qed.
+End VIEWCONSISTENT.
 
-Lemma self_promise_remove_promise
-      prom prom' mem_src mem_tgt mem_tgt' loc from to msg kind
-      (MEM: forget_memory (promised prom) mem_src mem_tgt)
-      (PROMISE: Memory.promise prom mem_tgt loc from to msg prom' mem_tgt' kind)
+
+Section NOREADSELFPROMS.
+
+  Lemma self_promise_remove_promise
+        prom prom' mem_src mem_tgt mem_tgt' loc from to msg kind
+        (MEM: forget_memory (promised prom) mem_src mem_tgt)
+        (PROMISE: Memory.promise prom mem_tgt loc from to msg prom' mem_tgt' kind)
   :
     forget_memory (promised prom') mem_src mem_tgt'.
-Proof.
-  dup MEM. eapply forget_memory_le in MEM0. inv MEM. inv PROMISE.
-  - econs; eauto.
-    * i. rewrite COMPLETE.
-      { symmetry. erewrite Memory.add_o; eauto. des_ifs.
-        - ss. des. clarify. exfalso. apply NPROMS.
-          apply Memory.add_get0 in PROMISES. des.
-          econs; eauto. }
-      { ii. inv H. eapply NPROMS.
-        exploit Memory.add_o; try apply PROMISES; eauto. i.
-        erewrite GET in *. des_ifs.
-        - econs; eauto.
-        - econs; eauto. }
-    * i. inv PROMS. destruct msg0.
-      erewrite Memory.add_o in GET; eauto. des_ifs.
-      { ss. des. clarify.
-        eapply memory_le_get_none; eauto.
-        apply Memory.add_get0 in MEM. des. eauto. }
-      { eapply FORGET. econs; eauto. }
-  - econs; eauto.
-    * i. rewrite COMPLETE.
-      { symmetry. erewrite Memory.split_o; eauto. des_ifs.
-        - ss. des. clarify. exfalso. apply NPROMS.
-          apply Memory.split_get0 in PROMISES. des.
-          econs; eauto.
-        - ss. destruct a. clarify. exfalso. apply NPROMS.
-          apply Memory.split_get0 in PROMISES.
-          econs; des; eauto. }
-      { ii. inv H. eapply NPROMS.
-        exploit Memory.split_o; try apply PROMISES; eauto. i.
-        erewrite GET in *. des_ifs.
-        - econs; eauto.
-        - econs; eauto.
-        - econs; eauto. }
-    * i. inv PROMS. destruct msg0.
-      erewrite Memory.split_o in GET; eauto. des_ifs.
-      { ss. des. clarify.
-        eapply memory_le_get_none; eauto.
-        apply Memory.split_get0 in MEM. des. eauto. }
-      { ss. destruct a. clarify.
-        eapply FORGET. apply Memory.split_get0 in PROMISES.
-        econs. des; eauto. }
-      { eapply FORGET. econs; eauto. }
-  - econs; eauto.
-    * i. rewrite COMPLETE.
-      { symmetry. erewrite Memory.lower_o; eauto. des_ifs.
-        - ss. des. clarify. exfalso. apply NPROMS.
-          apply Memory.lower_get0 in PROMISES. des.
-          econs; eauto. }
-      { ii. inv H. eapply NPROMS.
-        exploit Memory.lower_o; try apply PROMISES; eauto. i.
-        erewrite GET in *. des_ifs.
-        - econs; eauto.
-        - econs; eauto. }
-    * i. inv PROMS. destruct msg1.
-      erewrite Memory.lower_o in GET; eauto. des_ifs.
-      { ss. des. clarify. eapply FORGET.
-        apply Memory.lower_get0 in PROMISES. des. econs. eauto. }
-      { eapply FORGET. apply Memory.lower_get0 in PROMISES.
-        econs. des; eauto. }
-Qed.
-
-Lemma consistent_read_no_self_promise_read
-      v v' prom prom'
-      mem_tgt loc ts val released ord
-      (STEP: Local.read_step (Local.mk v prom) mem_tgt loc
-             ts val released ord (Local.mk v' prom'))
-      (CONSISTENT: local_consistent (Local.mk v' prom'))
-  :
-    ~ prom.(promised) loc ts.
-Proof.
-  ii. inv H. inv STEP. ss. clarify.
-  exploit CONSISTENT; ss; eauto.
-  { econs; eauto. }
-  unfold TimeMap.join. i.
-  apply TimeFacts.join_lt_des in x. des.
-  apply TimeFacts.join_lt_des in AC. des.
-  unfold View.singleton_ur_if, View.singleton_ur in *. clear - BC0. des_ifs; ss.
-  * unfold TimeMap.singleton in *.
-    setoid_rewrite LocFun.add_spec_eq in BC0. timetac.
-  * unfold TimeMap.singleton in *.
-    setoid_rewrite LocFun.add_spec_eq in BC0. timetac.
-Qed.
-
-Lemma consistent_read_no_self_promise
-      lang th_tgt th_tgt' st st' v v' prom prom' sc sc'
-      mem_tgt mem_tgt' pf e_tgt
-      (LOCALWF: Local.wf (Local.mk v prom) mem_tgt)
-      (CLOSED: Memory.closed mem_tgt)
-      (SC: Memory.closed_timemap sc mem_tgt)
-      (TH_TGT0: th_tgt = Thread.mk lang st (Local.mk v prom) sc mem_tgt)
-      (TH_TGT1: th_tgt' = Thread.mk lang st' (Local.mk v' prom') sc' mem_tgt')
-      (CONSISTENT: local_consistent (Local.mk v' prom'))
-      (STEP: Thread.step pf e_tgt th_tgt th_tgt')
-  :
-    no_read_msgs prom.(promised) e_tgt.
-Proof.
-  inv STEP; ss.
-  - inv STEP0. ss.
-  - inv STEP0. inv LOCAL; ss.
-    + ii. exploit consistent_read_no_self_promise_read; eauto.
-    + ii. destruct lc2. hexploit consistent_read_no_self_promise_read; eauto.
-      exploit Local.read_step_future; eauto. i. des.
-      eapply local_consistent_write; eauto.
-Qed.
-
-Definition no_sc (e : ThreadEvent.t) : Prop :=
-  match e with
-  | ThreadEvent.fence _ ordw => ~ Ordering.le Ordering.seqcst ordw
-  | ThreadEvent.syscall _ => False
-  | _ => True
-  end
-.
-
-Definition no_acq_read_msgs (MSGS : Loc.t -> Time.t -> Prop)
-           (e : ThreadEvent.t) : Prop :=
-  match e with
-  | ThreadEvent.read loc to _ _ ord =>
-    forall (SAT: MSGS loc to), ~ Ordering.le Ordering.acqrel ord
-  | ThreadEvent.update loc from _ _ _ _ _ ordr _ =>
-    forall (SAT: MSGS loc from), ~ Ordering.le Ordering.acqrel ordr
-  | _ => True
-  end
-.
-
-Lemma consistent_certification_no_sc
-      P lang th_tgt th_tgt' st st' v v' prom prom' sc sc'
-      mem_tgt mem_tgt' e_tgt
-      (SCMAX: ~ promise_view_consistent prom sc)
-      (TH_TGT0: th_tgt = Thread.mk lang st (Local.mk v Memory.bot) sc mem_tgt)
-      (TH_TGT1: th_tgt' = Thread.mk lang st' (Local.mk v' prom') sc' mem_tgt')
-      (CONSISTENT: promise_view_consistent prom v'.(TView.cur).(View.rlx))
-      (STEP: (@pred_step (P /1\ no_promise) lang) e_tgt th_tgt th_tgt')
-  :
-    no_sc e_tgt.
-Proof.
-  inv STEP. inv STEP0; ss. inv STEP; ss.
-  - inv STEP0. ss.
-  - inv STEP0. inv LOCAL; ss.
-    + ii. clarify. inv LOCAL0. ss. clarify. ss. eapply SCMAX.
-      eapply promise_view_consistent_le; eauto. des_ifs; ss.
-      eapply TViewFacts.write_fence_sc_incr.
-    + ii. clarify. inv LOCAL0. ss. clarify. ss. eapply SCMAX.
-      eapply promise_view_consistent_le; eauto. des_ifs; ss.
-      eapply TViewFacts.write_fence_sc_incr.
-Qed.
-
-Inductive capped_with_max_view mem (CAP: Loc.t -> Time.t -> Prop)
-          (prom: Loc.t -> Time.t -> Prop): Prop :=
-| capped_with_max_view_intro
-    (GET: forall loc to from val view
-                 (SAT: CAP loc to)
-                 (GET: Memory.get loc to mem = Some (from, Message.full val view)),
-        match view with
-        | None => False
-        | Some view' => ~ promise_view_consistent prom view'.(View.rlx)
-        end)
-.
-
-Lemma write_succeed mem1 loc from1 to1 val released
-      (NCOVER: forall t (COVER: covered loc t mem1),
-          ~ Interval.mem (from1, to1) t)
-      (TO: Time.le (View.rlx (View.unwrap released) loc) to1)
-      (FROMTO: Time.lt from1 to1)
-      (MSGWF: Message.wf (Message.full val released))
-  :
-    exists mem2,
-      (<<WRITE: Memory.write Memory.bot mem1 loc from1 to1 val released Memory.bot mem2 Memory.op_kind_add>>).
-Proof.
-  exploit Memory.add_exists; eauto.
-  { instantiate (1:=mem1). instantiate (1:=loc).
-    ii. eapply NCOVER; eauto. econs; eauto. }
-  i. des. exists mem2.
-  exploit Memory.add_exists; eauto.
-  { instantiate (1:=Memory.bot). instantiate (1:=loc).
-    ii. rewrite Memory.bot_get in *. clarify. } i. des.
-  econs.
-  - econs; eauto; ss.
-  - exploit Memory.remove_exists; eauto.
-    { eapply Memory.add_get0 in x1. des. eauto. } i. des.
-    exploit MemoryFacts.MemoryFacts.add_remove_eq; eauto.
-    i. clarify.
-Qed.
-
-Lemma write_disjoint promises1 mem1 loc from1 to1 val released promises3 mem2 kind
-      (MLE: Memory.le promises1 mem1)
-      (WRITE: Memory.write
-                promises1 mem1 loc from1 to1 val released promises3 mem2 kind)
-      to
-      (INT: Interval.mem (from1, to1) to)
-  :
-    (<<PROMISED: covered loc to promises1>>) \/
-    (<<NEWMSG: ~ covered loc to mem1>>).
-Proof.
-  inv WRITE. inv PROMISE.
-  - right. ii. inv H. inv MEM. inv ADD.
-    exploit DISJOINT; eauto.
-  - left. dup PROMISES. eapply Memory.split_get0 in PROMISES. des.
-    econs; eauto.
-    inv INT. inv PROMISES0. inv SPLIT. econs; ss.
-    etrans; eauto. left. auto.
-  - left. dup PROMISES. eapply Memory.lower_get0 in PROMISES. des.
-    econs; eauto.
-Qed.
-
-Lemma write_msg_wf v prom v' prom'
-      loc from to val releasedm released ord sc sc' mem_tgt mem_tgt' kind
-      (WRITE: Local.write_step
-                (Local.mk v prom) sc mem_tgt
-                loc from to val releasedm released ord
-                (Local.mk v' prom') sc' mem_tgt' kind)
-  :
-    (<<TLE: Time.le
-              (View.rlx (View.unwrap (TView.write_released v sc loc to releasedm ord)) loc) to>>) /\
-    (<<FROMTO: Time.lt from to>>) /\
-    (<<MSGWF: Message.wf (Message.full val (TView.write_released v sc loc to releasedm ord))>>)
-.
-Proof.
-  inv WRITE. inv WRITE0. inv PROMISE.
-  - inv TS. inv MEM. inv ADD. esplits; eauto.
-  - inv TS. inv MEM. inv SPLIT. esplits; eauto.
-  - inv TS. inv MEM. inv LOWER. esplits; eauto.
-Qed.
-
-Lemma self_promise_remove_write v prom v' prom'
-      loc from to val releasedm released ord sc sc' mem_src
-      mem_tgt mem_tgt' kind
-      (WRITE: Local.write_step
-                (Local.mk v prom) sc mem_tgt
-                loc from to val releasedm released ord
-                (Local.mk v' prom') sc' mem_tgt' kind)
-      (MEM: forget_memory (promised prom) mem_src mem_tgt)
-      (LCWF: Local.wf (Local.mk v prom) mem_tgt)
-  :
-    exists mem_src',
-      (<<WRITE: Local.write_step
-                  (Local.mk v Memory.bot) sc mem_src
-                  loc from to val releasedm released ord
-                  (Local.mk v' Memory.bot) sc' mem_src' Memory.op_kind_add>>) /\
-      (<<MEM: forget_memory (promised prom') mem_src' mem_tgt'>>).
-Proof.
-  dup MEM. eapply forget_memory_le in MEM0. inv MEM.
-  inv WRITE. ss. clarify.
-  (* inv WRITE0. *)
-  exploit write_msg_wf; eauto. i. des.
-  exploit write_succeed; eauto.
-  { instantiate (1:=mem_src).
-    ii. inv LCWF. exploit write_disjoint; try apply WRITE0; eauto.
-    i. des.
-    - inv PROMISED. inv COVER. dup GET0.
-      assert (NPRM: ~ promised prom loc to1).
-      { ii. erewrite FORGET in GET0; eauto. clarify. }
-      erewrite COMPLETE in GET0; eauto. exploit Memory.get_disjoint.
-      + eapply GET0.
-      + eapply PROMISES in GET. eapply GET.
-      + i. des; clarify; eauto.
-        eapply NPRM. econs; eauto.
-    - eapply NEWMSG. eapply memory_le_covered; try apply MEM0; eauto. }
-  i. des. exists mem2. esplits; ss.
-  - econs 1; ss; eauto.
-    ii. rewrite Memory.bot_get in *. clarify.
-  - inv WRITE0. inv WRITE. inv PROMISE0. inv PROMISE.
-    + exploit MemoryFacts.MemoryFacts.add_remove_eq.
-      { eapply PROMISES0. }
-      { eapply REMOVE. } i. clarify.
-      econs; i.
-      * erewrite (@Memory.add_o mem2); eauto.
-        erewrite (@Memory.add_o mem_tgt'); cycle 1; eauto.
-        des_ifs. eauto.
-      * erewrite (@Memory.add_o mem2); eauto.
-        des_ifs; eauto. ss. des. clarify. exfalso.
-        eapply Memory.add_get0 in PROMISES0. des. inv PROMS. clarify.
-    + econs; i.
-      * erewrite (@Memory.add_o mem2); eauto.
-        erewrite (@Memory.split_o mem_tgt'); cycle 1; eauto.
-        des_ifs.
-        { ss. destruct a. clarify. des; clarify. exfalso. eapply NPROMS.
-          eapply Memory.split_get0 in PROMISES0. des.
-          econs. erewrite Memory.remove_o; eauto. des_ifs; eauto.
-          des; ss; clarify. }
-        { ss. eapply COMPLETE. ii. eapply NPROMS.
-          inv H. econs. instantiate (1:=msg).
-          erewrite Memory.remove_o; eauto.
-          erewrite Memory.split_o; eauto. des_ifs; ss; des; clarify. }
-      * erewrite (@Memory.add_o mem2); eauto. des_ifs.
-        { ss. des. clarify. exfalso. inv PROMS.
-          erewrite Memory.remove_o in GET; eauto.
-          des_ifs. ss. des; clarify. }
-        { eapply FORGET. inv PROMS.
-          erewrite Memory.remove_o in GET; eauto.
-          erewrite Memory.split_o in GET; eauto. des_ifs.
-          - ss; des; clarify.
-            eapply Memory.split_get0 in PROMISES0. des. econs; eauto.
+  Proof.
+    dup MEM. eapply forget_memory_le in MEM0. inv MEM. inv PROMISE.
+    - econs; eauto.
+      * i. rewrite COMPLETE.
+        { symmetry. erewrite Memory.add_o; eauto. des_ifs.
+          - ss. des. clarify. exfalso. apply NPROMS.
+            apply Memory.add_get0 in PROMISES. des.
+            econs; eauto. }
+        { ii. inv H. eapply NPROMS.
+          exploit Memory.add_o; try apply PROMISES; eauto. i.
+          erewrite GET in *. des_ifs.
+          - econs; eauto.
           - econs; eauto. }
-    + econs; i.
-      * erewrite (@Memory.add_o mem2); eauto.
-        erewrite (@Memory.lower_o mem_tgt'); cycle 1; eauto.
-        des_ifs. eapply COMPLETE.
-        ii. eapply NPROMS. inv H. econs. instantiate (1:=msg).
-        erewrite Memory.remove_o; eauto.
-        erewrite Memory.lower_o; eauto. des_ifs. ss; des; clarify.
-      * erewrite (@Memory.add_o mem2); eauto. des_ifs.
-        { ss. des. clarify. exfalso. inv PROMS.
-          erewrite Memory.remove_o in GET; eauto.
-          des_ifs. ss. des; clarify. }
-        { eapply FORGET. inv PROMS. econs.
-          erewrite Memory.remove_o in GET; eauto.
-          erewrite Memory.lower_o in GET; eauto. des_ifs. eauto. }
-Qed.
+      * i. inv PROMS. destruct msg0.
+        erewrite Memory.add_o in GET; eauto. des_ifs.
+        { ss. des. clarify.
+          eapply memory_le_get_none; eauto.
+          apply Memory.add_get0 in MEM. des. eauto. }
+        { eapply FORGET. econs; eauto. }
+    - econs; eauto.
+      * i. rewrite COMPLETE.
+        { symmetry. erewrite Memory.split_o; eauto. des_ifs.
+          - ss. des. clarify. exfalso. apply NPROMS.
+            apply Memory.split_get0 in PROMISES. des.
+            econs; eauto.
+          - ss. destruct a. clarify. exfalso. apply NPROMS.
+            apply Memory.split_get0 in PROMISES.
+            econs; des; eauto. }
+        { ii. inv H. eapply NPROMS.
+          exploit Memory.split_o; try apply PROMISES; eauto. i.
+          erewrite GET in *. des_ifs.
+          - econs; eauto.
+          - econs; eauto.
+          - econs; eauto. }
+      * i. inv PROMS. destruct msg0.
+        erewrite Memory.split_o in GET; eauto. des_ifs.
+        { ss. des. clarify.
+          eapply memory_le_get_none; eauto.
+          apply Memory.split_get0 in MEM. des. eauto. }
+        { ss. destruct a. clarify.
+          eapply FORGET. apply Memory.split_get0 in PROMISES.
+          econs. des; eauto. }
+        { eapply FORGET. econs; eauto. }
+    - econs; eauto.
+      * i. rewrite COMPLETE.
+        { symmetry. erewrite Memory.lower_o; eauto. des_ifs.
+          - ss. des. clarify. exfalso. apply NPROMS.
+            apply Memory.lower_get0 in PROMISES. des.
+            econs; eauto. }
+        { ii. inv H. eapply NPROMS.
+          exploit Memory.lower_o; try apply PROMISES; eauto. i.
+          erewrite GET in *. des_ifs.
+          - econs; eauto.
+          - econs; eauto. }
+      * i. inv PROMS. destruct msg1.
+        erewrite Memory.lower_o in GET; eauto. des_ifs.
+        { ss. des. clarify. eapply FORGET.
+          apply Memory.lower_get0 in PROMISES. des. econs. eauto. }
+        { eapply FORGET. apply Memory.lower_get0 in PROMISES.
+          econs. des; eauto. }
+  Qed.
 
-Lemma self_promise_remove
-      P lang th_src th_tgt th_tgt' st st' v v' prom prom' sc sc'
-      mem_src mem_tgt mem_tgt' e_tgt
-      (STEP: (@pred_step (P /1\ no_read_msgs prom.(promised)) lang) e_tgt th_tgt th_tgt')
-      (TH_SRC: th_src = Thread.mk lang st (Local.mk v Memory.bot) sc mem_src)
-      (TH_TGT0: th_tgt = Thread.mk lang st (Local.mk v prom) sc mem_tgt)
-      (TH_TGT1: th_tgt' = Thread.mk lang st' (Local.mk v' prom') sc' mem_tgt')
-      (MEM: forget_memory (promised prom) mem_src mem_tgt)
-      (LCWF: Local.wf (Local.mk v prom) mem_tgt)
-      (CLOSED: Memory.closed mem_tgt)
-  :
-    exists mem_src' e_src,
-      (<<STEP: opt_pred_step
-                 (P /1\ no_promise) e_src th_src
-                 (Thread.mk lang st' (Local.mk v' Memory.bot) sc' mem_src')>>) /\
-      (<<EVT: ThreadEvent.get_event e_src = ThreadEvent.get_event e_tgt>>) /\
-      (<<MEM: forget_memory (promised prom') mem_src' mem_tgt'>>).
-Proof.
-  dup MEM. eapply forget_memory_le in MEM0.
-  clarify. inv STEP. des. inv STEP0. inv STEP.
-  - inv STEP0. ss. inv LOCAL. clarify. ss.
-    exists mem_src, ThreadEvent.silent. esplits; eauto.
-    eapply self_promise_remove_promise; eauto.
-  - inv STEP0. ss. inv LOCAL; clarify; ss.
-    + exists mem_src, ThreadEvent.silent.
-      esplits; eauto. econs. econs; ss; eauto. econs; eauto.
-      econs 2; eauto. econs; eauto.
-    + exists mem_src, (ThreadEvent.read loc ts val released ord).
-      inv LOCAL0. ss. clarify.
-      esplits; eauto. econs. econs; ss; eauto. econs; eauto.
-      econs 2; eauto. econs; eauto. econs 2; eauto. econs; eauto.
-      inv MEM. rewrite COMPLETE; eauto.
-    + exploit self_promise_remove_write; eauto. i. des.
-      exists mem_src', (ThreadEvent.write loc from to val released ord).
-      esplits; eauto. econs. econs; eauto. econs; eauto.
-      econs 2; eauto. econs; eauto.
-    + exploit Local.read_step_future; eauto. i. des.
-      inv LOCAL1. ss. exploit self_promise_remove_write; eauto. i. des.
-      exists mem_src',
-      (ThreadEvent.update loc tsr tsw valr valw releasedr releasedw ordr ordw).
-      esplits; eauto. econs. econs; ss; eauto. econs; eauto.
-      econs 2; eauto. econs; eauto. econs; eauto. econs; eauto.
-      inv MEM. rewrite COMPLETE; eauto.
-    + inv LOCAL0. ss. clarify.
-      exists mem_src, (ThreadEvent.fence ordr ordw).
-      esplits; eauto. econs. econs; ss; eauto. econs; eauto.
-      econs 2; eauto. econs; eauto. econs; eauto. econs; eauto. ss.
-      ii. rewrite Memory.bot_get in *. clarify.
-    + inv LOCAL0. ss. clarify.
-      exists mem_src, (ThreadEvent.syscall e).
-      esplits; eauto. econs. econs; ss; eauto. econs; eauto.
-      econs 2; eauto. econs; eauto. econs; eauto. econs; eauto. ss.
-      ii. rewrite Memory.bot_get in *. clarify.
-Qed.
-
-Lemma memory_write_bot_add
-      mem1 loc from1 to1 val released promises3 mem2 kind
-      (WRITE: Memory.write
-                Memory.bot mem1 loc from1 to1 val released promises3 mem2 kind)
-  :
-    kind = Memory.op_kind_add.
-Proof.
-  inv WRITE. inv PROMISE; auto.
-  - exfalso. eapply Memory.split_get0 in PROMISES. des.
-    rewrite Memory.bot_get in *. clarify.
-  - exfalso. eapply Memory.lower_get0 in PROMISES. des.
-    rewrite Memory.bot_get in *. clarify.
-Qed.
-
-Lemma other_promise_remove_write v v' prom'
-      loc from to val releasedm released ord sc sc' mem_src
-      mem_tgt mem_tgt' kind others
-      (WRITE: Local.write_step
-                (Local.mk v Memory.bot) sc mem_tgt
-                loc from to val releasedm released ord
-                (Local.mk v' prom') sc' mem_tgt' kind)
-      (MEM: forget_memory others mem_src mem_tgt)
-      (OTHERS: ~ others loc to)
-  :
-    exists mem_src',
-      (<<WRITE: Local.write_step
-                  (Local.mk v Memory.bot) sc mem_src
-                  loc from to val releasedm released ord
-                  (Local.mk v' Memory.bot) sc' mem_src' Memory.op_kind_add>>) /\
-      (<<MEM: forget_memory others mem_src' mem_tgt'>>).
-Proof.
-  exploit write_msg_wf; eauto. i. des.
-  inv WRITE. ss. clarify. exploit memory_write_bot_add; eauto. i. clarify.
-  dup WRITE0. inv WRITE0. inv PROMISE.
-  exploit write_succeed; eauto.
-  { instantiate (1:=mem_src). i. eapply forget_memory_le in MEM.
-    eapply memory_le_covered in COVER; eauto. ii.
-    exploit write_disjoint; try apply WRITE1; eauto.
-    { eapply Memory.bot_le. }
-    i. des; eauto. inv PROMISED.
-    erewrite Memory.bot_get in GET. clarify. }
-  i. des. exists mem2. econs; eauto.
-  inv MEM. inv WRITE. inv PROMISE. econs; i.
-  - erewrite (@Memory.add_o mem2); eauto.
-    erewrite (@Memory.add_o mem_tgt'); cycle 1; eauto. des_ifs. eauto.
-  - erewrite (@Memory.add_o mem2); eauto. des_ifs; eauto.
-    ss. des. clarify.
-Qed.
-
-Lemma other_promise_remove
-      P lang th_src th_tgt th_tgt' st st' v v' prom' sc sc'
-      mem_src mem_tgt mem_tgt' e_tgt others
-      (STEP: (@pred_step (P /1\ no_read_msgs others /1\ write_not_in others /1\ no_promise) lang) e_tgt th_tgt th_tgt')
-      (TH_SRC: th_src = Thread.mk lang st (Local.mk v Memory.bot) sc mem_src)
-      (TH_TGT0: th_tgt = Thread.mk lang st (Local.mk v Memory.bot) sc mem_tgt)
-      (TH_TGT1: th_tgt' = Thread.mk lang st' (Local.mk v' prom') sc' mem_tgt')
-      (MEM: forget_memory others mem_src mem_tgt)
-  :
-    exists mem_src',
-      (<<STEP: (@pred_step
-                  (P /1\ no_promise) lang)
-                 e_tgt th_src
-                 (Thread.mk lang st' (Local.mk v' Memory.bot) sc' mem_src')>>) /\
-      (<<MEM: forget_memory others mem_src' mem_tgt'>>).
-Proof.
-  dup MEM. eapply forget_memory_le in MEM0.
-  clarify. inv STEP. des. inv STEP0. inv STEP.
-  { inv STEP0. ss; clarify. }
-  inv STEP0. inv LOCAL; ss.
-  - exists mem_src. esplits; eauto. econs; eauto. econs; eauto.
-    econs 2; eauto. econs; eauto.
-  - inv LOCAL0. ss. clarify.
-    exists mem_src. esplits; eauto. econs; eauto. econs; eauto.
-    econs 2; eauto. econs; eauto. econs; eauto. econs; eauto.
-    inv MEM. erewrite COMPLETE; eauto.
-  - ss. exploit other_promise_remove_write; eauto.
-    { exploit write_msg_wf; eauto. i. des.
-      eapply SAT1. econs; eauto. refl. }
-    i. des. exists mem_src'. esplits; eauto.
-    econs; eauto. econs; eauto. econs 2; eauto. econs; eauto.
-  - ss. inv LOCAL1. ss.
-    exploit other_promise_remove_write; eauto.
-    { exploit write_msg_wf; eauto. i. des.
-      eapply SAT1. econs; eauto. refl. }
-    i. des. exists mem_src'. esplits; eauto.
-    econs; eauto. econs; eauto. econs 2; eauto. econs; eauto.
-    econs; eauto. econs; eauto. inv MEM. erewrite COMPLETE; eauto.
-  - inv LOCAL0. ss. clarify. exists mem_src. esplits; eauto.
-    econs; eauto. econs; eauto. econs 2; eauto. econs; eauto.
-  - inv LOCAL0. ss. clarify. exists mem_src. esplits; eauto.
-    econs; eauto. econs; eauto. econs 2; eauto. econs; eauto.
-Qed.
-
-Inductive map_preserving (P: Loc.t -> Time.t -> Prop) (f: Loc.t -> Time.t -> Time.t) :=
-| map_preserving_intro
-    (PRSVLT: forall loc t0 t1 (SAT0: P loc t0) (SAT1: P loc t1) (LT: Time.lt t0 t1),
-        Time.lt (f loc t0) (f loc t1))
-    (PRSVBOT: forall loc, f loc Time.bot = Time.bot)
-.
-
-Definition map_preserving_lt_iff P f
-           (PRSV: map_preserving P f)
-           loc t0 t1
-           (SAT0: P loc t0) (SAT1: P loc t1)
-  :
-    Time.lt t0 t1 <-> Time.lt (f loc t0) (f loc t1).
-Proof.
-  inv PRSV. split; eauto.
-  set (DenseOrder.DenseOrderFacts.OrderTac.TO.lt_total t0 t1). des; eauto.
-  - clarify. i. timetac.
-  - i. eapply PRSVLT in o; eauto. exfalso.
-    assert (LT: Time.lt (f loc t0) (f loc t0)).
-    + etrans; eauto.
-    + timetac.
-Qed.
-Hint Resolve map_preserving_lt_iff.
-
-Definition map_preserving_eq_iff P f
-           (PRSV: map_preserving P f)
-           loc t0 t1
-           (SAT0: P loc t0) (SAT1: P loc t1)
-  :
-    t0 = t1 <-> (f loc t0) = (f loc t1).
-Proof.
-  split; i; clarify; eauto.
-  set (DenseOrder.DenseOrderFacts.OrderTac.TO.lt_total t0 t1). des; eauto.
-  - erewrite map_preserving_lt_iff in o; eauto.
-    rewrite H in *. timetac.
-  - erewrite map_preserving_lt_iff in o; eauto.
-    rewrite H in *. timetac.
-Qed.
-Hint Resolve map_preserving_eq_iff.
-
-Definition map_preserving_le_iff P f
-           (PRSV: map_preserving P f)
-           loc t0 t1
-           (SAT0: P loc t0) (SAT1: P loc t1)
-  :
-    Time.le t0 t1 <-> Time.le (f loc t0) (f loc t1).
-Proof.
-  repeat rewrite DenseOrder.DenseOrder.le_lteq.
-  split; i; des; clarify; eauto.
-  - left. erewrite <- map_preserving_lt_iff; eauto.
-  - left. eapply map_preserving_lt_iff; eauto.
-  - right. eapply map_preserving_eq_iff; eauto.
-Qed.
-Hint Resolve map_preserving_le_iff.
-
-Definition map_preserving_bot P f
-           (PRSV: map_preserving P f)
-           loc
-  :
-    f loc Time.bot = Time.bot.
-Proof.
-  inv PRSV. eauto.
-Qed.
-Hint Resolve map_preserving_bot.
-
-Definition timemap_map (f: Loc.t -> Time.t -> Time.t) (tm: TimeMap.t): TimeMap.t :=
-  fun l => f l (tm l).
-
-Definition view_map (f: Loc.t -> Time.t -> Time.t) (v: View.t): View.t :=
-  View.mk (timemap_map f v.(View.pln)) (timemap_map f v.(View.rlx)).
-
-Definition tview_map (f: Loc.t -> Time.t -> Time.t) (v: TView.t): TView.t :=
-  TView.mk
-    (fun loc => view_map f (v.(TView.rel) loc))
-    (view_map f v.(TView.cur))
-    (view_map f v.(TView.acq)).
-
-Definition msg_map (f: Loc.t -> Time.t -> Time.t) (msg: Message.t): Message.t :=
-  match msg with
-  | Message.half => Message.half
-  | Message.full val released =>
-    Message.full val (option_map (view_map f) released)
-  end.
-
-Definition tevent_map (f: Loc.t -> Time.t -> Time.t) (te: ThreadEvent.t): ThreadEvent.t :=
-  match te with
-  | ThreadEvent.promise loc from to msg kind =>
-    ThreadEvent.promise loc (f loc from) (f loc to) (msg_map f msg) kind
-  | ThreadEvent.read loc to val v o =>
-    ThreadEvent.read loc (f loc to) val (option_map (view_map f) v) o
-  | ThreadEvent.write loc to from val v o =>
-    ThreadEvent.write loc (f loc to) (f loc from) val (option_map (view_map f) v) o
-  | ThreadEvent.update loc to from valr valw vr vw or ow =>
-    ThreadEvent.update loc (f loc to) (f loc from) valr valw (option_map (view_map f) vr) (option_map (view_map f) vw) or ow
-  | ThreadEvent.fence or ow => ThreadEvent.fence or ow
-  | ThreadEvent.syscall e => ThreadEvent.syscall e
-  | _ => ThreadEvent.silent
-  end.
-
-Inductive memory_map f m_src m_tgt: Prop :=
-| memory_map_intro
-    (MAPPED: forall loc to from msg (GET: Memory.get loc to m_tgt = Some (from, msg)),
-        Memory.get loc (f loc to) m_src = Some (f loc from, msg_map f msg))
-    (ONLY: forall loc to_src msg_src (GET: Memory.get loc to_src m_src = Some msg_src),
-        exists to msg,
-          (<<FROM: f loc to = to_src>>) /\
-          (<<GET: Memory.get loc to m_tgt = Some msg>>))
-.
-
-Definition times_in_memory (m: Memory.t) (l: Loc.t) (t: Time.t): Prop :=
-  (<<OFFROM: exists to msg,
-      (<<GET: Memory.get l to m = Some (t, msg)>>)>>) \/
-  (<<OFTO: exists from msg,
-      (<<GET: Memory.get l t m = Some (from, msg)>>)>>)
-.
-
-Definition times_in_memory_to (m: Memory.t) (l: Loc.t) (t: Time.t): Prop :=
-  (<<OFTO: exists from val released,
-      (<<GET: Memory.get l t m = Some (from, Message.full val released)>>)>>)
-.
-
-Lemma times_in_memory_to_in_memory:
-  times_in_memory_to <3= times_in_memory.
-Proof.
-  i. unfold times_in_memory_to in *. des. right. eauto.
-Qed.
-Hint Resolve times_in_memory_to_in_memory.
-
-Lemma map_closed_timemap m f tm
-      (INMEMORY: map_preserving (times_in_memory m) f)
-      (CLOSED: Memory.closed_timemap tm m)
-  :
-    forall loc, times_in_memory m loc (tm loc).
-Proof.
-  ii. right. specialize (CLOSED loc). unfold times_in_memory_to. des. eauto.
-Qed.
-
-Lemma map_time_join P f loc t0 t1
-      (PRSV: map_preserving P f)
-      (SAT0: P loc t0) (SAT1: P loc t1)
-  :
-    f loc (Time.join t0 t1) = Time.join (f loc t0) (f loc t1).
-Proof.
-  unfold Time.join. des_ifs.
-  - erewrite <- map_preserving_lt_iff in l0; eauto.
-    erewrite <- map_preserving_eq_iff; eauto.
-    timetac.
-  - erewrite <- map_preserving_le_iff in l0; eauto.
-    erewrite <- map_preserving_eq_iff; eauto.
-    timetac.
-Qed.
-
-Lemma map_timemap_join f m tm0 tm1
-      (INMEMORY: map_preserving (times_in_memory m) f)
-      (CLOSED0: Memory.closed_timemap tm0 m)
-      (CLOSED1: Memory.closed_timemap tm1 m)
-  :
-    timemap_map f (TimeMap.join tm0 tm1) = TimeMap.join (timemap_map f tm0) (timemap_map f tm1).
-Proof.
-  extensionality t. unfold timemap_map, TimeMap.join.
-  eapply map_time_join; eauto.
-  - eapply map_closed_timemap; eauto.
-  - eapply map_closed_timemap; eauto.
-Qed.
-
-Lemma map_viewjoin f m v0 v1
-      (INMEMORY: map_preserving (times_in_memory m) f)
-      (CLOSED0: Memory.closed_view v0 m)
-      (CLOSED1: Memory.closed_view v1 m)
-  :
-    view_map f (View.join v0 v1) = View.join (view_map f v0) (view_map f v1).
-Proof.
-  inv CLOSED0. inv CLOSED1.
-  unfold view_map, View.join. ss. f_equal.
-  - eapply map_timemap_join; eauto.
-  - eapply map_timemap_join; eauto.
-Qed.
-
-Lemma map_tviewjoin f m tv0 tv1
-      (INMEMORY: map_preserving (times_in_memory m) f)
-      (CLOSED0: TView.closed tv0 m)
-      (CLOSED1: TView.closed tv1 m)
-  :
-    tview_map f (TView.join tv0 tv1) = TView.join (tview_map f tv0) (tview_map f tv1).
-Proof.
-  inv CLOSED0. inv CLOSED1.
-  unfold tview_map, TView.join. ss. f_equal.
-  - extensionality l. eapply map_viewjoin; eauto.
-  - eapply map_viewjoin; eauto.
-  - eapply map_viewjoin; eauto.
-Qed.
-
-Lemma map_timemap_bot P f
-      (PRSV: map_preserving P f)
-  :
-    timemap_map f TimeMap.bot = TimeMap.bot.
-Proof.
-  extensionality loc. unfold timemap_map.
-  erewrite map_preserving_bot; eauto.
-Qed.
-
-Lemma map_view_bot P f
-      (PRSV: map_preserving P f)
-  :
-    view_map f View.bot = View.bot.
-Proof.
-  unfold view_map, View.bot. ss. f_equal.
-  - eapply map_timemap_bot; eauto.
-  - eapply map_timemap_bot; eauto.
-Qed.
-
-Lemma map_unwrap f m released
-      (INMEMORY: map_preserving (times_in_memory m) f)
-      (CLOSED0: Memory.closed_opt_view released m)
-  :
-    view_map f (View.unwrap released) =
-    View.unwrap (option_map (view_map f) released).
-Proof.
-  unfold View.unwrap. des_ifs. eapply map_view_bot; eauto.
-Qed.
-
-Lemma map_timemap_singleton f P loc to
-      (INMEMORY: map_preserving P f)
-      (CLOSED2: P loc to)
-  :
-    timemap_map f (TimeMap.singleton loc to) =
-    TimeMap.singleton loc (f loc to).
-Proof.
-  extensionality l.
-  unfold timemap_map, TimeMap.singleton.
-  setoid_rewrite LocFun.add_spec. des_ifs.
-  rewrite LocFun.init_spec. erewrite map_preserving_bot; eauto.
-Qed.
-
-Lemma map_singleton_ur f P loc to
-      (INMEMORY: map_preserving P f)
-      (CLOSED2: P loc to)
-  :
-    view_map f (View.singleton_ur loc to) =
-    View.singleton_ur loc (f loc to).
-Proof.
-  unfold view_map, View.singleton_ur. ss.
-  erewrite map_timemap_singleton; eauto.
-Qed.
-
-Lemma map_singleton_rw f P loc to
-      (INMEMORY: map_preserving P f)
-      (CLOSED2: P loc to)
-  :
-    view_map f (View.singleton_rw loc to) =
-    View.singleton_rw loc (f loc to).
-Proof.
-  unfold view_map, View.singleton_rw. ss.
-  erewrite map_timemap_singleton; eauto. f_equal.
-  eapply map_timemap_bot; eauto.
-Qed.
-
-Lemma map_singleton_ur_if f P loc to cond
-      (INMEMORY: map_preserving P f)
-      (CLOSED2: P loc to)
-  :
-    view_map f (View.singleton_ur_if cond loc to) =
-    View.singleton_ur_if cond loc (f loc to).
-Proof.
-  unfold view_map, View.singleton_ur_if. des_ifs.
-  - erewrite <- map_singleton_ur; eauto.
-  - erewrite <- map_singleton_rw; eauto.
-Qed.
-
-Lemma map_read_tview f m v loc to released ord
-      (INMEMORY: map_preserving (times_in_memory m) f)
-      (CLOSED0: TView.closed v m)
-      (CLOSED1: Memory.closed_opt_view released m)
-      (CLOSED2: times_in_memory_to m loc to)
-      (INHABITED: Memory.inhabited m)
+  Lemma consistent_read_no_self_promise_read
+        v v' prom prom'
+        mem_tgt loc ts val released ord
+        (STEP: Local.read_step (Local.mk v prom) mem_tgt loc
+                               ts val released ord (Local.mk v' prom'))
+        (CONSISTENT: local_consistent (Local.mk v' prom'))
     :
-    tview_map f (TView.read_tview v loc to released ord) =
-    TView.read_tview (tview_map f v) loc (f loc to) (option_map (view_map f) released) ord.
-Proof.
-  unfold tview_map, TView.read_tview. ss.
-  repeat (erewrite <- map_unwrap; eauto).
-  repeat (erewrite map_viewjoin; eauto).
-  - erewrite map_singleton_ur_if; eauto.
-    des_ifs; f_equal; erewrite map_view_bot; eauto.
-  - inv CLOSED0. eauto.
-  - unfold times_in_memory_to in *. des.
-    eapply Memory.singleton_ur_if_closed_view; eauto.
-  - eapply Memory.join_closed_view; eauto.
-    + inv CLOSED0; eauto.
-    + unfold times_in_memory_to in *. des.
-      eapply Memory.singleton_ur_if_closed_view; eauto.
-  - des_ifs.
-    + eapply Memory.unwrap_closed_opt_view; eauto.
-    + eapply Memory.closed_view_bot; eauto.
-  - inv CLOSED0. eauto.
-  - unfold times_in_memory_to in *. des.
-    eapply Memory.singleton_ur_if_closed_view; eauto.
-  - eapply Memory.join_closed_view; eauto.
-    + inv CLOSED0; eauto.
-    + unfold times_in_memory_to in *. des.
-      eapply Memory.singleton_ur_if_closed_view; eauto.
-  - des_ifs.
-    + eapply Memory.unwrap_closed_opt_view; eauto.
-    + eapply Memory.closed_view_bot; eauto.
-Qed.
+      ~ prom.(promised) loc ts.
+  Proof.
+    ii. inv H. inv STEP. ss. clarify.
+    exploit CONSISTENT; ss; eauto.
+    { econs; eauto. }
+    unfold TimeMap.join. i.
+    apply TimeFacts.join_lt_des in x. des.
+    apply TimeFacts.join_lt_des in AC. des.
+    unfold View.singleton_ur_if, View.singleton_ur in *. clear - BC0. des_ifs; ss.
+    * unfold TimeMap.singleton in *.
+      setoid_rewrite LocFun.add_spec_eq in BC0. timetac.
+    * unfold TimeMap.singleton in *.
+      setoid_rewrite LocFun.add_spec_eq in BC0. timetac.
+  Qed.
 
-Lemma map_step_read
-      f v v' prom'
-      mem_src mem_tgt loc to val released ord
-      (STEP: Local.read_step (Local.mk v Memory.bot) mem_tgt loc to val released ord
-                             (Local.mk v' prom'))
-      (INMEMORY0: map_preserving (times_in_memory mem_tgt) f)
-      (CLOSED0: Memory.closed mem_tgt)
-      (LCWF: Local.wf (Local.mk v Memory.bot) mem_tgt)
-      (MEM: memory_map f mem_src mem_tgt)
-      (INHABITED: Memory.inhabited mem_tgt)
-  :
-    (<<STEP: Local.read_step (Local.mk (tview_map f v) Memory.bot) mem_src loc
-                             (f loc to) val (option_map (view_map f) released) ord
-                             (Local.mk (tview_map f v') Memory.bot)>>).
-Proof.
-  inv STEP. ss. clarify. econs; eauto.
-  + inv MEM. exploit MAPPED; eauto.
-  + ss. inv READABLE. unfold view_map, option_map, timemap_map. des_ifs.
-    * econs; ss; eauto.
-      { erewrite <- map_preserving_le_iff; eauto.
-        - inv LCWF. ss. inv TVIEW_CLOSED. inv CUR.
-          eapply map_closed_timemap; eauto.
-        - right. eauto. }
-      { i. erewrite <- map_preserving_le_iff; eauto.
-        - inv LCWF. ss. inv TVIEW_CLOSED. inv CUR.
-          eapply map_closed_timemap; eauto.
-        - right. eauto. }
-    * econs; ss; eauto.
-      { erewrite <- map_preserving_le_iff; eauto.
-        - inv LCWF. ss. inv TVIEW_CLOSED. inv CUR.
-          eapply map_closed_timemap; eauto.
-        - right. eauto. }
-      { i. erewrite <- map_preserving_le_iff; eauto.
-        - inv LCWF. ss. inv TVIEW_CLOSED. inv CUR.
-          eapply map_closed_timemap; eauto.
-        - right. eauto. }
-  + ss. f_equal. erewrite map_read_tview; eauto.
-    * inv LCWF. ss.
-    * eapply CLOSED0 in GET. des. inv MSG_CLOSED. eauto.
-    * unfold times_in_memory_to. eauto.
-Qed.
+  Lemma consistent_read_no_self_promise
+        lang th_tgt th_tgt' st st' v v' prom prom' sc sc'
+        mem_tgt mem_tgt' pf e_tgt
+        (LOCALWF: Local.wf (Local.mk v prom) mem_tgt)
+        (CLOSED: Memory.closed mem_tgt)
+        (SC: Memory.closed_timemap sc mem_tgt)
+        (TH_TGT0: th_tgt = Thread.mk lang st (Local.mk v prom) sc mem_tgt)
+        (TH_TGT1: th_tgt' = Thread.mk lang st' (Local.mk v' prom') sc' mem_tgt')
+        (CONSISTENT: local_consistent (Local.mk v' prom'))
+        (STEP: Thread.step pf e_tgt th_tgt th_tgt')
+    :
+      no_read_msgs prom.(promised) e_tgt.
+  Proof.
+    inv STEP; ss.
+    - inv STEP0. ss.
+    - inv STEP0. inv LOCAL; ss.
+      + ii. exploit consistent_read_no_self_promise_read; eauto.
+      + ii. destruct lc2. hexploit consistent_read_no_self_promise_read; eauto.
+        exploit Local.read_step_future; eauto. i. des.
+        eapply local_consistent_write; eauto.
+  Qed.
 
-Lemma view_map_le f m tm0 tm1
-      (INMEMORY: map_preserving (times_in_memory m) f)
-      (CLOSED0: Memory.closed_timemap tm0 m)
-      (CLOSED1: Memory.closed_timemap tm1 m)
-      (LE: TimeMap.le tm0 tm1)
-  :
-    TimeMap.le (timemap_map f tm0) (timemap_map f tm1).
-Proof.
-  ii. unfold timemap_map.
-  erewrite <- map_preserving_le_iff; eauto.
-  - right. specialize (CLOSED0 loc). des. eauto.
-  - right. specialize (CLOSED1 loc). des. eauto.
-Qed.
+End NOREADSELFPROMS.
 
-Lemma view_map_wf f m view
-      (INMEMORY: map_preserving (times_in_memory m) f)
-      (CLOSED0: Memory.closed_view view m)
-      (WF : View.wf view)
-  :
-    View.wf (view_map f view).
-Proof.
-  unfold view_map. ss. econs. inv WF.
-  inv CLOSED0. eapply view_map_le in PLN_RLX; eauto.
-Qed.
 
-Lemma map_write_released f m v sc loc to releasedm ord
-      (INMEMORY0: map_preserving (times_in_memory m) f)
-      (INHABITED: Memory.inhabited m)
-      (CLOSED0: Memory.closed m)
-      (CLOSED1: Memory.closed_opt_view releasedm m)
-      (CLOSED2: times_in_memory_to m loc to)
-      (CLOSED3: TView.closed v m)
-      (CLOSED4: Memory.closed_timemap sc m)
-  :
-    option_map (view_map f) (TView.write_released v sc loc to releasedm ord) =
-    TView.write_released (tview_map f v) (timemap_map f sc) loc (f loc to)
-                         (option_map (view_map f) releasedm) ord.
-Proof.
-  dup CLOSED2. unfold times_in_memory_to in CLOSED2. des.
-  exploit TViewFacts.get_closed_released; eauto.
-  instantiate (1:=ord). i.
-  unfold TView.write_released in *. des_ifs. unfold option_map.
-  erewrite map_viewjoin; eauto.
-  - f_equal. erewrite map_unwrap; eauto. f_equal.
-    setoid_rewrite LocFun.add_spec_eq.
-    des_ifs.
-    + erewrite map_viewjoin; eauto.
-      * erewrite map_singleton_ur; eauto.
-      * inv CLOSED3. eauto.
-      * unfold times_in_memory_to in *. des.
-        eapply Memory.singleton_ur_closed_view; eauto.
-    + erewrite map_viewjoin; eauto.
-      * erewrite map_singleton_ur; eauto.
-      * inv CLOSED3. eauto.
-      * unfold times_in_memory_to in *. des.
-        eapply Memory.singleton_ur_closed_view; eauto.
-  - eapply Memory.unwrap_closed_opt_view; eauto.
-  - exploit TViewFacts.get_closed_tview; eauto. i.
-    inv x1. eauto.
-Qed.
+Section SELFPROMISEREMOVE.
 
-Lemma map_write_tview f m v sc ord loc to
-      (INMEMORY: map_preserving (times_in_memory m) f)
-      (INHABITED: Memory.inhabited m)
-      (CLOSED0: TView.closed v m)
-      (CLOSED1: Memory.closed_timemap sc m)
-      (CLOSED2: times_in_memory_to m loc to)
-  :
-    tview_map f (TView.write_tview v sc loc to ord) =
-    TView.write_tview (tview_map f v) (timemap_map f sc) loc (f loc to) ord.
-Proof.
-  unfold TView.write_tview. ss. unfold tview_map at 1. ss. f_equal.
-  - extensionality l. des_ifs.
-    + setoid_rewrite LocFun.add_spec. des_ifs.
-      erewrite map_viewjoin; eauto.
-      * f_equal. erewrite map_singleton_ur; eauto.
-      * inv CLOSED0. eauto.
-      * unfold times_in_memory_to in *. des.
-        eapply Memory.singleton_ur_closed_view; eauto.
-    + setoid_rewrite LocFun.add_spec. des_ifs.
-      erewrite map_viewjoin; eauto.
-      * f_equal. erewrite map_singleton_ur; eauto.
-      * inv CLOSED0. eauto.
-      * unfold times_in_memory_to in *. des.
-        eapply Memory.singleton_ur_closed_view; eauto.
-  - erewrite map_viewjoin; eauto.
-    + f_equal. erewrite map_singleton_ur; eauto.
-    + inv CLOSED0. eauto.
-    + unfold times_in_memory_to in *. des.
-      eapply Memory.singleton_ur_closed_view; eauto.
-  - erewrite map_viewjoin; eauto.
-    + f_equal. erewrite map_singleton_ur; eauto.
-    + inv CLOSED0. eauto.
-    + unfold times_in_memory_to in *. des.
-      eapply Memory.singleton_ur_closed_view; eauto.
-Qed.
-
-Lemma map_step_write f v v' prom'
-      loc from to val releasedm released ord sc sc' mem_src
-      mem_tgt mem_tgt' kind
-      (WRITE: Local.write_step
-                (Local.mk v Memory.bot) sc mem_tgt
-                loc from to val releasedm released ord
-                (Local.mk v' prom') sc' mem_tgt' kind)
-      (INMEMORY0: map_preserving (times_in_memory mem_tgt) f)
-      (INMEMORY1: map_preserving (times_in_memory mem_tgt') f)
-      (CLOSED0: Memory.closed mem_tgt)
-      (CLOSED1: View.opt_wf releasedm)
-      (CLOSED2: Memory.closed_opt_view releasedm mem_tgt)
-      (CLOSED3: Memory.closed_timemap sc mem_tgt)
-      (LCWF: Local.wf (Local.mk v Memory.bot) mem_tgt)
-      (MEM: memory_map f mem_src mem_tgt)
-      (INHABITED: Memory.inhabited mem_tgt)
-  :
-    exists mem_src',
-      (<<WRITE: Local.write_step
-                  (Local.mk (tview_map f v) Memory.bot)
-                  (timemap_map f sc)
-                  mem_src loc (f loc from) (f loc to) val
-                  (option_map (view_map f) releasedm)
-                  (option_map (view_map f) released) ord
-                  (Local.mk (tview_map f v') Memory.bot)
-                  (timemap_map f sc') mem_src' Memory.op_kind_add>>) /\
-      (<<MEM: memory_map f mem_src' mem_tgt'>>).
-Proof.
-  inv LCWF. exploit write_msg_wf; eauto. i. des.
-  dup WRITE. inv WRITE. ss. clarify. exploit memory_write_bot_add; eauto. i. clarify.
-  assert (CLOSEDV1: Memory.closed_opt_view (TView.write_released v sc loc to releasedm ord) mem_tgt').
-  { inv WRITE1. inv PROMISE. ss.
-    eapply TViewFacts.write_future; eauto. }
-  exploit Local.write_step_future; eauto. i. ss. des.
-  inv WRITE1. inv PROMISE. dup MEM0. eapply Memory.add_get0 in MEM1. des.
-  exploit write_succeed.
-  { instantiate (1:=f loc to). instantiate (1:=f loc from).
-    instantiate (1:=mem_src). instantiate (1:=loc).
-    ii. inv COVER.
-    inv MEM. ss. exploit ONLY; eauto. i. des. clarify.
-    destruct msg0. dup GET2. eapply MAPPED in GET2. clarify.
-    dup GET3. eapply Memory.add_get1 in GET3; eauto.
-    destruct H. destruct ITV. ss.
-    assert (LT0: Time.lt (f loc t0) (f loc to)).
-    { eapply DenseOrder.DenseOrderFacts.lt_le_lt; eauto. }
-    assert (LT1: Time.lt (f loc from) (f loc to1)).
-    { eapply DenseOrder.DenseOrderFacts.lt_le_lt; eauto. }
-    assert (LT2: Time.lt (f loc from) (f loc to)).
-    { eapply DenseOrder.DenseOrderFacts.lt_le_lt; try apply FROM; eauto. }
-    assert (LT3: Time.lt (f loc t0) (f loc to1)).
-    { eapply DenseOrder.DenseOrderFacts.lt_le_lt; try apply FROM0; eauto. }
-    erewrite <- map_preserving_lt_iff in LT0; eauto; cycle 1.
-    { left. eauto. }
-    { right. eauto. }
-    erewrite <- map_preserving_lt_iff in LT1; eauto; cycle 1.
-    { left. eauto. }
-    { right. eauto. }
-    erewrite <- map_preserving_lt_iff in LT2; eauto; cycle 1.
-    { left. eauto. }
-    { right. eauto. }
-    erewrite <- map_preserving_lt_iff in LT3; eauto; cycle 1.
-    { left. eauto. }
-    { right. eauto. }
-    exploit Memory.get_disjoint.
-    - eapply GET3.
-    - eapply GET0.
-    - i. des; clarify.
-      exploit Time.middle_spec.
-      { instantiate (1:=Time.meet to to1). instantiate (1:=Time.join from t0).
-        unfold Time.join, Time.meet. des_ifs. } i. des.
-      eapply x0.
-      + instantiate (1:=Time.middle (Time.join from t0) (Time.meet to to1)). econs; ss.
-        * eapply DenseOrder.DenseOrderFacts.le_lt_lt; eauto. eapply Time.join_r.
-        * left. eapply DenseOrder.DenseOrderFacts.lt_le_lt; eauto. eapply Time.meet_r.
-      + econs; ss.
-        * eapply DenseOrder.DenseOrderFacts.le_lt_lt; eauto. eapply Time.join_l.
-        * left. eapply DenseOrder.DenseOrderFacts.lt_le_lt; eauto. eapply Time.meet_l. }
-  { instantiate (1:=option_map
-                      (view_map f)
-                      (TView.write_released v sc loc to releasedm ord)).
-    erewrite map_preserving_le_iff in REL_TS; try apply INMEMORY1; eauto.
-    - instantiate (1:=loc) in REL_TS.
-      setoid_rewrite <- map_unwrap; try apply INMEMORY1; eauto.
-    - right. eapply Memory.unwrap_closed_opt_view in CLOSEDV1; eauto.
-      + inv CLOSEDV1. specialize (RLX loc). des. eauto.
-      + eapply inhabited_future; eauto.
-    - right. eauto. }
-  { erewrite <- map_preserving_lt_iff; eauto.
-    - left. eauto.
-    - right. eauto. }
-  { econs. inv REL_WF; ss. econs. eapply view_map_wf; try apply INMEMORY1; eauto.
-    inv CLOSEDV1; congruence. }
-  i. des. exists mem2. esplits; eauto.
-  - econs; ss; eauto.
-    + erewrite map_write_released; try apply INMEMORY1; eauto.
-      * eapply inhabited_future; eauto.
-      * eapply Memory.future_closed_opt_view; eauto.
-      * unfold times_in_memory_to. eauto.
-      * eapply TView.future_closed; eauto.
-    + inv WRITABLE. econs. unfold view_map, timemap_map. ss.
-      erewrite <- map_preserving_lt_iff; eauto.
-      * eapply TView.future_closed in TVIEW_CLOSED; eauto.
-        inv TVIEW_CLOSED. inv CUR. specialize (RLX loc). des.
-        unfold times_in_memory. eauto.
-      * unfold times_in_memory. eauto.
-    + f_equal. eapply map_write_tview; eauto.
-      * eapply inhabited_future; eauto.
-      * eapply TView.future_closed; eauto.
-      * unfold times_in_memory_to. eauto.
-  - inv WRITE. inv PROMISE. econs.
-    + i. erewrite Memory.add_o in GET1; eauto.
-      erewrite Memory.add_o; eauto. des_ifs; ss.
-      * des; clarify.
-      * des; clarify. exfalso.
-        erewrite <- map_preserving_eq_iff in a0; eauto.
-        { right. eapply Memory.add_get1 in GET1; eauto. }
-        { right. eauto. }
-      * des; clarify.
-      * inv MEM. eauto.
-    + i. erewrite Memory.add_o in GET1; eauto. des_ifs.
-      * ss; des; clarify. esplits; eauto.
-      * inv MEM. exploit ONLY; eauto. i.
-        destruct x as [to0 [msg [FROM GET2]]].
-        exists to0, msg. esplits; eauto.
-        erewrite Memory.add_o; eauto. des_ifs.
-        ss. des; clarify.
-Qed.
-
-Lemma map_read_fence_tview f v ord
-  :
-    tview_map f (TView.read_fence_tview v ord) =
-    TView.read_fence_tview (tview_map f v) ord.
-Proof.
-  unfold TView.read_fence_tview, tview_map. ss. f_equal.
-  des_ifs.
-Qed.
-
-Lemma map_write_fence_sc f m v sc ord
-      (INMEMORY: map_preserving (times_in_memory m) f)
-      (CLOSED0: TView.closed v m)
-      (CLOSED1: Memory.closed_timemap sc m)
-  :
-    timemap_map f (TView.write_fence_sc v sc ord) =
-    TView.write_fence_sc (tview_map f v) (timemap_map f sc) ord.
-Proof.
-  unfold TView.write_fence_sc. ss.
-  extensionality loc. des_ifs.
-  erewrite map_timemap_join; eauto.
-  inv CLOSED0. inv CUR. eauto.
-Qed.
-
-Lemma map_read_fence f v ord
-  :
-    tview_map f (TView.read_fence_tview v ord) =
-    TView.read_fence_tview (tview_map f v) ord.
-Proof.
-  unfold TView.read_fence_tview, tview_map. ss. f_equal. des_ifs.
-Qed.
-
-Lemma write_fence_sc_closed v sc ord m
-      (CLOSED0: TView.closed v m)
-      (CLOSED1: Memory.closed_timemap sc m)
-  :
-    Memory.closed_timemap (TView.write_fence_sc v sc ord) m.
-Proof.
-  unfold TView.write_fence_sc. des_ifs.
-  eapply Memory.join_closed_timemap; eauto.
-  inv CLOSED0. inv CUR. auto.
-Qed.
-
-Lemma read_fence_closed tview ord m
-      (CLOSED0: TView.closed tview m)
-  :
-    TView.closed (TView.read_fence_tview tview ord) m.
-Proof.
-  unfold TView.read_fence_tview. inv CLOSED0. des_ifs.
-Qed.
-
-Lemma map_write_fence_tview f m v sc ord
-      (INMEMORY: map_preserving (times_in_memory m) f)
-      (CLOSED0: TView.closed v m)
-      (CLOSED1: Memory.closed_timemap sc m)
-      (INHABITED: Memory.inhabited m)
-  :
-    tview_map f (TView.write_fence_tview v sc ord) =
-    TView.write_fence_tview (tview_map f v) (timemap_map f sc) ord.
-Proof.
-  unfold TView.write_fence_tview. ss.
-  erewrite <- map_write_fence_sc; eauto.
-  unfold tview_map at 1. ss. f_equal.
-  - extensionality loc. des_ifs.
-  - des_ifs.
-  - erewrite map_viewjoin; eauto.
-    + des_ifs. erewrite map_view_bot; eauto.
-    + inv CLOSED0. inv ACQ. auto.
-    + des_ifs.
-      * econs; ss; eapply write_fence_sc_closed; eauto.
-      * eapply Memory.closed_view_bot; eauto.
-Qed.
-
-Lemma map_step
-      f lang th_src th_tgt th_tgt' st st' v v' prom' sc sc'
-      mem_src mem_tgt mem_tgt' e_tgt
-      (STEP: (@pred_step no_promise lang) e_tgt th_tgt th_tgt')
-      (TH_SRC: th_src = Thread.mk lang st (Local.mk (tview_map f v) Memory.bot)
-                                  (timemap_map f sc) mem_src)
-      (TH_TGT0: th_tgt = Thread.mk lang st (Local.mk v Memory.bot) sc mem_tgt)
-      (TH_TGT1: th_tgt' = Thread.mk lang st' (Local.mk v' prom') sc' mem_tgt')
-      (INMEMORY0: map_preserving (times_in_memory mem_tgt) f)
-      (INMEMORY1: map_preserving (times_in_memory mem_tgt') f)
-      (CLOSEDMAP0: Memory.closed_timemap sc mem_tgt)
-      (CLOSED0: Memory.closed mem_tgt)
-      (LCWF: Local.wf (Local.mk v Memory.bot) mem_tgt)
-      (INHABITED: Memory.inhabited mem_tgt)
-      (MEM: memory_map f mem_src mem_tgt)
-  :
-    exists mem_src',
-      (<<STEP: (@pred_step no_promise lang)
-                 (tevent_map f e_tgt) th_src
-                 (Thread.mk lang st' (Local.mk (tview_map f v') Memory.bot) (timemap_map f sc') mem_src')>>) /\
-      (<<MEM: memory_map f mem_src' mem_tgt'>>).
-Proof.
-  clarify. inv STEP. inv STEP0. inv STEP; inv STEP0; ss. inv LOCAL; ss.
-  - exists mem_src. esplits; ss; eauto.
-    econs; eauto. econs; eauto. econs 2; eauto. econs; eauto.
-  - exploit map_step_read; eauto. i. des.
-    exists mem_src. esplits; eauto. econs; eauto. econs; eauto.
-    econs 2; eauto. econs; eauto.
-  - exploit map_step_write; eauto. i. des. ss.
-    exists mem_src'. esplits; eauto. econs; eauto. econs; eauto.
-    econs 2; eauto. econs; eauto.
-  - exploit Local.read_step_future; eauto. i. des.
-    destruct lc2. exploit map_step_read; eauto. i. des.
-    inv LOCAL1. ss. clarify.
-    exploit map_step_write; eauto. i. des.
-    exists mem_src'. esplits; eauto. econs; eauto. econs; eauto.
-    econs 2; eauto. econs; eauto.
-  - exists mem_src. esplits; eauto. econs; eauto. econs; eauto.
-    econs 2; eauto. econs; eauto. econs; eauto.
-    inv LOCAL0. ss. clarify.
-    erewrite map_write_fence_tview; eauto; cycle 1.
-    { eapply read_fence_closed; eauto. inv LCWF. eauto. }
-    repeat erewrite map_read_fence. econs; ss; eauto.
-    erewrite map_write_fence_sc; eauto.
-    + erewrite map_read_fence. auto.
-    + eapply read_fence_closed; eauto. inv LCWF. eauto.
-  - exists mem_src. esplits; eauto. econs; eauto. econs; eauto.
-    econs 2; eauto. econs; eauto. econs; eauto.
-    inv LOCAL0. ss. clarify.
-    erewrite map_write_fence_tview; eauto; cycle 1.
-    { eapply read_fence_closed; eauto. inv LCWF. eauto. }
-    repeat erewrite map_read_fence. econs; ss; eauto.
-    erewrite map_write_fence_sc; eauto.
-    eapply read_fence_closed; eauto. inv LCWF. eauto.
-Qed.
-
-Lemma unchanged_on_write v v' prom'
-      L loc from to val releasedm released ord sc sc' mem_src
-      mem_tgt mem_tgt' kind
-      (WRITE: Local.write_step
-                (Local.mk v Memory.bot) sc mem_tgt
-                loc from to val releasedm released ord
-                (Local.mk v' prom') sc' mem_tgt' kind)
-      (MEM: unchanged_on L mem_tgt mem_src)
-      (WRITEIN: forall t (IN: Interval.mem (from, to) t), (L loc t))
+  Lemma self_promise_remove_write v prom v' prom'
+        loc from to val releasedm released ord sc sc' mem_src
+        mem_tgt mem_tgt' kind
+        (WRITE: Local.write_step
+                  (Local.mk v prom) sc mem_tgt
+                  loc from to val releasedm released ord
+                  (Local.mk v' prom') sc' mem_tgt' kind)
+        (MEM: forget_memory (promised prom) mem_src mem_tgt)
+        (LCWF: Local.wf (Local.mk v prom) mem_tgt)
   :
     exists mem_src',
       (<<WRITE: Local.write_step
                   (Local.mk v Memory.bot) sc mem_src
                   loc from to val releasedm released ord
                   (Local.mk v' Memory.bot) sc' mem_src' Memory.op_kind_add>>) /\
-      (<<MEM: unchanged_on L mem_tgt' mem_src'>>).
-Proof.
-  inv MEM. inv WRITE. ss. clarify. exploit memory_write_bot_add; eauto. i. clarify.
-  exploit write_msg_wf; eauto. i. des.
-  inv WRITE0. inv PROMISE. dup MEM. eapply Memory.add_get0 in MEM; eauto. des.
-  exploit write_succeed; eauto.
-  { instantiate (1:=mem_src). ii.
-    exploit NCOV; eauto. intros COV. inv COV.
-    exploit Memory.get_disjoint.
-    - eapply GET0.
-    - eapply Memory.add_get1; eauto.
-    - i. des; clarify. eauto. }
-  i. des.
-  exists mem2. esplits; eauto.
-  inv WRITE. inv PROMISE.
-  econs; eauto.
-  - ii. inv COV. erewrite Memory.add_o in GET1; cycle 1; eauto. des_ifs.
-    + ss. des. clarify. econs; eauto.
-    + exploit NCOV; eauto.
-      * econs; eauto.
-      * i. inv x. econs; eauto. eapply Memory.add_get1; eauto.
-  - ii. erewrite Memory.add_o; eauto.
-    erewrite Memory.add_o in LHS; cycle 1; eauto. des_ifs.
-    eapply FUTURE; eauto.
-Qed.
+      (<<MEM: forget_memory (promised prom') mem_src' mem_tgt'>>).
+  Proof.
+    dup MEM. eapply forget_memory_le in MEM0. inv MEM.
+    inv WRITE. ss. clarify.
+    (* inv WRITE0. *)
+    exploit write_msg_wf; eauto. i. des.
+    exploit write_succeed; eauto.
+    { instantiate (1:=mem_src).
+      ii. inv LCWF. exploit write_disjoint; try apply WRITE0; eauto.
+      i. des.
+      - inv PROMISED. inv COVER. dup GET0.
+        assert (NPRM: ~ promised prom loc to1).
+        { ii. erewrite FORGET in GET0; eauto. clarify. }
+        erewrite COMPLETE in GET0; eauto. exploit Memory.get_disjoint.
+        + eapply GET0.
+        + eapply PROMISES in GET. eapply GET.
+        + i. des; clarify; eauto.
+          eapply NPRM. econs; eauto.
+      - eapply NEWMSG. eapply memory_le_covered; try apply MEM0; eauto. }
+    i. des. exists mem2. esplits; ss.
+    - econs 1; ss; eauto.
+      ii. rewrite Memory.bot_get in *. clarify.
+    - inv WRITE0. inv WRITE. inv PROMISE0. inv PROMISE.
+      + exploit MemoryFacts.MemoryFacts.add_remove_eq.
+        { eapply PROMISES0. }
+        { eapply REMOVE. } i. clarify.
+        econs; i.
+        * erewrite (@Memory.add_o mem2); eauto.
+          erewrite (@Memory.add_o mem_tgt'); cycle 1; eauto.
+          des_ifs. eauto.
+        * erewrite (@Memory.add_o mem2); eauto.
+          des_ifs; eauto. ss. des. clarify. exfalso.
+          eapply Memory.add_get0 in PROMISES0. des. inv PROMS. clarify.
+      + econs; i.
+        * erewrite (@Memory.add_o mem2); eauto.
+          erewrite (@Memory.split_o mem_tgt'); cycle 1; eauto.
+          des_ifs.
+          { ss. destruct a. clarify. des; clarify. exfalso. eapply NPROMS.
+            eapply Memory.split_get0 in PROMISES0. des.
+            econs. erewrite Memory.remove_o; eauto. des_ifs; eauto.
+            des; ss; clarify. }
+          { ss. eapply COMPLETE. ii. eapply NPROMS.
+            inv H. econs. instantiate (1:=msg).
+            erewrite Memory.remove_o; eauto.
+            erewrite Memory.split_o; eauto. des_ifs; ss; des; clarify. }
+        * erewrite (@Memory.add_o mem2); eauto. des_ifs.
+          { ss. des. clarify. exfalso. inv PROMS.
+            erewrite Memory.remove_o in GET; eauto.
+            des_ifs. ss. des; clarify. }
+          { eapply FORGET. inv PROMS.
+            erewrite Memory.remove_o in GET; eauto.
+            erewrite Memory.split_o in GET; eauto. des_ifs.
+            - ss; des; clarify.
+              eapply Memory.split_get0 in PROMISES0. des. econs; eauto.
+            - econs; eauto. }
+      + econs; i.
+        * erewrite (@Memory.add_o mem2); eauto.
+          erewrite (@Memory.lower_o mem_tgt'); cycle 1; eauto.
+          des_ifs. eapply COMPLETE.
+          ii. eapply NPROMS. inv H. econs. instantiate (1:=msg).
+          erewrite Memory.remove_o; eauto.
+          erewrite Memory.lower_o; eauto. des_ifs. ss; des; clarify.
+        * erewrite (@Memory.add_o mem2); eauto. des_ifs.
+          { ss. des. clarify. exfalso. inv PROMS.
+            erewrite Memory.remove_o in GET; eauto.
+            des_ifs. ss. des; clarify. }
+          { eapply FORGET. inv PROMS. econs.
+            erewrite Memory.remove_o in GET; eauto.
+            erewrite Memory.lower_o in GET; eauto. des_ifs. eauto. }
+  Qed.
 
-Lemma unchanged_on_step
-      P L lang th_src th_tgt th_tgt' st st' v v' prom' sc sc'
-      mem_src mem_tgt mem_tgt' e_tgt
-      (STEP: (@pred_step (P /1\ write_in L /1\ no_promise) lang) e_tgt th_tgt th_tgt')
-      (TH_SRC: th_src = Thread.mk lang st (Local.mk v Memory.bot) sc mem_src)
-      (TH_TGT0: th_tgt = Thread.mk lang st (Local.mk v Memory.bot) sc mem_tgt)
-      (TH_TGT1: th_tgt' = Thread.mk lang st' (Local.mk v' prom') sc' mem_tgt')
-      (MEM: unchanged_on L mem_tgt mem_src)
+  Lemma self_promise_remove
+        P lang th_src th_tgt th_tgt' st st' v v' prom prom' sc sc'
+        mem_src mem_tgt mem_tgt' e_tgt
+        (STEP: (@pred_step (P /1\ no_read_msgs prom.(promised)) lang) e_tgt th_tgt th_tgt')
+        (TH_SRC: th_src = Thread.mk lang st (Local.mk v Memory.bot) sc mem_src)
+        (TH_TGT0: th_tgt = Thread.mk lang st (Local.mk v prom) sc mem_tgt)
+        (TH_TGT1: th_tgt' = Thread.mk lang st' (Local.mk v' prom') sc' mem_tgt')
+        (MEM: forget_memory (promised prom) mem_src mem_tgt)
+        (LCWF: Local.wf (Local.mk v prom) mem_tgt)
+        (CLOSED: Memory.closed mem_tgt)
+    :
+      exists mem_src' e_src,
+        (<<STEP: opt_pred_step
+                   (P /1\ no_promise) e_src th_src
+                   (Thread.mk lang st' (Local.mk v' Memory.bot) sc' mem_src')>>) /\
+        (<<EVT: ThreadEvent.get_event e_src = ThreadEvent.get_event e_tgt>>) /\
+        (<<MEM: forget_memory (promised prom') mem_src' mem_tgt'>>).
+  Proof.
+    dup MEM. eapply forget_memory_le in MEM0.
+    clarify. inv STEP. des. inv STEP0. inv STEP.
+    - inv STEP0. ss. inv LOCAL. clarify. ss.
+      exists mem_src, ThreadEvent.silent. esplits; eauto.
+      eapply self_promise_remove_promise; eauto.
+    - inv STEP0. ss. inv LOCAL; clarify; ss.
+      + exists mem_src, ThreadEvent.silent.
+        esplits; eauto. econs. econs; ss; eauto. econs; eauto.
+        econs 2; eauto. econs; eauto.
+      + exists mem_src, (ThreadEvent.read loc ts val released ord).
+        inv LOCAL0. ss. clarify.
+        esplits; eauto. econs. econs; ss; eauto. econs; eauto.
+        econs 2; eauto. econs; eauto. econs 2; eauto. econs; eauto.
+        inv MEM. rewrite COMPLETE; eauto.
+      + exploit self_promise_remove_write; eauto. i. des.
+        exists mem_src', (ThreadEvent.write loc from to val released ord).
+        esplits; eauto. econs. econs; eauto. econs; eauto.
+        econs 2; eauto. econs; eauto.
+      + exploit Local.read_step_future; eauto. i. des.
+        inv LOCAL1. ss. exploit self_promise_remove_write; eauto. i. des.
+        exists mem_src',
+        (ThreadEvent.update loc tsr tsw valr valw releasedr releasedw ordr ordw).
+        esplits; eauto. econs. econs; ss; eauto. econs; eauto.
+        econs 2; eauto. econs; eauto. econs; eauto. econs; eauto.
+        inv MEM. rewrite COMPLETE; eauto.
+      + inv LOCAL0. ss. clarify.
+        exists mem_src, (ThreadEvent.fence ordr ordw).
+        esplits; eauto. econs. econs; ss; eauto. econs; eauto.
+        econs 2; eauto. econs; eauto. econs; eauto. econs; eauto. ss.
+        ii. rewrite Memory.bot_get in *. clarify.
+      + inv LOCAL0. ss. clarify.
+        exists mem_src, (ThreadEvent.syscall e).
+        esplits; eauto. econs. econs; ss; eauto. econs; eauto.
+        econs 2; eauto. econs; eauto. econs; eauto. econs; eauto. ss.
+        ii. rewrite Memory.bot_get in *. clarify.
+  Qed.
+
+
+End SELFPROMISEREMOVE.
+
+
+Section OTHERPROMISEREMOVE.
+
+  Lemma other_promise_remove_write v v' prom'
+        loc from to val releasedm released ord sc sc' mem_src
+        mem_tgt mem_tgt' kind others
+        (WRITE: Local.write_step
+                  (Local.mk v Memory.bot) sc mem_tgt
+                  loc from to val releasedm released ord
+                  (Local.mk v' prom') sc' mem_tgt' kind)
+        (MEM: forget_memory others mem_src mem_tgt)
+        (OTHERS: ~ others loc to)
   :
     exists mem_src',
-      (<<STEP: (@pred_step (P /1\ write_in L /1\ no_promise) lang)
-                 e_tgt th_src
-                 (Thread.mk lang st' (Local.mk v' Memory.bot) sc' mem_src')>>) /\
-      (<<MEM: unchanged_on L mem_tgt' mem_src'>>).
-Proof.
-  dup MEM. inv MEM.
-  clarify. inv STEP. des. inv STEP0. inv STEP.
-  { inv STEP0. ss; clarify. }
-  inv STEP0. inv LOCAL; ss.
-  - exists mem_src. esplits; eauto. econs; eauto. econs; eauto.
-    econs 2; eauto. econs; eauto.
-  - inv LOCAL0. ss. clarify.
-    exists mem_src. esplits; eauto. econs; eauto. econs; eauto.
-    econs 2; eauto. econs; eauto.
-  - exploit unchanged_on_write; eauto. i. des. esplits; eauto.
-    econs; eauto. econs; eauto. econs 2; eauto. econs; eauto.
-  - inv LOCAL1. ss.
-    exploit unchanged_on_write; eauto. i. des. esplits; eauto.
-    econs; eauto. econs; eauto. econs 2; eauto. econs; eauto.
-  - inv LOCAL0. ss. clarify. exists mem_src. esplits; eauto.
-    econs; eauto. econs; eauto. econs 2; eauto. econs; eauto.
-  - inv LOCAL0. ss. clarify. exists mem_src. esplits; eauto.
-    econs; eauto. econs; eauto. econs 2; eauto. econs; eauto.
-Qed.
+      (<<WRITE: Local.write_step
+                  (Local.mk v Memory.bot) sc mem_src
+                  loc from to val releasedm released ord
+                  (Local.mk v' Memory.bot) sc' mem_src' Memory.op_kind_add>>) /\
+      (<<MEM: forget_memory others mem_src' mem_tgt'>>).
+  Proof.
+    exploit write_msg_wf; eauto. i. des.
+    inv WRITE. ss. clarify. exploit memory_write_bot_add; eauto. i. clarify.
+    dup WRITE0. inv WRITE0. inv PROMISE.
+    exploit write_succeed; eauto.
+    { instantiate (1:=mem_src). i. eapply forget_memory_le in MEM.
+      eapply memory_le_covered in COVER; eauto. ii.
+      exploit write_disjoint; try apply WRITE1; eauto.
+      { eapply Memory.bot_le. }
+      i. des; eauto. inv PROMISED.
+      erewrite Memory.bot_get in GET. clarify. }
+    i. des. exists mem2. econs; eauto.
+    inv MEM. inv WRITE. inv PROMISE. econs; i.
+    - erewrite (@Memory.add_o mem2); eauto.
+      erewrite (@Memory.add_o mem_tgt'); cycle 1; eauto. des_ifs. eauto.
+    - erewrite (@Memory.add_o mem2); eauto. des_ifs; eauto.
+      ss. des. clarify.
+  Qed.
 
-Definition cap (m mcap: Memory.t) (l: Loc.t) (t: Time.t): Prop :=
-  (<<NCOV: ~ covered l t m>>) /\ (<<CAP: ~ covered l t mcap>>).
+  Lemma other_promise_remove
+        P lang th_src th_tgt th_tgt' st st' v v' prom' sc sc'
+        mem_src mem_tgt mem_tgt' e_tgt others
+        (STEP: (@pred_step (P /1\ no_read_msgs others /1\ write_not_in others /1\ no_promise) lang) e_tgt th_tgt th_tgt')
+        (TH_SRC: th_src = Thread.mk lang st (Local.mk v Memory.bot) sc mem_src)
+        (TH_TGT0: th_tgt = Thread.mk lang st (Local.mk v Memory.bot) sc mem_tgt)
+        (TH_TGT1: th_tgt' = Thread.mk lang st' (Local.mk v' prom') sc' mem_tgt')
+        (MEM: forget_memory others mem_src mem_tgt)
+    :
+      exists mem_src',
+        (<<STEP: (@pred_step
+                    (P /1\ no_promise) lang)
+                   e_tgt th_src
+                   (Thread.mk lang st' (Local.mk v' Memory.bot) sc' mem_src')>>) /\
+        (<<MEM: forget_memory others mem_src' mem_tgt'>>).
+  Proof.
+    dup MEM. eapply forget_memory_le in MEM0.
+    clarify. inv STEP. des. inv STEP0. inv STEP.
+    { inv STEP0. ss; clarify. }
+    inv STEP0. inv LOCAL; ss.
+    - exists mem_src. esplits; eauto. econs; eauto. econs; eauto.
+      econs 2; eauto. econs; eauto.
+    - inv LOCAL0. ss. clarify.
+      exists mem_src. esplits; eauto. econs; eauto. econs; eauto.
+      econs 2; eauto. econs; eauto. econs; eauto. econs; eauto.
+      inv MEM. erewrite COMPLETE; eauto.
+    - ss. exploit other_promise_remove_write; eauto.
+      { exploit write_msg_wf; eauto. i. des.
+        eapply SAT1. econs; eauto. refl. }
+      i. des. exists mem_src'. esplits; eauto.
+      econs; eauto. econs; eauto. econs 2; eauto. econs; eauto.
+    - ss. inv LOCAL1. ss.
+      exploit other_promise_remove_write; eauto.
+      { exploit write_msg_wf; eauto. i. des.
+        eapply SAT1. econs; eauto. refl. }
+      i. des. exists mem_src'. esplits; eauto.
+      econs; eauto. econs; eauto. econs 2; eauto. econs; eauto.
+      econs; eauto. econs; eauto. inv MEM. erewrite COMPLETE; eauto.
+    - inv LOCAL0. ss. clarify. exists mem_src. esplits; eauto.
+      econs; eauto. econs; eauto. econs 2; eauto. econs; eauto.
+    - inv LOCAL0. ss. clarify. exists mem_src. esplits; eauto.
+      econs; eauto. econs; eauto. econs 2; eauto. econs; eauto.
+  Qed.
 
-Definition cap_write_with_update (CAP : Loc.t -> Time.t -> Prop)
-           (e : ThreadEvent.t) : Prop :=
-  match e with
-  | ThreadEvent.write loc from to _ _ _ =>
-    forall t (IN: Interval.mem (from, to) t), (~ CAP loc t)
-  | _ => True
-  end.
+End OTHERPROMISEREMOVE.
 
-Inductive capped (mem_src mem_tgt: Memory.t): Prop :=
-| capped_intro
-    (COVERLE: forall l t (COVER: covered l t mem_src), covered l t mem_tgt)
-    (MLE: forall loc to from val released
-                 (GET: Memory.get loc to mem_tgt = Some (from, Message.full val released)),
-        exists to_src from_src released_src,
-          (<<GET: Memory.get loc to_src mem_src =
-                  Some (from_src, Message.full val released_src)>>) /\
-          (<<EMPTY: forall l t (IN: Interval.mem (to_src, to) t), ~ covered l t mem_src>>) /\
-          (<<TOLE: Time.le to_src to>>) /\
-          (<<VIEWLE: View.opt_le released_src released>>))
-.
 
-Lemma list_filter_exists A (P: A -> Prop) (l: list A)
-  :
-    exists l',
-      (<<COMPLETE: forall a, ((<<IN: List.In a l>>) /\ (<<SAT: P a>>))
-                             <-> (<<IN: List.In a l'>>)>>).
-Proof.
-  induction l.
-  - exists []. ii. split; i; des.
-    + inv IN.
-    + inv H.
-  - des. destruct (classic (P a)).
-    + exists (a :: l'). split; i; ss; des; clarify; eauto.
-      * right. eapply COMPLETE; eauto.
-      * eapply COMPLETE in H0. des. eauto.
-    + exists l'. split; i; ss; des; clarify; eauto.
-      * eapply COMPLETE; eauto.
-      * eapply COMPLETE in H0. des; eauto.
-Qed.
 
-Lemma forget_exists_list l mem_tgt:
-  exists mem_src, <<FORGET: forget_memory (fun loc to => List.In (loc, to) l)
-                                                 mem_src mem_tgt>>.
-Proof.
-  induction l; ss.
-  - exists mem_tgt. econs; ss.
-  - i. destruct a as [loc to]. des.
-    destruct (Memory.get loc to mem_src) as [[from msg]|] eqn:GET.
-    + exploit Memory.remove_exists; eauto. i. des. exists mem2.
-      inv FORGET. econs; i.
-      * erewrite Memory.remove_o; eauto. des_ifs; eauto.
-        ss; des; clarify. exfalso. eauto.
-      * erewrite Memory.remove_o; eauto. des_ifs; clarify.
-        eapply FORGET0; eauto. ss. des; clarify; eauto.
-    + exists mem_src. inv FORGET.
-      econs; eauto. i. des; clarify; eauto.
-Qed.
+Section MAPPED.
 
-Lemma forget_exists P mem_tgt:
-  exists mem_src, <<FORGET: forget_memory P mem_src mem_tgt>>.
-Proof.
-  hexploit (Memory.finite_sound_exists mem_tgt); eauto. i. des.
-  hexploit (list_filter_exists (fun locto => P (fst locto) (snd locto)) dom). i. des.
-  hexploit (forget_exists_list l' mem_tgt). i. des.
-  exists mem_src. inv FORGET. econs; eauto.
-  - i. eapply COMPLETE0. ii. eapply COMPLETE in H1. des; eauto.
-  - i. destruct (classic (List.In (l, t) dom)).
-    + eapply FORGET0; eauto. eapply COMPLETE; eauto.
-    + rewrite COMPLETE0; eauto.
-      * destruct (Memory.get l t mem_tgt) as [[from msg]|] eqn:GET; auto.
-        exfalso. exploit H; eauto.
-      * ii. eapply COMPLETE in H2. des; clarify.
-Qed.
+  Inductive map_preserving (P: Loc.t -> Time.t -> Prop) (f: Loc.t -> Time.t -> Time.t) :=
+  | map_preserving_intro
+      (PRSVLT: forall loc t0 t1 (SAT0: P loc t0) (SAT1: P loc t1) (LT: Time.lt t0 t1),
+          Time.lt (f loc t0) (f loc t1))
+      (PRSVBOT: forall loc, f loc Time.bot = Time.bot)
+  .
 
-Lemma forget_unique P mem_tgt mem_src0 mem_src1
-      (FORGET0: forget_memory P mem_src0 mem_tgt)
-      (FORGET1: forget_memory P mem_src1 mem_tgt)
-  :
-    mem_src0 = mem_src1.
-Proof.
-  inv FORGET0. inv FORGET1.
-  eapply Memory.ext. i. destruct (classic (P loc ts)).
-  - erewrite FORGET; auto. erewrite FORGET0; auto.
-  - erewrite COMPLETE; auto. erewrite COMPLETE0; auto.
-Qed.
+  Definition map_preserving_lt_iff P f
+             (PRSV: map_preserving P f)
+             loc t0 t1
+             (SAT0: P loc t0) (SAT1: P loc t1)
+    :
+      Time.lt t0 t1 <-> Time.lt (f loc t0) (f loc t1).
+  Proof.
+    inv PRSV. split; eauto.
+    set (DenseOrder.DenseOrderFacts.OrderTac.TO.lt_total t0 t1). des; eauto.
+    - clarify. i. timetac.
+    - i. eapply PRSVLT in o; eauto. exfalso.
+      assert (LT: Time.lt (f loc t0) (f loc t0)).
+      + etrans; eauto.
+      + timetac.
+  Qed.
+  Hint Resolve map_preserving_lt_iff.
 
-Definition unchangables (mem prom: Memory.t) (l: Loc.t) (t: Time.t) :=
-  (<<COV: covered l t mem>>) /\
-  (<<NCOV: ~ covered l t prom>>).
+  Definition map_preserving_eq_iff P f
+             (PRSV: map_preserving P f)
+             loc t0 t1
+             (SAT0: P loc t0) (SAT1: P loc t1)
+    :
+      t0 = t1 <-> (f loc t0) = (f loc t1).
+  Proof.
+    split; i; clarify; eauto.
+    set (DenseOrder.DenseOrderFacts.OrderTac.TO.lt_total t0 t1). des; eauto.
+    - erewrite map_preserving_lt_iff in o; eauto.
+      rewrite H in *. timetac.
+    - erewrite map_preserving_lt_iff in o; eauto.
+      rewrite H in *. timetac.
+  Qed.
+  Hint Resolve map_preserving_eq_iff.
 
-Lemma step_wirte_not_in_write promises1 mem1 loc from1 to1 val released promises3 mem2 kind
-      (WRITE: Memory.write promises1 mem1 loc from1 to1 val released promises3 mem2 kind)
-      t
-      (IN: Interval.mem (from1, to1) t)
-  :
-    ~ unchangables mem1 promises1 loc t.
-Proof.
-  unfold unchangables. inv WRITE. apply or_not_and. inv PROMISE.
-  - left. ii. inv H. dup GET. eapply Memory.add_get1 in GET; eauto.
-    eapply Memory.add_get0 in MEM. des.
-    exploit Memory.get_disjoint.
-    + eapply GET.
-    + eapply GET2.
-    + i. des; clarify. eauto.
-  - right. eapply Memory.split_get0 in PROMISES. des. ii. apply H.
-    econs; eauto. inv IN. econs; ss; eauto. etrans; eauto.
-    inv MEM. inv SPLIT. left. eauto.
-  - right. eapply Memory.lower_get0 in PROMISES. des. ii. apply H.
+  Definition map_preserving_le_iff P f
+             (PRSV: map_preserving P f)
+             loc t0 t1
+             (SAT0: P loc t0) (SAT1: P loc t1)
+    :
+      Time.le t0 t1 <-> Time.le (f loc t0) (f loc t1).
+  Proof.
+    repeat rewrite DenseOrder.DenseOrder.le_lteq.
+    split; i; des; clarify; eauto.
+    - left. erewrite <- map_preserving_lt_iff; eauto.
+    - left. eapply map_preserving_lt_iff; eauto.
+    - right. eapply map_preserving_eq_iff; eauto.
+  Qed.
+  Hint Resolve map_preserving_le_iff.
+
+  Definition map_preserving_bot P f
+             (PRSV: map_preserving P f)
+             loc
+    :
+      f loc Time.bot = Time.bot.
+  Proof.
+    inv PRSV. eauto.
+  Qed.
+  Hint Resolve map_preserving_bot.
+
+  Definition timemap_map (f: Loc.t -> Time.t -> Time.t) (tm: TimeMap.t): TimeMap.t :=
+    fun l => f l (tm l).
+
+  Definition view_map (f: Loc.t -> Time.t -> Time.t) (v: View.t): View.t :=
+    View.mk (timemap_map f v.(View.pln)) (timemap_map f v.(View.rlx)).
+
+  Definition tview_map (f: Loc.t -> Time.t -> Time.t) (v: TView.t): TView.t :=
+    TView.mk
+      (fun loc => view_map f (v.(TView.rel) loc))
+      (view_map f v.(TView.cur))
+      (view_map f v.(TView.acq)).
+
+  Definition msg_map (f: Loc.t -> Time.t -> Time.t) (msg: Message.t): Message.t :=
+    match msg with
+    | Message.half => Message.half
+    | Message.full val released =>
+      Message.full val (option_map (view_map f) released)
+    end.
+
+  Definition tevent_map (f: Loc.t -> Time.t -> Time.t) (te: ThreadEvent.t): ThreadEvent.t :=
+    match te with
+    | ThreadEvent.promise loc from to msg kind =>
+      ThreadEvent.promise loc (f loc from) (f loc to) (msg_map f msg) kind
+    | ThreadEvent.read loc to val v o =>
+      ThreadEvent.read loc (f loc to) val (option_map (view_map f) v) o
+    | ThreadEvent.write loc to from val v o =>
+      ThreadEvent.write loc (f loc to) (f loc from) val (option_map (view_map f) v) o
+    | ThreadEvent.update loc to from valr valw vr vw or ow =>
+      ThreadEvent.update loc (f loc to) (f loc from) valr valw (option_map (view_map f) vr) (option_map (view_map f) vw) or ow
+    | ThreadEvent.fence or ow => ThreadEvent.fence or ow
+    | ThreadEvent.syscall e => ThreadEvent.syscall e
+    | _ => ThreadEvent.silent
+    end.
+
+  Inductive memory_map f m_src m_tgt: Prop :=
+  | memory_map_intro
+      (MAPPED: forall loc to from msg (GET: Memory.get loc to m_tgt = Some (from, msg)),
+          Memory.get loc (f loc to) m_src = Some (f loc from, msg_map f msg))
+      (ONLY: forall loc to_src msg_src (GET: Memory.get loc to_src m_src = Some msg_src),
+          exists to msg,
+            (<<FROM: f loc to = to_src>>) /\
+            (<<GET: Memory.get loc to m_tgt = Some msg>>))
+  .
+
+  Definition times_in_memory (m: Memory.t) (l: Loc.t) (t: Time.t): Prop :=
+    (<<OFFROM: exists to msg,
+        (<<GET: Memory.get l to m = Some (t, msg)>>)>>) \/
+    (<<OFTO: exists from msg,
+        (<<GET: Memory.get l t m = Some (from, msg)>>)>>)
+  .
+
+  Definition times_in_memory_to (m: Memory.t) (l: Loc.t) (t: Time.t): Prop :=
+    (<<OFTO: exists from val released,
+        (<<GET: Memory.get l t m = Some (from, Message.full val released)>>)>>)
+  .
+
+  Lemma times_in_memory_to_in_memory:
+    times_in_memory_to <3= times_in_memory.
+  Proof.
+    i. unfold times_in_memory_to in *. des. right. eauto.
+  Qed.
+  Hint Resolve times_in_memory_to_in_memory.
+
+  Lemma map_closed_timemap m f tm
+        (INMEMORY: map_preserving (times_in_memory m) f)
+        (CLOSED: Memory.closed_timemap tm m)
+    :
+      forall loc, times_in_memory m loc (tm loc).
+  Proof.
+    ii. right. specialize (CLOSED loc). unfold times_in_memory_to. des. eauto.
+  Qed.
+
+  Lemma map_time_join P f loc t0 t1
+        (PRSV: map_preserving P f)
+        (SAT0: P loc t0) (SAT1: P loc t1)
+    :
+      f loc (Time.join t0 t1) = Time.join (f loc t0) (f loc t1).
+  Proof.
+    unfold Time.join. des_ifs.
+    - erewrite <- map_preserving_lt_iff in l0; eauto.
+      erewrite <- map_preserving_eq_iff; eauto.
+      timetac.
+    - erewrite <- map_preserving_le_iff in l0; eauto.
+      erewrite <- map_preserving_eq_iff; eauto.
+      timetac.
+  Qed.
+
+  Lemma map_timemap_join f m tm0 tm1
+        (INMEMORY: map_preserving (times_in_memory m) f)
+        (CLOSED0: Memory.closed_timemap tm0 m)
+        (CLOSED1: Memory.closed_timemap tm1 m)
+    :
+      timemap_map f (TimeMap.join tm0 tm1) = TimeMap.join (timemap_map f tm0) (timemap_map f tm1).
+  Proof.
+    extensionality t. unfold timemap_map, TimeMap.join.
+    eapply map_time_join; eauto.
+    - eapply map_closed_timemap; eauto.
+    - eapply map_closed_timemap; eauto.
+  Qed.
+
+  Lemma map_viewjoin f m v0 v1
+        (INMEMORY: map_preserving (times_in_memory m) f)
+        (CLOSED0: Memory.closed_view v0 m)
+        (CLOSED1: Memory.closed_view v1 m)
+    :
+      view_map f (View.join v0 v1) = View.join (view_map f v0) (view_map f v1).
+  Proof.
+    inv CLOSED0. inv CLOSED1.
+    unfold view_map, View.join. ss. f_equal.
+    - eapply map_timemap_join; eauto.
+    - eapply map_timemap_join; eauto.
+  Qed.
+
+  Lemma map_tviewjoin f m tv0 tv1
+        (INMEMORY: map_preserving (times_in_memory m) f)
+        (CLOSED0: TView.closed tv0 m)
+        (CLOSED1: TView.closed tv1 m)
+    :
+      tview_map f (TView.join tv0 tv1) = TView.join (tview_map f tv0) (tview_map f tv1).
+  Proof.
+    inv CLOSED0. inv CLOSED1.
+    unfold tview_map, TView.join. ss. f_equal.
+    - extensionality l. eapply map_viewjoin; eauto.
+    - eapply map_viewjoin; eauto.
+    - eapply map_viewjoin; eauto.
+  Qed.
+
+  Lemma map_timemap_bot P f
+        (PRSV: map_preserving P f)
+    :
+      timemap_map f TimeMap.bot = TimeMap.bot.
+  Proof.
+    extensionality loc. unfold timemap_map.
+    erewrite map_preserving_bot; eauto.
+  Qed.
+
+  Lemma map_view_bot P f
+        (PRSV: map_preserving P f)
+    :
+      view_map f View.bot = View.bot.
+  Proof.
+    unfold view_map, View.bot. ss. f_equal.
+    - eapply map_timemap_bot; eauto.
+    - eapply map_timemap_bot; eauto.
+  Qed.
+
+  Lemma map_unwrap f m released
+        (INMEMORY: map_preserving (times_in_memory m) f)
+        (CLOSED0: Memory.closed_opt_view released m)
+    :
+      view_map f (View.unwrap released) =
+      View.unwrap (option_map (view_map f) released).
+  Proof.
+    unfold View.unwrap. des_ifs. eapply map_view_bot; eauto.
+  Qed.
+
+  Lemma map_timemap_singleton f P loc to
+        (INMEMORY: map_preserving P f)
+        (CLOSED2: P loc to)
+    :
+      timemap_map f (TimeMap.singleton loc to) =
+      TimeMap.singleton loc (f loc to).
+  Proof.
+    extensionality l.
+    unfold timemap_map, TimeMap.singleton.
+    setoid_rewrite LocFun.add_spec. des_ifs.
+    rewrite LocFun.init_spec. erewrite map_preserving_bot; eauto.
+  Qed.
+
+  Lemma map_singleton_ur f P loc to
+        (INMEMORY: map_preserving P f)
+        (CLOSED2: P loc to)
+    :
+      view_map f (View.singleton_ur loc to) =
+      View.singleton_ur loc (f loc to).
+  Proof.
+    unfold view_map, View.singleton_ur. ss.
+    erewrite map_timemap_singleton; eauto.
+  Qed.
+
+  Lemma map_singleton_rw f P loc to
+        (INMEMORY: map_preserving P f)
+        (CLOSED2: P loc to)
+    :
+      view_map f (View.singleton_rw loc to) =
+      View.singleton_rw loc (f loc to).
+  Proof.
+    unfold view_map, View.singleton_rw. ss.
+    erewrite map_timemap_singleton; eauto. f_equal.
+    eapply map_timemap_bot; eauto.
+  Qed.
+
+  Lemma map_singleton_ur_if f P loc to cond
+        (INMEMORY: map_preserving P f)
+        (CLOSED2: P loc to)
+    :
+      view_map f (View.singleton_ur_if cond loc to) =
+      View.singleton_ur_if cond loc (f loc to).
+  Proof.
+    unfold view_map, View.singleton_ur_if. des_ifs.
+    - erewrite <- map_singleton_ur; eauto.
+    - erewrite <- map_singleton_rw; eauto.
+  Qed.
+
+  Lemma map_read_tview f m v loc to released ord
+        (INMEMORY: map_preserving (times_in_memory m) f)
+        (CLOSED0: TView.closed v m)
+        (CLOSED1: Memory.closed_opt_view released m)
+        (CLOSED2: times_in_memory_to m loc to)
+        (INHABITED: Memory.inhabited m)
+    :
+      tview_map f (TView.read_tview v loc to released ord) =
+      TView.read_tview (tview_map f v) loc (f loc to) (option_map (view_map f) released) ord.
+  Proof.
+    unfold tview_map, TView.read_tview. ss.
+    repeat (erewrite <- map_unwrap; eauto).
+    repeat (erewrite map_viewjoin; eauto).
+    - erewrite map_singleton_ur_if; eauto.
+      des_ifs; f_equal; erewrite map_view_bot; eauto.
+    - inv CLOSED0. eauto.
+    - unfold times_in_memory_to in *. des.
+      eapply Memory.singleton_ur_if_closed_view; eauto.
+    - eapply Memory.join_closed_view; eauto.
+      + inv CLOSED0; eauto.
+      + unfold times_in_memory_to in *. des.
+        eapply Memory.singleton_ur_if_closed_view; eauto.
+    - des_ifs.
+      + eapply Memory.unwrap_closed_opt_view; eauto.
+      + eapply Memory.closed_view_bot; eauto.
+    - inv CLOSED0. eauto.
+    - unfold times_in_memory_to in *. des.
+      eapply Memory.singleton_ur_if_closed_view; eauto.
+    - eapply Memory.join_closed_view; eauto.
+      + inv CLOSED0; eauto.
+      + unfold times_in_memory_to in *. des.
+        eapply Memory.singleton_ur_if_closed_view; eauto.
+    - des_ifs.
+      + eapply Memory.unwrap_closed_opt_view; eauto.
+      + eapply Memory.closed_view_bot; eauto.
+  Qed.
+
+  Lemma map_step_read
+        f v v' prom'
+        mem_src mem_tgt loc to val released ord
+        (STEP: Local.read_step (Local.mk v Memory.bot) mem_tgt loc to val released ord
+                               (Local.mk v' prom'))
+        (INMEMORY0: map_preserving (times_in_memory mem_tgt) f)
+        (CLOSED0: Memory.closed mem_tgt)
+        (LCWF: Local.wf (Local.mk v Memory.bot) mem_tgt)
+        (MEM: memory_map f mem_src mem_tgt)
+        (INHABITED: Memory.inhabited mem_tgt)
+    :
+      (<<STEP: Local.read_step (Local.mk (tview_map f v) Memory.bot) mem_src loc
+                               (f loc to) val (option_map (view_map f) released) ord
+                               (Local.mk (tview_map f v') Memory.bot)>>).
+  Proof.
+    inv STEP. ss. clarify. econs; eauto.
+    + inv MEM. exploit MAPPED; eauto.
+    + ss. inv READABLE. unfold view_map, option_map, timemap_map. des_ifs.
+      * econs; ss; eauto.
+        { erewrite <- map_preserving_le_iff; eauto.
+          - inv LCWF. ss. inv TVIEW_CLOSED. inv CUR.
+            eapply map_closed_timemap; eauto.
+          - right. eauto. }
+        { i. erewrite <- map_preserving_le_iff; eauto.
+          - inv LCWF. ss. inv TVIEW_CLOSED. inv CUR.
+            eapply map_closed_timemap; eauto.
+          - right. eauto. }
+      * econs; ss; eauto.
+        { erewrite <- map_preserving_le_iff; eauto.
+          - inv LCWF. ss. inv TVIEW_CLOSED. inv CUR.
+            eapply map_closed_timemap; eauto.
+          - right. eauto. }
+        { i. erewrite <- map_preserving_le_iff; eauto.
+          - inv LCWF. ss. inv TVIEW_CLOSED. inv CUR.
+            eapply map_closed_timemap; eauto.
+          - right. eauto. }
+    + ss. f_equal. erewrite map_read_tview; eauto.
+      * inv LCWF. ss.
+      * eapply CLOSED0 in GET. des. inv MSG_CLOSED. eauto.
+      * unfold times_in_memory_to. eauto.
+  Qed.
+
+  Lemma view_map_le f m tm0 tm1
+        (INMEMORY: map_preserving (times_in_memory m) f)
+        (CLOSED0: Memory.closed_timemap tm0 m)
+        (CLOSED1: Memory.closed_timemap tm1 m)
+        (LE: TimeMap.le tm0 tm1)
+    :
+      TimeMap.le (timemap_map f tm0) (timemap_map f tm1).
+  Proof.
+    ii. unfold timemap_map.
+    erewrite <- map_preserving_le_iff; eauto.
+    - right. specialize (CLOSED0 loc). des. eauto.
+    - right. specialize (CLOSED1 loc). des. eauto.
+  Qed.
+
+  Lemma view_map_wf f m view
+        (INMEMORY: map_preserving (times_in_memory m) f)
+        (CLOSED0: Memory.closed_view view m)
+        (WF : View.wf view)
+    :
+      View.wf (view_map f view).
+  Proof.
+    unfold view_map. ss. econs. inv WF.
+    inv CLOSED0. eapply view_map_le in PLN_RLX; eauto.
+  Qed.
+
+  Lemma map_write_released f m v sc loc to releasedm ord
+        (INMEMORY0: map_preserving (times_in_memory m) f)
+        (INHABITED: Memory.inhabited m)
+        (CLOSED0: Memory.closed m)
+        (CLOSED1: Memory.closed_opt_view releasedm m)
+        (CLOSED2: times_in_memory_to m loc to)
+        (CLOSED3: TView.closed v m)
+        (CLOSED4: Memory.closed_timemap sc m)
+    :
+      option_map (view_map f) (TView.write_released v sc loc to releasedm ord) =
+      TView.write_released (tview_map f v) (timemap_map f sc) loc (f loc to)
+                           (option_map (view_map f) releasedm) ord.
+  Proof.
+    dup CLOSED2. unfold times_in_memory_to in CLOSED2. des.
+    exploit TViewFacts.get_closed_released; eauto.
+    instantiate (1:=ord). i.
+    unfold TView.write_released in *. des_ifs. unfold option_map.
+    erewrite map_viewjoin; eauto.
+    - f_equal. erewrite map_unwrap; eauto. f_equal.
+      setoid_rewrite LocFun.add_spec_eq.
+      des_ifs.
+      + erewrite map_viewjoin; eauto.
+        * erewrite map_singleton_ur; eauto.
+        * inv CLOSED3. eauto.
+        * unfold times_in_memory_to in *. des.
+          eapply Memory.singleton_ur_closed_view; eauto.
+      + erewrite map_viewjoin; eauto.
+        * erewrite map_singleton_ur; eauto.
+        * inv CLOSED3. eauto.
+        * unfold times_in_memory_to in *. des.
+          eapply Memory.singleton_ur_closed_view; eauto.
+    - eapply Memory.unwrap_closed_opt_view; eauto.
+    - exploit TViewFacts.get_closed_tview; eauto. i.
+      inv x1. eauto.
+  Qed.
+
+  Lemma map_write_tview f m v sc ord loc to
+        (INMEMORY: map_preserving (times_in_memory m) f)
+        (INHABITED: Memory.inhabited m)
+        (CLOSED0: TView.closed v m)
+        (CLOSED1: Memory.closed_timemap sc m)
+        (CLOSED2: times_in_memory_to m loc to)
+    :
+      tview_map f (TView.write_tview v sc loc to ord) =
+      TView.write_tview (tview_map f v) (timemap_map f sc) loc (f loc to) ord.
+  Proof.
+    unfold TView.write_tview. ss. unfold tview_map at 1. ss. f_equal.
+    - extensionality l. des_ifs.
+      + setoid_rewrite LocFun.add_spec. des_ifs.
+        erewrite map_viewjoin; eauto.
+        * f_equal. erewrite map_singleton_ur; eauto.
+        * inv CLOSED0. eauto.
+        * unfold times_in_memory_to in *. des.
+          eapply Memory.singleton_ur_closed_view; eauto.
+      + setoid_rewrite LocFun.add_spec. des_ifs.
+        erewrite map_viewjoin; eauto.
+        * f_equal. erewrite map_singleton_ur; eauto.
+        * inv CLOSED0. eauto.
+        * unfold times_in_memory_to in *. des.
+          eapply Memory.singleton_ur_closed_view; eauto.
+    - erewrite map_viewjoin; eauto.
+      + f_equal. erewrite map_singleton_ur; eauto.
+      + inv CLOSED0. eauto.
+      + unfold times_in_memory_to in *. des.
+        eapply Memory.singleton_ur_closed_view; eauto.
+    - erewrite map_viewjoin; eauto.
+      + f_equal. erewrite map_singleton_ur; eauto.
+      + inv CLOSED0. eauto.
+      + unfold times_in_memory_to in *. des.
+        eapply Memory.singleton_ur_closed_view; eauto.
+  Qed.
+
+  Lemma map_step_write f v v' prom'
+        loc from to val releasedm released ord sc sc' mem_src
+        mem_tgt mem_tgt' kind
+        (WRITE: Local.write_step
+                  (Local.mk v Memory.bot) sc mem_tgt
+                  loc from to val releasedm released ord
+                  (Local.mk v' prom') sc' mem_tgt' kind)
+        (INMEMORY0: map_preserving (times_in_memory mem_tgt) f)
+        (INMEMORY1: map_preserving (times_in_memory mem_tgt') f)
+        (CLOSED0: Memory.closed mem_tgt)
+        (CLOSED1: View.opt_wf releasedm)
+        (CLOSED2: Memory.closed_opt_view releasedm mem_tgt)
+        (CLOSED3: Memory.closed_timemap sc mem_tgt)
+        (LCWF: Local.wf (Local.mk v Memory.bot) mem_tgt)
+        (MEM: memory_map f mem_src mem_tgt)
+        (INHABITED: Memory.inhabited mem_tgt)
+    :
+      exists mem_src',
+        (<<WRITE: Local.write_step
+                    (Local.mk (tview_map f v) Memory.bot)
+                    (timemap_map f sc)
+                    mem_src loc (f loc from) (f loc to) val
+                    (option_map (view_map f) releasedm)
+                    (option_map (view_map f) released) ord
+                    (Local.mk (tview_map f v') Memory.bot)
+                    (timemap_map f sc') mem_src' Memory.op_kind_add>>) /\
+        (<<MEM: memory_map f mem_src' mem_tgt'>>).
+  Proof.
+    inv LCWF. exploit write_msg_wf; eauto. i. des.
+    dup WRITE. inv WRITE. ss. clarify. exploit memory_write_bot_add; eauto. i. clarify.
+    assert (CLOSEDV1: Memory.closed_opt_view (TView.write_released v sc loc to releasedm ord) mem_tgt').
+    { inv WRITE1. inv PROMISE. ss.
+      eapply TViewFacts.write_future; eauto. }
+    exploit Local.write_step_future; eauto. i. ss. des.
+    inv WRITE1. inv PROMISE. dup MEM0. eapply Memory.add_get0 in MEM1. des.
+    exploit write_succeed.
+    { instantiate (1:=f loc to). instantiate (1:=f loc from).
+      instantiate (1:=mem_src). instantiate (1:=loc).
+      ii. inv COVER.
+      inv MEM. ss. exploit ONLY; eauto. i. des. clarify.
+      destruct msg0. dup GET2. eapply MAPPED in GET2. clarify.
+      dup GET3. eapply Memory.add_get1 in GET3; eauto.
+      destruct H. destruct ITV. ss.
+      assert (LT0: Time.lt (f loc t0) (f loc to)).
+      { eapply DenseOrder.DenseOrderFacts.lt_le_lt; eauto. }
+      assert (LT1: Time.lt (f loc from) (f loc to1)).
+      { eapply DenseOrder.DenseOrderFacts.lt_le_lt; eauto. }
+      assert (LT2: Time.lt (f loc from) (f loc to)).
+      { eapply DenseOrder.DenseOrderFacts.lt_le_lt; try apply FROM; eauto. }
+      assert (LT3: Time.lt (f loc t0) (f loc to1)).
+      { eapply DenseOrder.DenseOrderFacts.lt_le_lt; try apply FROM0; eauto. }
+      erewrite <- map_preserving_lt_iff in LT0; eauto; cycle 1.
+      { left. eauto. }
+      { right. eauto. }
+      erewrite <- map_preserving_lt_iff in LT1; eauto; cycle 1.
+      { left. eauto. }
+      { right. eauto. }
+      erewrite <- map_preserving_lt_iff in LT2; eauto; cycle 1.
+      { left. eauto. }
+      { right. eauto. }
+      erewrite <- map_preserving_lt_iff in LT3; eauto; cycle 1.
+      { left. eauto. }
+      { right. eauto. }
+      exploit Memory.get_disjoint.
+      - eapply GET3.
+      - eapply GET0.
+      - i. des; clarify.
+        exploit Time.middle_spec.
+        { instantiate (1:=Time.meet to to1). instantiate (1:=Time.join from t0).
+          unfold Time.join, Time.meet. des_ifs. } i. des.
+        eapply x0.
+        + instantiate (1:=Time.middle (Time.join from t0) (Time.meet to to1)). econs; ss.
+          * eapply DenseOrder.DenseOrderFacts.le_lt_lt; eauto. eapply Time.join_r.
+          * left. eapply DenseOrder.DenseOrderFacts.lt_le_lt; eauto. eapply Time.meet_r.
+        + econs; ss.
+          * eapply DenseOrder.DenseOrderFacts.le_lt_lt; eauto. eapply Time.join_l.
+          * left. eapply DenseOrder.DenseOrderFacts.lt_le_lt; eauto. eapply Time.meet_l. }
+    { instantiate (1:=option_map
+                        (view_map f)
+                        (TView.write_released v sc loc to releasedm ord)).
+      erewrite map_preserving_le_iff in REL_TS; try apply INMEMORY1; eauto.
+      - instantiate (1:=loc) in REL_TS.
+        setoid_rewrite <- map_unwrap; try apply INMEMORY1; eauto.
+      - right. eapply Memory.unwrap_closed_opt_view in CLOSEDV1; eauto.
+        + inv CLOSEDV1. specialize (RLX loc). des. eauto.
+        + eapply inhabited_future; eauto.
+      - right. eauto. }
+    { erewrite <- map_preserving_lt_iff; eauto.
+      - left. eauto.
+      - right. eauto. }
+    { econs. inv REL_WF; ss. econs. eapply view_map_wf; try apply INMEMORY1; eauto.
+      inv CLOSEDV1; congruence. }
+    i. des. exists mem2. esplits; eauto.
+    - econs; ss; eauto.
+      + erewrite map_write_released; try apply INMEMORY1; eauto.
+        * eapply inhabited_future; eauto.
+        * eapply Memory.future_closed_opt_view; eauto.
+        * unfold times_in_memory_to. eauto.
+        * eapply TView.future_closed; eauto.
+      + inv WRITABLE. econs. unfold view_map, timemap_map. ss.
+        erewrite <- map_preserving_lt_iff; eauto.
+        * eapply TView.future_closed in TVIEW_CLOSED; eauto.
+          inv TVIEW_CLOSED. inv CUR. specialize (RLX loc). des.
+          unfold times_in_memory. eauto.
+        * unfold times_in_memory. eauto.
+      + f_equal. eapply map_write_tview; eauto.
+        * eapply inhabited_future; eauto.
+        * eapply TView.future_closed; eauto.
+        * unfold times_in_memory_to. eauto.
+    - inv WRITE. inv PROMISE. econs.
+      + i. erewrite Memory.add_o in GET1; eauto.
+        erewrite Memory.add_o; eauto. des_ifs; ss.
+        * des; clarify.
+        * des; clarify. exfalso.
+          erewrite <- map_preserving_eq_iff in a0; eauto.
+          { right. eapply Memory.add_get1 in GET1; eauto. }
+          { right. eauto. }
+        * des; clarify.
+        * inv MEM. eauto.
+      + i. erewrite Memory.add_o in GET1; eauto. des_ifs.
+        * ss; des; clarify. esplits; eauto.
+        * inv MEM. exploit ONLY; eauto. i.
+          destruct x as [to0 [msg [FROM GET2]]].
+          exists to0, msg. esplits; eauto.
+          erewrite Memory.add_o; eauto. des_ifs.
+          ss. des; clarify.
+  Qed.
+
+  Lemma map_read_fence_tview f v ord
+    :
+      tview_map f (TView.read_fence_tview v ord) =
+      TView.read_fence_tview (tview_map f v) ord.
+  Proof.
+    unfold TView.read_fence_tview, tview_map. ss. f_equal.
+    des_ifs.
+  Qed.
+
+  Lemma map_write_fence_sc f m v sc ord
+        (INMEMORY: map_preserving (times_in_memory m) f)
+        (CLOSED0: TView.closed v m)
+        (CLOSED1: Memory.closed_timemap sc m)
+    :
+      timemap_map f (TView.write_fence_sc v sc ord) =
+      TView.write_fence_sc (tview_map f v) (timemap_map f sc) ord.
+  Proof.
+    unfold TView.write_fence_sc. ss.
+    extensionality loc. des_ifs.
+    erewrite map_timemap_join; eauto.
+    inv CLOSED0. inv CUR. eauto.
+  Qed.
+
+  Lemma map_read_fence f v ord
+    :
+      tview_map f (TView.read_fence_tview v ord) =
+      TView.read_fence_tview (tview_map f v) ord.
+  Proof.
+    unfold TView.read_fence_tview, tview_map. ss. f_equal. des_ifs.
+  Qed.
+
+  Lemma write_fence_sc_closed v sc ord m
+        (CLOSED0: TView.closed v m)
+        (CLOSED1: Memory.closed_timemap sc m)
+    :
+      Memory.closed_timemap (TView.write_fence_sc v sc ord) m.
+  Proof.
+    unfold TView.write_fence_sc. des_ifs.
+    eapply Memory.join_closed_timemap; eauto.
+    inv CLOSED0. inv CUR. auto.
+  Qed.
+
+  Lemma read_fence_closed tview ord m
+        (CLOSED0: TView.closed tview m)
+    :
+      TView.closed (TView.read_fence_tview tview ord) m.
+  Proof.
+    unfold TView.read_fence_tview. inv CLOSED0. des_ifs.
+  Qed.
+
+  Lemma map_write_fence_tview f m v sc ord
+        (INMEMORY: map_preserving (times_in_memory m) f)
+        (CLOSED0: TView.closed v m)
+        (CLOSED1: Memory.closed_timemap sc m)
+        (INHABITED: Memory.inhabited m)
+    :
+      tview_map f (TView.write_fence_tview v sc ord) =
+      TView.write_fence_tview (tview_map f v) (timemap_map f sc) ord.
+  Proof.
+    unfold TView.write_fence_tview. ss.
+    erewrite <- map_write_fence_sc; eauto.
+    unfold tview_map at 1. ss. f_equal.
+    - extensionality loc. des_ifs.
+    - des_ifs.
+    - erewrite map_viewjoin; eauto.
+      + des_ifs. erewrite map_view_bot; eauto.
+      + inv CLOSED0. inv ACQ. auto.
+      + des_ifs.
+        * econs; ss; eapply write_fence_sc_closed; eauto.
+        * eapply Memory.closed_view_bot; eauto.
+  Qed.
+
+  Lemma map_step
+        f lang th_src th_tgt th_tgt' st st' v v' prom' sc sc'
+        mem_src mem_tgt mem_tgt' e_tgt
+        (STEP: (@pred_step no_promise lang) e_tgt th_tgt th_tgt')
+        (TH_SRC: th_src = Thread.mk lang st (Local.mk (tview_map f v) Memory.bot)
+                                    (timemap_map f sc) mem_src)
+        (TH_TGT0: th_tgt = Thread.mk lang st (Local.mk v Memory.bot) sc mem_tgt)
+        (TH_TGT1: th_tgt' = Thread.mk lang st' (Local.mk v' prom') sc' mem_tgt')
+        (INMEMORY0: map_preserving (times_in_memory mem_tgt) f)
+        (INMEMORY1: map_preserving (times_in_memory mem_tgt') f)
+        (CLOSEDMAP0: Memory.closed_timemap sc mem_tgt)
+        (CLOSED0: Memory.closed mem_tgt)
+        (LCWF: Local.wf (Local.mk v Memory.bot) mem_tgt)
+        (INHABITED: Memory.inhabited mem_tgt)
+        (MEM: memory_map f mem_src mem_tgt)
+    :
+      exists mem_src',
+        (<<STEP: (@pred_step no_promise lang)
+                   (tevent_map f e_tgt) th_src
+                   (Thread.mk lang st' (Local.mk (tview_map f v') Memory.bot) (timemap_map f sc') mem_src')>>) /\
+        (<<MEM: memory_map f mem_src' mem_tgt'>>).
+  Proof.
+    clarify. inv STEP. inv STEP0. inv STEP; inv STEP0; ss. inv LOCAL; ss.
+    - exists mem_src. esplits; ss; eauto.
+      econs; eauto. econs; eauto. econs 2; eauto. econs; eauto.
+    - exploit map_step_read; eauto. i. des.
+      exists mem_src. esplits; eauto. econs; eauto. econs; eauto.
+      econs 2; eauto. econs; eauto.
+    - exploit map_step_write; eauto. i. des. ss.
+      exists mem_src'. esplits; eauto. econs; eauto. econs; eauto.
+      econs 2; eauto. econs; eauto.
+    - exploit Local.read_step_future; eauto. i. des.
+      destruct lc2. exploit map_step_read; eauto. i. des.
+      inv LOCAL1. ss. clarify.
+      exploit map_step_write; eauto. i. des.
+      exists mem_src'. esplits; eauto. econs; eauto. econs; eauto.
+      econs 2; eauto. econs; eauto.
+    - exists mem_src. esplits; eauto. econs; eauto. econs; eauto.
+      econs 2; eauto. econs; eauto. econs; eauto.
+      inv LOCAL0. ss. clarify.
+      erewrite map_write_fence_tview; eauto; cycle 1.
+      { eapply read_fence_closed; eauto. inv LCWF. eauto. }
+      repeat erewrite map_read_fence. econs; ss; eauto.
+      erewrite map_write_fence_sc; eauto.
+      + erewrite map_read_fence. auto.
+      + eapply read_fence_closed; eauto. inv LCWF. eauto.
+    - exists mem_src. esplits; eauto. econs; eauto. econs; eauto.
+      econs 2; eauto. econs; eauto. econs; eauto.
+      inv LOCAL0. ss. clarify.
+      erewrite map_write_fence_tview; eauto; cycle 1.
+      { eapply read_fence_closed; eauto. inv LCWF. eauto. }
+      repeat erewrite map_read_fence. econs; ss; eauto.
+      erewrite map_write_fence_sc; eauto.
+      eapply read_fence_closed; eauto. inv LCWF. eauto.
+  Qed.
+
+End MAPPED.
+
+
+
+
+Section UNCHANGEDON.
+
+  Inductive unchanged_on (P: Loc.t -> Time.t -> Prop) m0 m1 : Prop :=
+  | unchanged_on_intro
+      (NCOV: forall l t (IN: P l t) (COV: covered l t m1), covered l t m0)
+      (FUTURE : Memory.le m0 m1)
+  .
+  Global Program Instance le_PreOrder P: PreOrder (unchanged_on P).
+  Next Obligation. ii. econs; eauto. refl. Qed.
+  Next Obligation. ii. inv H. inv H0. econs; eauto. etrans; eauto. Qed.
+
+  Lemma unchanged_on_mon L0 L1
+        m0 m1
+        (NOTIN: unchanged_on L1 m0 m1)
+        (LE: L0 <2= L1)
+    :
+      unchanged_on L0 m0 m1.
+  Proof.
+    inv NOTIN. econs; eauto.
+  Qed.
+
+  Lemma unchanged_on_write v v' prom'
+        L loc from to val releasedm released ord sc sc' mem_src
+        mem_tgt mem_tgt' kind
+        (WRITE: Local.write_step
+                  (Local.mk v Memory.bot) sc mem_tgt
+                  loc from to val releasedm released ord
+                  (Local.mk v' prom') sc' mem_tgt' kind)
+        (MEM: unchanged_on L mem_tgt mem_src)
+        (WRITEIN: forall t (IN: Interval.mem (from, to) t), (L loc t))
+    :
+      exists mem_src',
+        (<<WRITE: Local.write_step
+                    (Local.mk v Memory.bot) sc mem_src
+                    loc from to val releasedm released ord
+                    (Local.mk v' Memory.bot) sc' mem_src' Memory.op_kind_add>>) /\
+        (<<MEM: unchanged_on L mem_tgt' mem_src'>>).
+  Proof.
+    inv MEM. inv WRITE. ss. clarify. exploit memory_write_bot_add; eauto. i. clarify.
+    exploit write_msg_wf; eauto. i. des.
+    inv WRITE0. inv PROMISE. dup MEM. eapply Memory.add_get0 in MEM; eauto. des.
+    exploit write_succeed; eauto.
+    { instantiate (1:=mem_src). ii.
+      exploit NCOV; eauto. intros COV. inv COV.
+      exploit Memory.get_disjoint.
+      - eapply GET0.
+      - eapply Memory.add_get1; eauto.
+      - i. des; clarify. eauto. }
+    i. des.
+    exists mem2. esplits; eauto.
+    inv WRITE. inv PROMISE.
     econs; eauto.
-Qed.
+    - ii. inv COV. erewrite Memory.add_o in GET1; cycle 1; eauto. des_ifs.
+      + ss. des. clarify. econs; eauto.
+      + exploit NCOV; eauto.
+        * econs; eauto.
+        * i. inv x. econs; eauto. eapply Memory.add_get1; eauto.
+    - ii. erewrite Memory.add_o; eauto.
+      erewrite Memory.add_o in LHS; cycle 1; eauto. des_ifs.
+      eapply FUTURE; eauto.
+  Qed.
 
-Lemma step_wirte_not_in lang (th_tgt th_tgt': Thread.t lang) e_tgt pf
-      (STEP: Thread.step pf e_tgt th_tgt th_tgt')
-  :
-    write_not_in (unchangables th_tgt.(Thread.memory) th_tgt.(Thread.local).(Local.promises))
-                 e_tgt.
-Proof.
-  unfold unchangables. inv STEP.
-  - inv STEP0; ss.
-  - inv STEP0; ss. inv LOCAL; ss.
-    + inv LOCAL0. ii. exploit step_wirte_not_in_write; eauto.
-    + inv LOCAL1. inv LOCAL2. ss. ii. exploit step_wirte_not_in_write; eauto.
-Qed.
+  Lemma unchanged_on_step
+        P L lang th_src th_tgt th_tgt' st st' v v' prom' sc sc'
+        mem_src mem_tgt mem_tgt' e_tgt
+        (STEP: (@pred_step (P /1\ write_in L /1\ no_promise) lang) e_tgt th_tgt th_tgt')
+        (TH_SRC: th_src = Thread.mk lang st (Local.mk v Memory.bot) sc mem_src)
+        (TH_TGT0: th_tgt = Thread.mk lang st (Local.mk v Memory.bot) sc mem_tgt)
+        (TH_TGT1: th_tgt' = Thread.mk lang st' (Local.mk v' prom') sc' mem_tgt')
+        (MEM: unchanged_on L mem_tgt mem_src)
+    :
+      exists mem_src',
+        (<<STEP: (@pred_step (P /1\ write_in L /1\ no_promise) lang)
+                   e_tgt th_src
+                   (Thread.mk lang st' (Local.mk v' Memory.bot) sc' mem_src')>>) /\
+        (<<MEM: unchanged_on L mem_tgt' mem_src'>>).
+  Proof.
+    dup MEM. inv MEM.
+    clarify. inv STEP. des. inv STEP0. inv STEP.
+    { inv STEP0. ss; clarify. }
+    inv STEP0. inv LOCAL; ss.
+    - exists mem_src. esplits; eauto. econs; eauto. econs; eauto.
+      econs 2; eauto. econs; eauto.
+    - inv LOCAL0. ss. clarify.
+      exists mem_src. esplits; eauto. econs; eauto. econs; eauto.
+      econs 2; eauto. econs; eauto.
+    - exploit unchanged_on_write; eauto. i. des. esplits; eauto.
+      econs; eauto. econs; eauto. econs 2; eauto. econs; eauto.
+    - inv LOCAL1. ss.
+      exploit unchanged_on_write; eauto. i. des. esplits; eauto.
+      econs; eauto. econs; eauto. econs 2; eauto. econs; eauto.
+    - inv LOCAL0. ss. clarify. exists mem_src. esplits; eauto.
+      econs; eauto. econs; eauto. econs 2; eauto. econs; eauto.
+    - inv LOCAL0. ss. clarify. exists mem_src. esplits; eauto.
+      econs; eauto. econs; eauto. econs 2; eauto. econs; eauto.
+  Qed.
 
-Lemma unchangables_promise mem0 prom0 loc from to msg prom1 mem1 kind
-      (PROMISE: Memory.promise prom0 mem0 loc from to msg prom1 mem1 kind)
-  :
-    unchangables mem0 prom0 <2= unchangables mem1 prom1.
-Proof.
-  unfold unchangables. inv PROMISE.
-  - ii. des. econs.
-    + red. erewrite add_covered; eauto.
-    + red. erewrite add_covered; eauto.
-      ii. des; clarify. dup MEM. eapply Memory.add_get0 in MEM. des.
-      inv COV. exfalso. exploit Memory.get_disjoint.
-      { eapply GET0. }
-      { eapply Memory.add_get1; eauto. }
-      i. des; clarify. eapply x0; eauto.
-  - ii. des. econs.
-    + red. erewrite split_covered; eauto.
-    + red. erewrite split_covered; eauto.
-  - ii. des. econs.
-    + red. erewrite lower_covered; eauto.
-    + red. erewrite lower_covered; eauto.
-Qed.
+  Lemma write_not_in_unchanged_on_write L v v' prom'
+        loc from to val releasedm released ord sc sc'
+        mem_tgt mem_tgt' kind
+        (WRITE: Local.write_step
+                  (Local.mk v Memory.bot) sc mem_tgt
+                  loc from to val releasedm released ord
+                  (Local.mk v' prom') sc' mem_tgt' kind)
+        (NOTIN: forall t (IN: Interval.mem (from, to) t), ~ (L loc t))
+    :
+      unchanged_on L mem_tgt mem_tgt'.
+  Proof.
+    inv WRITE. ss. clarify.
+    exploit memory_write_bot_add; eauto. i. clarify.
+    inv WRITE0. inv PROMISE. econs.
+    - i. rewrite add_covered in COV; eauto. des; auto.
+      clarify. exfalso. eapply NOTIN; eauto.
+    - ii. eapply Memory.add_get1; eauto.
+  Qed.
 
-Lemma other_promise_unchangable c tid1 tid2 st1 st2 lc1 lc2
-      (CWF: Configuration.wf c)
-      (TID1: IdentMap.find tid1 c.(Configuration.threads) = Some (st1, lc1))
-      (TID2: IdentMap.find tid2 c.(Configuration.threads) = Some (st2, lc2))
-      (DIFF: tid1 <> tid2)
-      l t
-      (COV: covered l t lc2.(Local.promises))
-  :
-    unchangables c.(Configuration.memory) lc1.(Local.promises) l t.
-Proof.
-  inv CWF. inv WF. inv COV. destruct st1, st2. econs; eauto.
-  - exploit THREADS; try apply TID2; eauto. intros LCWF. inv LCWF.
-    econs; eauto.
-  - ii. inv H. exploit DISJOINT; eauto. intros LCDISJ. inv LCDISJ.
-    inv DISJOINT0. exploit DISJOINT1; eauto. i. des.
-    eapply x1; eauto.
-Qed.
+  Lemma write_not_in_unchanged_on P L e lang (th0 th1: Thread.t lang)
+        (STEP: pred_step (P /1\ write_not_in L /1\ no_promise) e th0 th1)
+        (BOT: th0.(Thread.local).(Local.promises) = Memory.bot)
+    :
+      unchanged_on L th0.(Thread.memory) th1.(Thread.memory).
+  Proof.
+    inv STEP. inv STEP0. inv STEP.
+    - inv STEP0; ss; des; clarify.
+    - des. inv STEP0. ss. inv LOCAL; try refl.
+      + destruct lc1, lc2. ss. clarify. exploit write_not_in_unchanged_on_write; eauto.
+      + inv LOCAL1. ss.
+        destruct lc1, lc2. ss. clarify. exploit write_not_in_unchanged_on_write; eauto.
+  Qed.
 
-Lemma unchangables_remove mem prom0 loc from to msg prom1
-      (PROMISE: Memory.remove prom0 loc from to msg prom1)
-  :
-    unchangables mem prom0 <2= unchangables mem prom1.
-Proof.
-  unfold unchangables. ii. des. econs; eauto.
-  ii. eapply NCOV. inv H. erewrite Memory.remove_o in GET; eauto.
-  des_ifs. econs; eauto.
-Qed.
+End UNCHANGEDON.
 
-Lemma unchangables_increase pf e lang (th0 th1: Thread.t lang)
-      (STEP: Thread.step pf e th0 th1)
-  :
-    unchangables th0.(Thread.memory) th0.(Thread.local).(Local.promises) <2=
-    unchangables th1.(Thread.memory) th1.(Thread.local).(Local.promises).
-Proof.
-  inv STEP.
-  - inv STEP0; ss. inv LOCAL. i.
-    hexploit unchangables_promise; eauto.
-  - i. inv STEP0; ss. inv LOCAL; try inv LOCAL0; ss.
-    + inv WRITE. exploit unchangables_promise; eauto.
-      eapply unchangables_remove; eauto.
-    + inv LOCAL1. inv LOCAL2. ss. inv WRITE.
-      exploit unchangables_promise; eauto.
-      eapply unchangables_remove; eauto.
-Qed.
 
-Lemma write_not_in_unchanged_on_write L v v' prom'
-      loc from to val releasedm released ord sc sc'
-      mem_tgt mem_tgt' kind
-      (WRITE: Local.write_step
-                (Local.mk v Memory.bot) sc mem_tgt
-                loc from to val releasedm released ord
-                (Local.mk v' prom') sc' mem_tgt' kind)
-      (NOTIN: forall t (IN: Interval.mem (from, to) t), ~ (L loc t))
-  :
-    unchanged_on L mem_tgt mem_tgt'.
-Proof.
-  inv WRITE. ss. clarify.
-  exploit memory_write_bot_add; eauto. i. clarify.
-  inv WRITE0. inv PROMISE. econs.
-  - i. rewrite add_covered in COV; eauto. des; auto.
-    clarify. exfalso. eapply NOTIN; eauto.
-  - ii. eapply Memory.add_get1; eauto.
-Qed.
+Section UNCHANGAGBLES.
 
-Lemma write_not_in_unchanged_on P L e lang (th0 th1: Thread.t lang)
-      (STEP: pred_step (P /1\ write_not_in L /1\ no_promise) e th0 th1)
-      (BOT: th0.(Thread.local).(Local.promises) = Memory.bot)
-  :
-    unchanged_on L th0.(Thread.memory) th1.(Thread.memory).
-Proof.
-  inv STEP. inv STEP0. inv STEP.
-  - inv STEP0; ss; des; clarify.
-  - des. inv STEP0. ss. inv LOCAL; try refl.
-    + destruct lc1, lc2. ss. clarify. exploit write_not_in_unchanged_on_write; eauto.
-    + inv LOCAL1. ss.
-      destruct lc1, lc2. ss. clarify. exploit write_not_in_unchanged_on_write; eauto.
-Qed.
+  Definition unchangables (mem prom: Memory.t) (l: Loc.t) (t: Time.t) :=
+    (<<COV: covered l t mem>>) /\
+    (<<NCOV: ~ covered l t prom>>).
 
-Lemma no_sc_any_sc
-      P lang th_src th_tgt th_tgt' st st' v v' prom prom' sc sc_src sc'
-      mem mem' e
-      (STEP: (@pred_step (P /1\ no_sc) lang) e th_tgt th_tgt')
-      (TH_SRC: th_src = Thread.mk lang st (Local.mk v prom) sc_src mem)
-      (TH_TGT0: th_tgt = Thread.mk lang st (Local.mk v prom) sc mem)
-      (TH_TGT1: th_tgt' = Thread.mk lang st' (Local.mk v' prom') sc' mem')
+  Lemma step_wirte_not_in_write promises1 mem1 loc from1 to1 val released promises3 mem2 kind
+        (WRITE: Memory.write promises1 mem1 loc from1 to1 val released promises3 mem2 kind)
+        t
+        (IN: Interval.mem (from1, to1) t)
+    :
+      ~ unchangables mem1 promises1 loc t.
+  Proof.
+    unfold unchangables. inv WRITE. apply or_not_and. inv PROMISE.
+    - left. ii. inv H. dup GET. eapply Memory.add_get1 in GET; eauto.
+      eapply Memory.add_get0 in MEM. des.
+      exploit Memory.get_disjoint.
+      + eapply GET.
+      + eapply GET2.
+      + i. des; clarify. eauto.
+    - right. eapply Memory.split_get0 in PROMISES. des. ii. apply H.
+      econs; eauto. inv IN. econs; ss; eauto. etrans; eauto.
+      inv MEM. inv SPLIT. left. eauto.
+    - right. eapply Memory.lower_get0 in PROMISES. des. ii. apply H.
+      econs; eauto.
+  Qed.
+
+  Lemma step_wirte_not_in lang (th_tgt th_tgt': Thread.t lang) e_tgt pf
+        (STEP: Thread.step pf e_tgt th_tgt th_tgt')
+    :
+      write_not_in (unchangables th_tgt.(Thread.memory) th_tgt.(Thread.local).(Local.promises))
+                   e_tgt.
+  Proof.
+    unfold unchangables. inv STEP.
+    - inv STEP0; ss.
+    - inv STEP0; ss. inv LOCAL; ss.
+      + inv LOCAL0. ii. exploit step_wirte_not_in_write; eauto.
+      + inv LOCAL1. inv LOCAL2. ss. ii. exploit step_wirte_not_in_write; eauto.
+  Qed.
+
+  Lemma unchangables_promise mem0 prom0 loc from to msg prom1 mem1 kind
+        (PROMISE: Memory.promise prom0 mem0 loc from to msg prom1 mem1 kind)
+    :
+      unchangables mem0 prom0 <2= unchangables mem1 prom1.
+  Proof.
+    unfold unchangables. inv PROMISE.
+    - ii. des. econs.
+      + red. erewrite add_covered; eauto.
+      + red. erewrite add_covered; eauto.
+        ii. des; clarify. dup MEM. eapply Memory.add_get0 in MEM. des.
+        inv COV. exfalso. exploit Memory.get_disjoint.
+        { eapply GET0. }
+        { eapply Memory.add_get1; eauto. }
+        i. des; clarify. eapply x0; eauto.
+    - ii. des. econs.
+      + red. erewrite split_covered; eauto.
+      + red. erewrite split_covered; eauto.
+    - ii. des. econs.
+      + red. erewrite lower_covered; eauto.
+      + red. erewrite lower_covered; eauto.
+  Qed.
+
+  Lemma other_promise_unchangable c tid1 tid2 st1 st2 lc1 lc2
+        (CWF: Configuration.wf c)
+        (TID1: IdentMap.find tid1 c.(Configuration.threads) = Some (st1, lc1))
+        (TID2: IdentMap.find tid2 c.(Configuration.threads) = Some (st2, lc2))
+        (DIFF: tid1 <> tid2)
+        l t
+        (COV: covered l t lc2.(Local.promises))
+    :
+      unchangables c.(Configuration.memory) lc1.(Local.promises) l t.
+  Proof.
+    inv CWF. inv WF. inv COV. destruct st1, st2. econs; eauto.
+    - exploit THREADS; try apply TID2; eauto. intros LCWF. inv LCWF.
+      econs; eauto.
+    - ii. inv H. exploit DISJOINT; eauto. intros LCDISJ. inv LCDISJ.
+      inv DISJOINT0. exploit DISJOINT1; eauto. i. des.
+      eapply x1; eauto.
+  Qed.
+
+  Lemma unchangables_remove mem prom0 loc from to msg prom1
+        (PROMISE: Memory.remove prom0 loc from to msg prom1)
+    :
+      unchangables mem prom0 <2= unchangables mem prom1.
+  Proof.
+    unfold unchangables. ii. des. econs; eauto.
+    ii. eapply NCOV. inv H. erewrite Memory.remove_o in GET; eauto.
+    des_ifs. econs; eauto.
+  Qed.
+
+  Lemma unchangables_increase pf e lang (th0 th1: Thread.t lang)
+        (STEP: Thread.step pf e th0 th1)
+    :
+      unchangables th0.(Thread.memory) th0.(Thread.local).(Local.promises) <2=
+      unchangables th1.(Thread.memory) th1.(Thread.local).(Local.promises).
+  Proof.
+    inv STEP.
+    - inv STEP0; ss. inv LOCAL. i.
+      hexploit unchangables_promise; eauto.
+    - i. inv STEP0; ss. inv LOCAL; try inv LOCAL0; ss.
+      + inv WRITE. exploit unchangables_promise; eauto.
+        eapply unchangables_remove; eauto.
+      + inv LOCAL1. inv LOCAL2. ss. inv WRITE.
+        exploit unchangables_promise; eauto.
+        eapply unchangables_remove; eauto.
+  Qed.
+
+End UNCHANGAGBLES.
+
+
+Section SHORTERMEMORY.
+
+  Inductive shorter_memory (mem_src mem_tgt: Memory.t): Prop :=
+  | shorter_memory_intro
+      (COMPLETE: forall loc to from_tgt msg
+                        (GET: Memory.get loc to mem_tgt = Some (from_tgt, msg)),
+          exists from_src,
+            (<<GET: Memory.get loc to mem_src = Some (from_src, msg)>>))
+      (COVER: forall l t (COV: covered l t mem_src), covered l t mem_tgt)
+  .
+  Global Program Instance shorter_memory_PreOrder: PreOrder shorter_memory.
+  Next Obligation. ii. econs; eauto. Qed.
+  Next Obligation.
+    ii. inv H. inv H0. econs; eauto.
+    ii. exploit COMPLETE0; eauto. i. des.
+    exploit COMPLETE; eauto.
+  Qed.
+
+  (* TODO: make threadevent le and force eventpredicate is closed under that? *)
+  Lemma shorter_memory_write prom mem_src mem_tgt loc from1 to1 val released mem_tgt' from'
+        (SHORTER: shorter_memory mem_src mem_tgt)
+        (ADD: Memory.write Memory.bot mem_tgt loc from1 to1 val released prom mem_tgt' Memory.op_kind_add)
+        (TO: Time.le from1 from')
+        (FROM: Time.lt from' to1)
+    :
+      exists mem_src',
+        (<<ADD: Memory.write Memory.bot mem_src loc from' to1 val released prom mem_src' Memory.op_kind_add>>) /\
+        (<<SHORTER: shorter_memory mem_src' mem_tgt'>>).
+  Proof.
+    dup SHORTER. inv SHORTER. inv ADD. inv PROMISE.
+    exploit MemoryFacts.MemoryFacts.add_remove_eq; try apply REMOVE; eauto. i. clarify.
+    exploit write_succeed; eauto.
+    - instantiate (1:=mem_src). instantiate (1:=loc).
+      ii. eapply COVER in COVER0. inv COVER0.
+      dup MEM. eapply Memory.add_get0 in MEM. des.
+      dup GET. eapply Memory.add_get1 in GET; eauto.
+      exploit Memory.get_disjoint.
+      + eapply GET.
+      + eapply GET1.
+      + i. des; clarify.
+        eapply x0; eauto. inv H. econs; ss; eauto.
+        eapply TimeFacts.le_lt_lt; eauto.
+    - inv MEM. inv ADD. inv MSG_WF. inv TS. eauto.
+    - inv MEM. inv ADD. eauto.
+    - i. des. inv WRITE. inv PROMISE. esplits; eauto. econs.
+      + i. erewrite Memory.add_o in GET; eauto.
+        erewrite Memory.add_o; cycle 1; eauto. des_ifs; eauto.
+      + i. inv COV. erewrite Memory.add_o in GET; eauto. des_ifs.
+        * ss; des; clarify. eapply Memory.add_get0 in MEM. des.
+          econs; eauto. inv ITV. econs; eauto.
+          ss. eapply TimeFacts.le_lt_lt; eauto.
+        * exploit COVER.
+          { econs; eauto. }
+          intros COV. inv COV. eapply Memory.add_get1 in GET0; eauto.
+          econs; eauto.
+  Qed.
+
+  Lemma shorter_memory_step
+        P lang th_src th_tgt th_tgt' st st' v v' prom' sc sc'
+        mem_tgt mem_tgt' mem_src e
+        (STEP: (@pred_step (P /1\ no_promise) lang) e th_tgt th_tgt')
+        (TH_SRC: th_src = Thread.mk lang st (Local.mk v Memory.bot) sc mem_src)
+        (TH_TGT0: th_tgt = Thread.mk lang st (Local.mk v Memory.bot) sc mem_tgt)
+        (TH_TGT1: th_tgt' = Thread.mk lang st' (Local.mk v' prom') sc' mem_tgt')
+        (SHORTER: shorter_memory mem_src mem_tgt)
+    :
+      exists mem_src',
+        (<<STEP: (@pred_step (P /1\ no_promise) lang)
+                   e th_src
+                   (Thread.mk lang st' (Local.mk v' prom') sc' mem_src')>>) /\
+        (<<SHORTER: shorter_memory mem_src' mem_tgt'>>).
+  Proof.
+    dup SHORTER. inv SHORTER. inv STEP. inv STEP0. des. inv STEP.
+    - inv STEP0. ss.
+    - inv STEP0. inv LOCAL.
+      + exists mem_src; eauto. econs; eauto. econs; eauto.
+        econs; eauto. econs 2; eauto. econs; eauto.
+      + inv LOCAL0. ss. clarify. exploit COMPLETE; eauto. i. des.
+        exists mem_src; eauto. econs; eauto. econs; eauto.
+        econs; eauto. econs 2; eauto. econs; eauto.
+      + exploit write_msg_wf; eauto. i. des.
+        inv LOCAL0. ss. clarify.
+        exploit memory_write_bot_add; eauto. i. clarify.
+        dup WRITE. exploit shorter_memory_write; eauto.
+        { refl. }
+        i. des. esplits; eauto. econs; eauto. econs; eauto.
+        econs 2; eauto. econs; eauto.
+      + inv LOCAL1. ss. exploit write_msg_wf; eauto. i. des.
+        exploit COMPLETE; eauto. i. des.
+        inv LOCAL2. ss. clarify.
+        exploit memory_write_bot_add; eauto. i. clarify.
+        dup WRITE. exploit shorter_memory_write; eauto.
+        { refl. }
+        i. des. esplits; eauto. econs; eauto. econs; eauto.
+        econs 2; eauto. econs; eauto.
+      + inv LOCAL0. ss. clarify. esplits; eauto. econs; eauto.
+        econs; eauto. econs 2; eauto. econs; eauto.
+      + inv LOCAL0. ss. clarify. esplits; eauto. econs; eauto.
+        econs; eauto. econs 2; eauto. econs; eauto.
+  Qed.
+
+End SHORTERMEMORY.
+
+
+
+Section NOTATTATCHED.
+
+  Definition not_attatched (L: Loc.t -> Time.t -> Prop) (m: Memory.t) :=
+    forall loc to (SAT: L loc to),
+      (<<GET: exists msg, <<MSG: Memory.get loc to m = Some msg>> >>) /\
+      (<<NOATTATCH: exists to',
+          (<<TLE: Time.lt to to'>>) /\
+          (<<EMPTY: forall t (ITV: Interval.mem (to, to') t), ~ covered loc t m>>)>>).
+
+  Lemma not_attatch_write L prom mem_src loc from1 to1 val released mem_src'
+        (ADD: Memory.write Memory.bot mem_src loc from1 to1 val released prom mem_src' Memory.op_kind_add)
+        (NOATTATCH: not_attatched L mem_src)
+        (FROM: ~ L loc from1)
+    :
+      (<<NOATTATCH: not_attatched L mem_src'>>).
+  Proof.
+    inv ADD. inv PROMISE. ii.
+    exploit NOATTATCH; eauto. i. des. destruct msg.
+    destruct (Loc.eq_dec loc loc0); clarify.
+    - esplit; eauto.
+      + eexists. eapply Memory.add_get1; eauto.
+      + exists (if (Time.le_lt_dec to from1)
+                then (Time.meet to' from1)
+                else to'). esplits; eauto.
+        * unfold Time.meet. des_ifs.
+          destruct l; eauto. destruct H. clarify.
+        * ii. erewrite add_covered in H; eauto. des.
+          { eapply EMPTY; eauto. unfold Time.meet in *. des_ifs.
+            inv ITV. econs; ss; eauto.
+            left. eapply TimeFacts.le_lt_lt; eauto. }
+          { clarify. unfold Time.meet in *.
+            dup ITV. dup H0. inv ITV. inv H0. ss. des_ifs.
+            - clear - FROM1 TO l0.
+              eapply DenseOrder.DenseOrder.lt_strorder.
+              instantiate (1:=from1).
+              eapply TimeFacts.lt_le_lt; eauto.
+            - eapply DenseOrder.DenseOrder.lt_strorder.
+              instantiate (1:=from1).
+              eapply TimeFacts.lt_le_lt; eauto.
+            - dup MEM. eapply Memory.add_get0 in MEM. des.
+              exploit Memory.get_disjoint.
+              { eapply Memory.add_get1; try apply MSG; eauto. }
+              { eapply GET0. }
+              i. des; clarify. eapply x0.
+              { instantiate (1:=to).
+                exploit Memory.get_ts; eauto. i. des; clarify.
+                - exfalso. eapply DenseOrder.DenseOrder.lt_strorder.
+                  instantiate (1:=from1).
+                  eapply TimeFacts.lt_le_lt; try apply l; eauto.
+                  eapply Time.bot_spec.
+                - econs; ss; eauto. refl. }
+              { econs; ss; eauto. left.
+                eapply TimeFacts.lt_le_lt; eauto. }
+          }
+    - esplits; eauto.
+      + eapply Memory.add_get1; eauto.
+      + ii. erewrite add_covered in H; eauto. des; clarify.
+        eapply EMPTY; eauto.
+  Qed.
+
+  Lemma no_update_on_step
+        P L0 L1 lang th_src th_tgt th_tgt' st st' v v' prom' sc sc'
+        mem_tgt mem_tgt' mem_src e_tgt
+        (STEP: (@pred_step (P /1\ write_not_in L0 /1\ no_update_on L1 /1\ no_promise) lang) e_tgt th_tgt th_tgt')
+        (TH_SRC: th_src = Thread.mk lang st (Local.mk v Memory.bot) sc mem_src)
+        (TH_TGT0: th_tgt = Thread.mk lang st (Local.mk v Memory.bot) sc mem_tgt)
+        (TH_TGT1: th_tgt' = Thread.mk lang st' (Local.mk v' prom') sc' mem_tgt')
+        (SHORTER: shorter_memory mem_src mem_tgt)
+        (NOATTATCH: not_attatched L1 mem_src)
+    :
+      exists e_src mem_src',
+        (<<STEP: (@pred_step ((fun _ => True) /1\ write_not_in L0 /1\ no_promise) lang)
+                   e_src th_src
+                   (Thread.mk lang st' (Local.mk v' prom') sc' mem_src')>>) /\
+        (<<EVT: ThreadEvent.get_event e_src = ThreadEvent.get_event e_tgt>>) /\
+        (<<SHORTER: shorter_memory mem_src' mem_tgt'>>) /\
+        (<<NOATTATCH: not_attatched L1 mem_src'>>).
+  Proof.
+    dup SHORTER. inv SHORTER. inv STEP. inv STEP0. des. inv STEP.
+    - inv STEP0. ss.
+    - inv STEP0. inv LOCAL.
+      + eexists. exists mem_src; eauto. econs; eauto. econs; eauto.
+        econs; eauto. econs 2; eauto. econs; eauto.
+      + inv LOCAL0. ss. clarify. exploit COMPLETE; eauto. i. des.
+        exists (ThreadEvent.read loc ts val released ord). exists mem_src; eauto.
+        econs; eauto. econs; eauto. econs; eauto. econs 2; eauto. econs; eauto.
+      + exploit write_msg_wf; eauto. i. des.
+        exists (ThreadEvent.write loc (Time.middle from to) to val released ord).
+        inv LOCAL0. ss. clarify.
+        exploit memory_write_bot_add; eauto. i. clarify.
+        dup WRITE. exploit Time.middle_spec; eauto. i. des.
+        exploit shorter_memory_write.
+        { eauto. }
+        { eauto. }
+        { instantiate (1:=Time.middle from to). left. auto. }
+        { auto. }
+        i. des. esplits; eauto.
+        * econs; eauto.
+          { econs; eauto. econs 2; eauto. econs; eauto. }
+          ss. esplits; eauto. i. eapply SAT2; eauto.
+          inv IN; ss. econs; eauto.
+        * eapply not_attatch_write; eauto. ii.
+          exploit NOATTATCH; eauto. i. des.
+          exploit memory_add_cover_disjoint; auto.
+          { inv WRITE. inv PROMISE. eapply MEM. }
+          { instantiate (1:=(Time.middle from to)).
+            econs; eauto. ss. left. eauto. }
+          { apply COVER. destruct msg. econs; eauto.
+            econs; ss; eauto.
+            - exploit Memory.get_ts; eauto. i. des; clarify.
+              exfalso. rewrite x3 in *.
+              eapply DenseOrder.DenseOrder.lt_strorder.
+              instantiate (1:=Time.bot).
+              eapply DenseOrder.DenseOrderFacts.le_lt_lt; eauto.
+              apply Time.bot_spec.
+            - refl. }
+      + inv LOCAL1. ss.
+        exists (ThreadEvent.update loc tsr tsw valr valw releasedr releasedw ordr ordw).
+        exploit write_msg_wf; eauto. i. des.
+        exploit COMPLETE; eauto. i. des.
+        inv LOCAL2. ss. clarify.
+        exploit memory_write_bot_add; eauto. i. clarify.
+        dup WRITE. exploit shorter_memory_write; eauto.
+        { refl. }
+        i. des. esplits; eauto.
+        * econs; eauto. econs; eauto.
+          econs 2; eauto. econs; eauto.
+        * eapply not_attatch_write; eauto.
+      + inv LOCAL0. exists (ThreadEvent.fence ordr ordw).
+        ss. clarify. esplits; eauto. econs; eauto.
+        econs; eauto. econs 2; eauto. econs; eauto.
+      + inv LOCAL0. exists (ThreadEvent.syscall e).
+        ss. clarify. esplits; eauto. econs; eauto.
+        econs; eauto. econs 2; eauto. econs; eauto.
+  Qed.
+
+End NOTATTATCHED.
+
+
+Section NOSC.
+
+  Lemma no_sc_any_sc
+        P lang th_src th_tgt th_tgt' st st' v v' prom prom' sc sc_src sc'
+        mem mem' e
+        (STEP: (@pred_step (P /1\ no_sc) lang) e th_tgt th_tgt')
+        (TH_SRC: th_src = Thread.mk lang st (Local.mk v prom) sc_src mem)
+        (TH_TGT0: th_tgt = Thread.mk lang st (Local.mk v prom) sc mem)
+        (TH_TGT1: th_tgt' = Thread.mk lang st' (Local.mk v' prom') sc' mem')
   :
     exists sc_src',
       (<<STEP: (@pred_step (P /1\ no_sc) lang)
                  e th_src
                  (Thread.mk lang st' (Local.mk v' prom') sc_src' mem')>>).
-Proof.
-  clarify. inv STEP. inv STEP0. des. inv STEP.
-  - inv STEP0. inv LOCAL. ss. clarify.
-    esplits. econs; eauto. econs; eauto. econs 1; eauto. econs; eauto.
-  - inv STEP0. inv LOCAL; ss.
-    + esplits. econs; eauto. econs; eauto. econs 2; eauto. econs; eauto.
-    + esplits. econs; eauto. econs; eauto. econs 2; eauto. econs; eauto.
-    + inv LOCAL0. ss. clarify. exists sc_src.
-      econs; eauto. econs; eauto. econs 2; eauto. econs; eauto.
-      econs; eauto. econs; eauto. ss.
-      inv WRITABLE. econs; eauto.
-    + inv LOCAL1. ss. inv LOCAL2. ss. clarify. exists sc_src.
-      econs; eauto. econs; eauto. econs 2; eauto. econs; eauto.
-      econs; eauto. econs; eauto. ss.
-      inv WRITABLE. econs; eauto.
-    + inv LOCAL0. ss. clarify.
-      esplits. econs; eauto. econs; eauto. econs 2; eauto. econs; eauto.
-      econs; eauto. econs; eauto. ss. f_equal.
-      unfold TView.write_fence_tview. ss. des_ifs.
-Qed.
+  Proof.
+    clarify. inv STEP. inv STEP0. des. inv STEP.
+    - inv STEP0. inv LOCAL. ss. clarify.
+      esplits. econs; eauto. econs; eauto. econs 1; eauto. econs; eauto.
+    - inv STEP0. inv LOCAL; ss.
+      + esplits. econs; eauto. econs; eauto. econs 2; eauto. econs; eauto.
+      + esplits. econs; eauto. econs; eauto. econs 2; eauto. econs; eauto.
+      + inv LOCAL0. ss. clarify. exists sc_src.
+        econs; eauto. econs; eauto. econs 2; eauto. econs; eauto.
+        econs; eauto. econs; eauto. ss.
+        inv WRITABLE. econs; eauto.
+      + inv LOCAL1. ss. inv LOCAL2. ss. clarify. exists sc_src.
+        econs; eauto. econs; eauto. econs 2; eauto. econs; eauto.
+        econs; eauto. econs; eauto. ss.
+        inv WRITABLE. econs; eauto.
+      + inv LOCAL0. ss. clarify.
+        esplits. econs; eauto. econs; eauto. econs 2; eauto. econs; eauto.
+        econs; eauto. econs; eauto. ss. f_equal.
+        unfold TView.write_fence_tview. ss. des_ifs.
+  Qed.
 
-Inductive shorter_memory (mem_src mem_tgt: Memory.t): Prop :=
-| shorter_memory_intro
-    (COMPLETE: forall loc to from_tgt msg
-                      (GET: Memory.get loc to mem_tgt = Some (from_tgt, msg)),
-        exists from_src,
-          (<<GET: Memory.get loc to mem_src = Some (from_src, msg)>>))
-    (COVER: forall l t (COV: covered l t mem_src), covered l t mem_tgt)
-.
-Global Program Instance shorter_memory_PreOrder: PreOrder shorter_memory.
-Next Obligation. ii. econs; eauto. Qed.
-Next Obligation.
-  ii. inv H. inv H0. econs; eauto.
-  ii. exploit COMPLETE0; eauto. i. des.
-  exploit COMPLETE; eauto.
-Qed.
+  Lemma consistent_certification_no_sc
+        P lang th_tgt th_tgt' st st' v v' prom prom' sc sc'
+        mem_tgt mem_tgt' e_tgt
+        (SCMAX: ~ promise_view_consistent prom sc)
+        (TH_TGT0: th_tgt = Thread.mk lang st (Local.mk v Memory.bot) sc mem_tgt)
+        (TH_TGT1: th_tgt' = Thread.mk lang st' (Local.mk v' prom') sc' mem_tgt')
+        (CONSISTENT: promise_view_consistent prom v'.(TView.cur).(View.rlx))
+        (STEP: (@pred_step (P /1\ no_promise) lang) e_tgt th_tgt th_tgt')
+    :
+      no_sc e_tgt.
+  Proof.
+    inv STEP. inv STEP0; ss. inv STEP; ss.
+    - inv STEP0. ss.
+    - inv STEP0. inv LOCAL; ss.
+      + ii. clarify. inv LOCAL0. ss. clarify. ss. eapply SCMAX.
+        eapply promise_view_consistent_le; eauto. des_ifs; ss.
+        eapply TViewFacts.write_fence_sc_incr.
+      + ii. clarify. inv LOCAL0. ss. clarify. ss. eapply SCMAX.
+        eapply promise_view_consistent_le; eauto. des_ifs; ss.
+        eapply TViewFacts.write_fence_sc_incr.
+  Qed.
 
-Definition not_attatched (L: Loc.t -> Time.t -> Prop) (m: Memory.t) :=
-  forall loc to (SAT: L loc to),
-    (<<GET: exists msg, <<MSG: Memory.get loc to m = Some msg>> >>) /\
-    (<<NOATTATCH: exists to',
-        (<<TLE: Time.lt to to'>>) /\
-        (<<EMPTY: forall t (ITV: Interval.mem (to, to') t), ~ covered loc t m>>)>>).
+End NOSC.
 
-Definition no_update_on (MSGS : Loc.t -> Time.t -> Prop)
-           (e : ThreadEvent.t) : Prop :=
-  match e with
-  | ThreadEvent.update loc from to _ _ _ _ _ _ =>
-    ~ MSGS loc from
-  | _ => True
-  end.
 
-(* TODO: make threadevent le and force eventpredicate is closed under that? *)
-Lemma shorter_memory_write prom mem_src mem_tgt loc from1 to1 val released mem_tgt' from'
-      (SHORTER: shorter_memory mem_src mem_tgt)
-      (ADD: Memory.write Memory.bot mem_tgt loc from1 to1 val released prom mem_tgt' Memory.op_kind_add)
-      (TO: Time.le from1 from')
-      (FROM: Time.lt from' to1)
-  :
-    exists mem_src',
-      (<<ADD: Memory.write Memory.bot mem_src loc from' to1 val released prom mem_src' Memory.op_kind_add>>) /\
-      (<<SHORTER: shorter_memory mem_src' mem_tgt'>>).
-Proof.
-  dup SHORTER. inv SHORTER. inv ADD. inv PROMISE.
-  exploit MemoryFacts.MemoryFacts.add_remove_eq; try apply REMOVE; eauto. i. clarify.
-  exploit write_succeed; eauto.
-  - instantiate (1:=mem_src). instantiate (1:=loc).
-    ii. eapply COVER in COVER0. inv COVER0.
-    dup MEM. eapply Memory.add_get0 in MEM. des.
-    dup GET. eapply Memory.add_get1 in GET; eauto.
-    exploit Memory.get_disjoint.
-    + eapply GET.
-    + eapply GET1.
-    + i. des; clarify.
-      eapply x0; eauto. inv H. econs; ss; eauto.
-      eapply TimeFacts.le_lt_lt; eauto.
-  - inv MEM. inv ADD. inv MSG_WF. inv TS. eauto.
-  - inv MEM. inv ADD. eauto.
-  - i. des. inv WRITE. inv PROMISE. esplits; eauto. econs.
-    + i. erewrite Memory.add_o in GET; eauto.
-      erewrite Memory.add_o; cycle 1; eauto. des_ifs; eauto.
-    + i. inv COV. erewrite Memory.add_o in GET; eauto. des_ifs.
-      * ss; des; clarify. eapply Memory.add_get0 in MEM. des.
-        econs; eauto. inv ITV. econs; eauto.
-        ss. eapply TimeFacts.le_lt_lt; eauto.
-      * exploit COVER.
-        { econs; eauto. }
-        intros COV. inv COV. eapply Memory.add_get1 in GET0; eauto.
-        econs; eauto.
-Qed.
+Section WFPROMISE.
 
-Lemma shorter_memory_step
-      P lang th_src th_tgt th_tgt' st st' v v' prom' sc sc'
-      mem_tgt mem_tgt' mem_src e
-      (STEP: (@pred_step (P /1\ no_promise) lang) e th_tgt th_tgt')
-      (TH_SRC: th_src = Thread.mk lang st (Local.mk v Memory.bot) sc mem_src)
-      (TH_TGT0: th_tgt = Thread.mk lang st (Local.mk v Memory.bot) sc mem_tgt)
-      (TH_TGT1: th_tgt' = Thread.mk lang st' (Local.mk v' prom') sc' mem_tgt')
-      (SHORTER: shorter_memory mem_src mem_tgt)
-  :
-    exists mem_src',
-      (<<STEP: (@pred_step (P /1\ no_promise) lang)
-                 e th_src
-                 (Thread.mk lang st' (Local.mk v' prom') sc' mem_src')>>) /\
-      (<<SHORTER: shorter_memory mem_src' mem_tgt'>>).
-Proof.
-  dup SHORTER. inv SHORTER. inv STEP. inv STEP0. des. inv STEP.
-  - inv STEP0. ss.
-  - inv STEP0. inv LOCAL.
-    + exists mem_src; eauto. econs; eauto. econs; eauto.
-      econs; eauto. econs 2; eauto. econs; eauto.
-    + inv LOCAL0. ss. clarify. exploit COMPLETE; eauto. i. des.
-      exists mem_src; eauto. econs; eauto. econs; eauto.
-      econs; eauto. econs 2; eauto. econs; eauto.
-    + exploit write_msg_wf; eauto. i. des.
-      inv LOCAL0. ss. clarify.
-      exploit memory_write_bot_add; eauto. i. clarify.
-      dup WRITE. exploit shorter_memory_write; eauto.
-      { refl. }
-      i. des. esplits; eauto. econs; eauto. econs; eauto.
-      econs 2; eauto. econs; eauto.
-    + inv LOCAL1. ss. exploit write_msg_wf; eauto. i. des.
-      exploit COMPLETE; eauto. i. des.
-      inv LOCAL2. ss. clarify.
-      exploit memory_write_bot_add; eauto. i. clarify.
-      dup WRITE. exploit shorter_memory_write; eauto.
-      { refl. }
-      i. des. esplits; eauto. econs; eauto. econs; eauto.
-      econs 2; eauto. econs; eauto.
-    + inv LOCAL0. ss. clarify. esplits; eauto. econs; eauto.
-      econs; eauto. econs 2; eauto. econs; eauto.
-    + inv LOCAL0. ss. clarify. esplits; eauto. econs; eauto.
-      econs; eauto. econs 2; eauto. econs; eauto.
-Qed.
+  Definition wf_promise (mem: Memory.t): Prop :=
+    forall loc, Memory.get loc Time.bot mem = None.
 
-Lemma not_attatch_write L prom mem_src loc from1 to1 val released mem_src'
-      (ADD: Memory.write Memory.bot mem_src loc from1 to1 val released prom mem_src' Memory.op_kind_add)
-      (NOATTATCH: not_attatched L mem_src)
-      (FROM: ~ L loc from1)
-  :
-    (<<NOATTATCH: not_attatched L mem_src'>>).
-Proof.
-  inv ADD. inv PROMISE. ii.
-  exploit NOATTATCH; eauto. i. des. destruct msg.
-  destruct (Loc.eq_dec loc loc0); clarify.
-  - esplit; eauto.
-    + eexists. eapply Memory.add_get1; eauto.
-    + exists (if (Time.le_lt_dec to from1)
-              then (Time.meet to' from1)
-              else to'). esplits; eauto.
-      * unfold Time.meet. des_ifs.
-        destruct l; eauto. destruct H. clarify.
-      * ii. erewrite add_covered in H; eauto. des.
-        { eapply EMPTY; eauto. unfold Time.meet in *. des_ifs.
-          inv ITV. econs; ss; eauto.
-          left. eapply TimeFacts.le_lt_lt; eauto. }
-        { clarify. unfold Time.meet in *.
-          dup ITV. dup H0. inv ITV. inv H0. ss. des_ifs.
-          - clear - FROM1 TO l0.
-            eapply DenseOrder.DenseOrder.lt_strorder.
-            instantiate (1:=from1).
-            eapply TimeFacts.lt_le_lt; eauto.
-          - eapply DenseOrder.DenseOrder.lt_strorder.
-            instantiate (1:=from1).
-            eapply TimeFacts.lt_le_lt; eauto.
-          - dup MEM. eapply Memory.add_get0 in MEM. des.
-            exploit Memory.get_disjoint.
-            { eapply Memory.add_get1; try apply MSG; eauto. }
-            { eapply GET0. }
-            i. des; clarify. eapply x0.
-            { instantiate (1:=to).
-              exploit Memory.get_ts; eauto. i. des; clarify.
-              - exfalso. eapply DenseOrder.DenseOrder.lt_strorder.
-                instantiate (1:=from1).
-                eapply TimeFacts.lt_le_lt; try apply l; eauto.
-                eapply Time.bot_spec.
-              - econs; ss; eauto. refl. }
-            { econs; ss; eauto. left.
-              eapply TimeFacts.lt_le_lt; eauto. }
-        }
-  - esplits; eauto.
-    + eapply Memory.add_get1; eauto.
-    + ii. erewrite add_covered in H; eauto. des; clarify.
-      eapply EMPTY; eauto.
-Qed.
-
-Lemma no_update_on_step
-      P L0 L1 lang th_src th_tgt th_tgt' st st' v v' prom' sc sc'
-      mem_tgt mem_tgt' mem_src e_tgt
-      (STEP: (@pred_step (P /1\ write_not_in L0 /1\ no_update_on L1 /1\ no_promise) lang) e_tgt th_tgt th_tgt')
-      (TH_SRC: th_src = Thread.mk lang st (Local.mk v Memory.bot) sc mem_src)
-      (TH_TGT0: th_tgt = Thread.mk lang st (Local.mk v Memory.bot) sc mem_tgt)
-      (TH_TGT1: th_tgt' = Thread.mk lang st' (Local.mk v' prom') sc' mem_tgt')
-      (SHORTER: shorter_memory mem_src mem_tgt)
-      (NOATTATCH: not_attatched L1 mem_src)
-  :
-    exists e_src mem_src',
-      (<<STEP: (@pred_step ((fun _ => True) /1\ write_not_in L0 /1\ no_promise) lang)
-                 e_src th_src
-                 (Thread.mk lang st' (Local.mk v' prom') sc' mem_src')>>) /\
-      (<<EVT: ThreadEvent.get_event e_src = ThreadEvent.get_event e_tgt>>) /\
-      (<<SHORTER: shorter_memory mem_src' mem_tgt'>>) /\
-      (<<NOATTATCH: not_attatched L1 mem_src'>>).
-Proof.
-  dup SHORTER. inv SHORTER. inv STEP. inv STEP0. des. inv STEP.
-  - inv STEP0. ss.
-  - inv STEP0. inv LOCAL.
-    + eexists. exists mem_src; eauto. econs; eauto. econs; eauto.
-      econs; eauto. econs 2; eauto. econs; eauto.
-    + inv LOCAL0. ss. clarify. exploit COMPLETE; eauto. i. des.
-      exists (ThreadEvent.read loc ts val released ord). exists mem_src; eauto.
-      econs; eauto. econs; eauto. econs; eauto. econs 2; eauto. econs; eauto.
-    + exploit write_msg_wf; eauto. i. des.
-      exists (ThreadEvent.write loc (Time.middle from to) to val released ord).
-      inv LOCAL0. ss. clarify.
-      exploit memory_write_bot_add; eauto. i. clarify.
-      dup WRITE. exploit Time.middle_spec; eauto. i. des.
-      exploit shorter_memory_write.
-      { eauto. }
-      { eauto. }
-      { instantiate (1:=Time.middle from to). left. auto. }
-      { auto. }
-      i. des. esplits; eauto.
-      * econs; eauto.
-        { econs; eauto. econs 2; eauto. econs; eauto. }
-        ss. esplits; eauto. i. eapply SAT2; eauto.
-        inv IN; ss. econs; eauto.
-      * eapply not_attatch_write; eauto. ii.
-        exploit NOATTATCH; eauto. i. des.
-        exploit memory_add_cover_disjoint; auto.
-        { inv WRITE. inv PROMISE. eapply MEM. }
-        { instantiate (1:=(Time.middle from to)).
-          econs; eauto. ss. left. eauto. }
-        { apply COVER. destruct msg. econs; eauto.
-          econs; ss; eauto.
-          - exploit Memory.get_ts; eauto. i. des; clarify.
-            exfalso. rewrite x3 in *.
-            eapply DenseOrder.DenseOrder.lt_strorder.
-            instantiate (1:=Time.bot).
-            eapply DenseOrder.DenseOrderFacts.le_lt_lt; eauto.
-            apply Time.bot_spec.
-          - refl. }
-    + inv LOCAL1. ss.
-      exists (ThreadEvent.update loc tsr tsw valr valw releasedr releasedw ordr ordw).
-      exploit write_msg_wf; eauto. i. des.
-      exploit COMPLETE; eauto. i. des.
-      inv LOCAL2. ss. clarify.
-      exploit memory_write_bot_add; eauto. i. clarify.
-      dup WRITE. exploit shorter_memory_write; eauto.
-      { refl. }
-      i. des. esplits; eauto.
-      * econs; eauto. econs; eauto.
-        econs 2; eauto. econs; eauto.
-      * eapply not_attatch_write; eauto.
-    + inv LOCAL0. exists (ThreadEvent.fence ordr ordw).
-      ss. clarify. esplits; eauto. econs; eauto.
-      econs; eauto. econs 2; eauto. econs; eauto.
-    + inv LOCAL0. exists (ThreadEvent.syscall e).
-      ss. clarify. esplits; eauto. econs; eauto.
-      econs; eauto. econs 2; eauto. econs; eauto.
-Qed.
-
-Inductive forget_statelocal:
-  sigT Language.state * Local.t -> sigT Language.state * Local.t -> Prop :=
-| forget_statelocal_intro
-    st lc1 lc2
-    (TVIEW : lc1.(Local.tview) = lc2.(Local.tview))
-    (PROMS : lc1.(Local.promises) = Memory.bot)
-  :
-    forget_statelocal (st, lc1) (st, lc2)
-.
-
-Inductive full_promised (mem: Memory.t) (loc: Loc.t) (to: Time.t) : Prop :=
-| full_promised_intro
-    from val released
-    (GET: Memory.get loc to mem = Some (from, Message.full val released))
-.
-
-Inductive all_promises (c: Configuration.t) (P: IdentMap.key -> Prop)
-          (l: Loc.t) (t: Time.t) : Prop :=
-| all_promises_intro
-    tid st lc
-    (TID1: IdentMap.find tid c.(Configuration.threads) = Some (st, lc))
-    (PROMISED: promised lc.(Local.promises) l t)
-    (SAT: P tid)
-.
-
-Inductive pf_sim_memory (proms: Loc.t -> Time.t -> Prop) (mem_src mem_tgt: Memory.t): Prop :=
-| pf_sim_memory_intro
-    mem_inter
-    (FORGET: forget_memory proms mem_inter mem_tgt)
-    (SHORTER: shorter_memory mem_src mem_inter)
-.
-
-Inductive forget_config csrc ctgt : Prop :=
-| forget_configuration_intro
-    (THS : forall tid, option_rel
-                         forget_statelocal
-                         (IdentMap.find tid csrc.(Configuration.threads))
-                         (IdentMap.find tid ctgt.(Configuration.threads)))
-    (SC : csrc.(Configuration.sc) = ctgt.(Configuration.sc))
-    (MEM : pf_sim_memory (all_promises ctgt (fun _ => True))
-                         (Configuration.memory csrc)
-                         (Configuration.memory ctgt))
-.
-
-Definition wf_promise (mem: Memory.t): Prop :=
-  forall loc, Memory.get loc Time.bot mem = None.
-
-Lemma wf_promise_promise
-      promises1 mem1 loc from to msg promises2 mem2 kind
-      (PROMISE: Memory.promise promises1 mem1 loc from to msg promises2 mem2 kind)
-      (WFPROM: wf_promise promises1)
-      (INHABITED: Memory.inhabited mem1)
-  :
-    (<<WFPROM: wf_promise promises2>>) /\
-    (<<INHABITED: Memory.inhabited mem2>>).
-Proof.
-  inv PROMISE.
-  - split; [|eapply Memory.op_inhabited; eauto].
-    ii. erewrite Memory.add_o; eauto. des_ifs.
-    ss; des; clarify. exfalso.
-    inv MEM. inv ADD.
-    eapply DenseOrder.DenseOrder.lt_strorder.
-    instantiate (1:=Time.bot).
-    eapply TimeFacts.le_lt_lt; eauto. apply Time.bot_spec.
-  - split; [|eapply Memory.op_inhabited; eauto].
-    ii. erewrite Memory.split_o; eauto. des_ifs.
-    + ss; des; clarify. exfalso.
-      inv MEM. inv SPLIT.
+  Lemma wf_promise_promise
+        promises1 mem1 loc from to msg promises2 mem2 kind
+        (PROMISE: Memory.promise promises1 mem1 loc from to msg promises2 mem2 kind)
+        (WFPROM: wf_promise promises1)
+        (INHABITED: Memory.inhabited mem1)
+    :
+      (<<WFPROM: wf_promise promises2>>) /\
+      (<<INHABITED: Memory.inhabited mem2>>).
+  Proof.
+    inv PROMISE.
+    - split; [|eapply Memory.op_inhabited; eauto].
+      ii. erewrite Memory.add_o; eauto. des_ifs.
+      ss; des; clarify. exfalso.
+      inv MEM. inv ADD.
       eapply DenseOrder.DenseOrder.lt_strorder.
       instantiate (1:=Time.bot).
       eapply TimeFacts.le_lt_lt; eauto. apply Time.bot_spec.
-    + ss. destruct a. clarify. exfalso.
-      inv MEM. inv SPLIT.
+    - split; [|eapply Memory.op_inhabited; eauto].
+      ii. erewrite Memory.split_o; eauto. des_ifs.
+      + ss; des; clarify. exfalso.
+        inv MEM. inv SPLIT.
+        eapply DenseOrder.DenseOrder.lt_strorder.
+        instantiate (1:=Time.bot).
+        eapply TimeFacts.le_lt_lt; eauto. apply Time.bot_spec.
+      + ss. destruct a. clarify. exfalso.
+        inv MEM. inv SPLIT.
+        eapply DenseOrder.DenseOrder.lt_strorder.
+        instantiate (1:=Time.bot).
+        eapply TimeFacts.le_lt_lt; eauto. apply Time.bot_spec.
+    - split; [|eapply Memory.op_inhabited; eauto].
+      ii. erewrite Memory.lower_o; eauto. des_ifs.
+      ss; des; clarify. exfalso.
+      inv MEM. inv LOWER.
       eapply DenseOrder.DenseOrder.lt_strorder.
       instantiate (1:=Time.bot).
       eapply TimeFacts.le_lt_lt; eauto. apply Time.bot_spec.
-  - split; [|eapply Memory.op_inhabited; eauto].
-    ii. erewrite Memory.lower_o; eauto. des_ifs.
-    ss; des; clarify. exfalso.
-    inv MEM. inv LOWER.
-    eapply DenseOrder.DenseOrder.lt_strorder.
-    instantiate (1:=Time.bot).
-    eapply TimeFacts.le_lt_lt; eauto. apply Time.bot_spec.
-Qed.
+  Qed.
 
-Lemma wf_promise_remove
-      prom1 loc from1 to1 msg1 prom2
-      (REMOVE: Memory.remove prom1 loc from1 to1 msg1 prom2)
-      (WFPROM: wf_promise prom1)
-  :
-    wf_promise prom2.
-Proof.
-  ii. erewrite Memory.remove_o; eauto. des_ifs.
-Qed.
+  Lemma wf_promise_remove
+        prom1 loc from1 to1 msg1 prom2
+        (REMOVE: Memory.remove prom1 loc from1 to1 msg1 prom2)
+        (WFPROM: wf_promise prom1)
+    :
+      wf_promise prom2.
+  Proof.
+    ii. erewrite Memory.remove_o; eauto. des_ifs.
+  Qed.
 
-Lemma wf_promise_step pf e lang (th0 th1: Thread.t lang)
-      (STEP: Thread.step pf e th0 th1)
-      (WFPROM: wf_promise th0.(Thread.local).(Local.promises))
-      (INHABITED: Memory.inhabited th0.(Thread.memory))
-  :
-    (<<WFPROM: wf_promise th1.(Thread.local).(Local.promises)>>) /\
-    (<<INHABITED: Memory.inhabited th1.(Thread.memory)>>)
-.
-Proof.
-  inv STEP; ss.
-  - inv STEP0; ss. inv LOCAL; ss.
-    eapply wf_promise_promise; eauto.
-  - inv STEP0; ss. inv LOCAL; ss.
-    + inv LOCAL0; ss.
-    + inv LOCAL0; ss. inv WRITE; ss.
-      exploit wf_promise_promise; eauto. i. des. split; ss.
-      eapply wf_promise_remove; eauto.
-    + inv LOCAL1; ss. inv LOCAL2; ss. inv WRITE; ss.
-      exploit wf_promise_promise; eauto. i. des. split; ss.
-      eapply wf_promise_remove; eauto.
-    + inv LOCAL0; ss.
-    + inv LOCAL0; ss.
-Qed.
+  Lemma wf_promise_step pf e lang (th0 th1: Thread.t lang)
+        (STEP: Thread.step pf e th0 th1)
+        (WFPROM: wf_promise th0.(Thread.local).(Local.promises))
+        (INHABITED: Memory.inhabited th0.(Thread.memory))
+    :
+      (<<WFPROM: wf_promise th1.(Thread.local).(Local.promises)>>) /\
+      (<<INHABITED: Memory.inhabited th1.(Thread.memory)>>)
+  .
+  Proof.
+    inv STEP; ss.
+    - inv STEP0; ss. inv LOCAL; ss.
+      eapply wf_promise_promise; eauto.
+    - inv STEP0; ss. inv LOCAL; ss.
+      + inv LOCAL0; ss.
+      + inv LOCAL0; ss. inv WRITE; ss.
+        exploit wf_promise_promise; eauto. i. des. split; ss.
+        eapply wf_promise_remove; eauto.
+      + inv LOCAL1; ss. inv LOCAL2; ss. inv WRITE; ss.
+        exploit wf_promise_promise; eauto. i. des. split; ss.
+        eapply wf_promise_remove; eauto.
+      + inv LOCAL0; ss.
+      + inv LOCAL0; ss.
+  Qed.
 
-Lemma wf_promise_rtc_step lang (th0 th1: Thread.t lang)
-      (STEP: rtc (@Thread.tau_step lang) th0 th1)
-      (INHABITED: Memory.inhabited th0.(Thread.memory))
-      (WFPROM: wf_promise th0.(Thread.local).(Local.promises))
-  :
-    (<<WFPROM: wf_promise th1.(Thread.local).(Local.promises)>>) /\
-    (<<INHABITED: Memory.inhabited th1.(Thread.memory)>>)
-.
-Proof.
-  eapply (@Relation_Operators.clos_refl_trans_1n_ind
-            _ (Thread.tau_step (lang:=lang))
-            (fun e0 e1 =>
-               forall (INHABITED: Memory.inhabited e0.(Thread.memory))
-                      (WFPROM: wf_promise e0.(Thread.local).(Local.promises)),
-                 (<<WFPROM: wf_promise e1.(Thread.local).(Local.promises)>>) /\
-                 (<<INHABITED: Memory.inhabited e1.(Thread.memory)>>))); eauto.
-  i. inv H. inv TSTEP. exploit wf_promise_step; eauto. i. des. eauto.
-Qed.
+  Lemma wf_promise_rtc_step lang (th0 th1: Thread.t lang)
+        (STEP: rtc (@Thread.tau_step lang) th0 th1)
+        (INHABITED: Memory.inhabited th0.(Thread.memory))
+        (WFPROM: wf_promise th0.(Thread.local).(Local.promises))
+    :
+      (<<WFPROM: wf_promise th1.(Thread.local).(Local.promises)>>) /\
+      (<<INHABITED: Memory.inhabited th1.(Thread.memory)>>)
+  .
+  Proof.
+    eapply (@Relation_Operators.clos_refl_trans_1n_ind
+              _ (Thread.tau_step (lang:=lang))
+              (fun e0 e1 =>
+                 forall (INHABITED: Memory.inhabited e0.(Thread.memory))
+                        (WFPROM: wf_promise e0.(Thread.local).(Local.promises)),
+                   (<<WFPROM: wf_promise e1.(Thread.local).(Local.promises)>>) /\
+                   (<<INHABITED: Memory.inhabited e1.(Thread.memory)>>))); eauto.
+    i. inv H. inv TSTEP. exploit wf_promise_step; eauto. i. des. eauto.
+  Qed.
 
-Lemma configuraion_step_wf_promises c1 c2 e tid
-      (CWF: Configuration.wf c1)
-      (STEP: Configuration.step e tid c1 c2)
-      (WFPROMS:
+  Lemma configuraion_step_wf_promises c1 c2 e tid
+        (CWF: Configuration.wf c1)
+        (STEP: Configuration.step e tid c1 c2)
+        (WFPROMS:
+           forall tid lang_src st_src lc_src
+                  (TIDSRC: IdentMap.find tid c1.(Configuration.threads) =
+                           Some (existT _ lang_src st_src, lc_src)),
+             wf_promise lc_src.(Local.promises))
+    :
+      (<<WFPROMS:
          forall tid lang_src st_src lc_src
-                (TIDSRC: IdentMap.find tid c1.(Configuration.threads) =
+                (TIDSRC: IdentMap.find tid c2.(Configuration.threads) =
                          Some (existT _ lang_src st_src, lc_src)),
-           wf_promise lc_src.(Local.promises))
-  :
-    (<<WFPROMS:
-       forall tid lang_src st_src lc_src
-              (TIDSRC: IdentMap.find tid c2.(Configuration.threads) =
-                       Some (existT _ lang_src st_src, lc_src)),
-         wf_promise lc_src.(Local.promises)>>).
-Proof.
-  inv STEP. ss. red. i. rewrite IdentMap.gsspec in TIDSRC. des_ifs.
-  - eapply inj_pair2 in H0. clarify.
-    inv CWF. inv MEM. ss.
-    exploit wf_promise_rtc_step; eauto. i. des.
-    exploit wf_promise_step; eauto. ss. i. des. eauto.
-  - eapply WFPROMS; eauto.
-Qed.
+           wf_promise lc_src.(Local.promises)>>).
+  Proof.
+    inv STEP. ss. red. i. rewrite IdentMap.gsspec in TIDSRC. des_ifs.
+    - eapply inj_pair2 in H0. clarify.
+      inv CWF. inv MEM. ss.
+      exploit wf_promise_rtc_step; eauto. i. des.
+      exploit wf_promise_step; eauto. ss. i. des. eauto.
+    - eapply WFPROMS; eauto.
+  Qed.
+
+End WFPROMISE.
+
+
+Section FORGET.
+
+  Inductive forget_statelocal:
+    sigT Language.state * Local.t -> sigT Language.state * Local.t -> Prop :=
+  | forget_statelocal_intro
+      st lc1 lc2
+      (TVIEW : lc1.(Local.tview) = lc2.(Local.tview))
+      (PROMS : lc1.(Local.promises) = Memory.bot)
+    :
+      forget_statelocal (st, lc1) (st, lc2)
+  .
+
+  Inductive pf_sim_memory (proms: Loc.t -> Time.t -> Prop) (mem_src mem_tgt: Memory.t): Prop :=
+  | pf_sim_memory_intro
+      mem_inter
+      (FORGET: forget_memory proms mem_inter mem_tgt)
+      (SHORTER: shorter_memory mem_src mem_inter)
+  .
+
+  Inductive forget_thread others lang: Thread.t lang -> Thread.t lang -> Prop :=
+  | forget_thread_intro
+      st v prom sc mem_src mem_tgt
+      (MEMP: pf_sim_memory (others \2/ promised prom) mem_src mem_tgt)
+    :
+      forget_thread
+        others
+        (Thread.mk lang st (Local.mk v prom) sc mem_src)
+        (Thread.mk lang st (Local.mk v Memory.bot) sc mem_tgt)
+  .
+
+  Inductive all_promises (c: Configuration.t) (P: IdentMap.key -> Prop)
+            (l: Loc.t) (t: Time.t) : Prop :=
+  | all_promises_intro
+      tid st lc
+      (TID1: IdentMap.find tid c.(Configuration.threads) = Some (st, lc))
+      (PROMISED: promised lc.(Local.promises) l t)
+      (SAT: P tid)
+  .
+
+  Inductive concrete_promised (mem: Memory.t) (loc: Loc.t) (to: Time.t) : Prop :=
+  | concrete_promised_intro
+      from val released
+      (GET: Memory.get loc to mem = Some (from, Message.full val released))
+  .
+
+  Inductive concrete_covered (mem: Memory.t) (loc: Loc.t) (ts: Time.t): Prop :=
+  | concrete_covered_intro
+      from to val released
+      (GET: Memory.get loc to mem = Some (from, Message.full val released))
+      (ITV: Interval.mem (from, to) ts)
+  .
+
+  Inductive forget_config csrc ctgt : Prop :=
+  | forget_configuration_intro
+      (THS : forall tid, option_rel
+                           forget_statelocal
+                           (IdentMap.find tid csrc.(Configuration.threads))
+                           (IdentMap.find tid ctgt.(Configuration.threads)))
+      (SC : csrc.(Configuration.sc) = ctgt.(Configuration.sc))
+      (MEM : pf_sim_memory (all_promises ctgt (fun _ => True))
+                           (Configuration.memory csrc)
+                           (Configuration.memory ctgt))
+  .
+
+End FORGET.
+
 
 Module Inv.
 
@@ -2181,10 +2250,8 @@ Module Inv.
             (proms: Memory.t) (updates : Loc.t -> Time.t -> Prop) (mlast: Memory.t): Prop :=
   | inv_intro
       (PROMS: forall
-          loc to m sc (PROM : full_promised proms loc to)
-          (FUTURE: unchanged_on
-                     (fun loc to => covered loc to proms)
-                     mlast m)
+          loc to m sc (PROM : concrete_promised proms loc to)
+          (FUTURE: unchanged_on (concrete_covered proms) mlast m)
           (UNCHANGED: not_attatched updates m),
           exists st' lc' sc' m',
             (<<STEPS : rtc (tau (@Thread.program_step _))
@@ -2193,9 +2260,7 @@ Module Inv.
             (<<WRITING : is_writing _ st' loc Ordering.relaxed>>))
       (UPDATE : forall
           loc to m sc (UPD : updates loc to)
-          (FUTURE: unchanged_on
-                     (fun loc to => covered loc to proms)
-                     mlast m)
+          (FUTURE: unchanged_on (concrete_covered proms) mlast m)
           (UNCHANGED: not_attatched updates m),
           exists st' lc' sc' m',
             (<<STEPS : rtc (tau (@Thread.program_step _))
@@ -2208,81 +2273,145 @@ Module Inv.
 End Inv.
 
 
-Inductive sim_pf
-          (mlast: Ident.t -> Memory.t) (updates: Ident.t -> (Loc.t -> Time.t -> Prop))
-          (c_src c_tgt: Configuration.t) : Prop :=
-| sim_pf_intro
-    (FORGET: forget_config c_src c_tgt)
+Section SIMPF.
 
-    (INV:
-       forall
-         tid lang_src st_src lc_src lang_tgt st_tgt lc_tgt
-         (TIDSRC: IdentMap.find tid c_src.(Configuration.threads) =
-                  Some (existT _ lang_src st_src, lc_src))
-         (TIDTGT: IdentMap.find tid c_tgt.(Configuration.threads) =
-                  Some (existT _ lang_tgt st_tgt, lc_tgt)),
-         Inv.t _ st_src lc_src lc_tgt.(Local.promises) (updates tid) (mlast tid))
+  Inductive thread_wf lang (th: Thread.t lang): Prop :=
+  | thread_wf_intro
+      (SC: Memory.closed_timemap th.(Thread.sc) th.(Thread.memory))
+      (CLOSED: Memory.closed th.(Thread.memory))
+      (LCWF: Local.wf th.(Thread.local) th.(Thread.memory))
+  .
 
-    (FUTURE:
-       forall tid lang_src st_src lc_src
-              (TIDSRC: IdentMap.find tid c_src.(Configuration.threads) =
-                       Some (existT _ lang_src st_src, lc_src)),
-         unchanged_on
-           (fun loc to => covered loc to lc_src.(Local.promises))
-           (mlast tid) c_src.(Configuration.memory))
-    (NOATTATCH:
-       forall tid,
-         not_attatched (updates tid) c_src.(Configuration.memory))
 
-    (RACEFREE: pf_racefree c_src)
-    (WFSRC: Configuration.wf c_src)
-    (WFTGT: Configuration.wf c_tgt)
-    (WFPROMS:
-       forall tid lang st lc
-              (TIDSRC: IdentMap.find tid c_tgt.(Configuration.threads) =
-                       Some (existT _ lang st, lc)),
-         wf_promise lc.(Local.promises))
-.
+  Inductive sim_pf
+            (mlast: Ident.t -> Memory.t) (updates: Ident.t -> (Loc.t -> Time.t -> Prop))
+            (c_src c_tgt: Configuration.t) : Prop :=
+  | sim_pf_intro
+      (FORGET: forget_config c_src c_tgt)
 
-Inductive sim_pf_all c_src c_tgt: Prop :=
-| sim_pf_all_intro mlast updates (SIM : sim_pf mlast updates c_src c_tgt)
-.
+      (INV:
+         forall
+           tid lang_src st_src lc_src lang_tgt st_tgt lc_tgt
+           (TIDSRC: IdentMap.find tid c_src.(Configuration.threads) =
+                    Some (existT _ lang_src st_src, lc_src))
+           (TIDTGT: IdentMap.find tid c_tgt.(Configuration.threads) =
+                    Some (existT _ lang_tgt st_tgt, lc_tgt)),
+           Inv.t _ st_src lc_src lc_tgt.(Local.promises) (updates tid) (mlast tid))
 
-Lemma init_pf s tid st lc
-      (TID: IdentMap.find tid (Threads.init s) = Some (st, lc))
-  :
-    Local.promises lc = Memory.bot.
-Proof.
-  unfold Threads.init in *. erewrite UsualFMapPositive.UsualPositiveMap.Facts.map_o in *.
-  unfold option_map in *. des_ifs.
-Qed.
+      (FUTURE:
+         forall tid lang_src st_src lc_src
+                (TIDSRC: IdentMap.find tid c_src.(Configuration.threads) =
+                         Some (existT _ lang_src st_src, lc_src)),
+           unchanged_on
+             (fun loc to => covered loc to lc_src.(Local.promises))
+             (mlast tid) c_src.(Configuration.memory))
+      (NOATTATCH:
+         forall tid,
+           not_attatched (updates tid) c_src.(Configuration.memory))
 
-Lemma sim_pf_init
-      s
-      (RACEFREE: pf_racefree (Configuration.init s))
-  :
-    sim_pf_all (Configuration.init s) (Configuration.init s)
-.
-Proof.
-  econs. instantiate (1:=fun _ _ _ => False). instantiate (1:=fun _ => Memory.init).
-  econs; eauto; ss; i.
-  - econs; i; ss.
-    + unfold Threads.init in *. erewrite UsualFMapPositive.UsualPositiveMap.Facts.map_o in *.
-      unfold option_map in *. des_ifs.
-    + econs.
-      * instantiate (1:= Memory.init). econs; ss; eauto.
-        ii. inv PROMS. ss.
-        exploit init_pf; eauto. i. rewrite x0 in *.
-        inv PROMISED. rewrite Memory.bot_get in *. clarify.
-      * refl.
-  - econs; s.
-    + i. exploit init_pf; try apply TIDTGT; eauto. i.
-      rewrite x0 in *. inv PROM.
-      rewrite Memory.bot_get in *. clarify.
-    + i. clarify.
-  - econs; eauto. refl.
-  - eapply Configuration.init_wf.
-  - eapply Configuration.init_wf.
-  - unfold Threads.init in *. erewrite UsualFMapPositive.UsualPositiveMap.Facts.map_o in *.
+      (RACEFREE: pf_racefree c_src)
+      (WFSRC: Configuration.wf c_src)
+      (WFTGT: Configuration.wf c_tgt)
+      (WFPROMS:
+         forall tid lang st lc
+                (TIDSRC: IdentMap.find tid c_tgt.(Configuration.threads) =
+                         Some (existT _ lang st, lc)),
+           wf_promise lc.(Local.promises))
+  .
+
+  Inductive sim_pf_all c_src c_tgt: Prop :=
+  | sim_pf_all_intro mlast updates (SIM : sim_pf mlast updates c_src c_tgt)
+  .
+
+  Lemma init_pf s tid st lc
+        (TID: IdentMap.find tid (Threads.init s) = Some (st, lc))
+    :
+      Local.promises lc = Memory.bot.
+  Proof.
+    unfold Threads.init in *. erewrite UsualFMapPositive.UsualPositiveMap.Facts.map_o in *.
     unfold option_map in *. des_ifs.
-Qed.
+  Qed.
+
+  Lemma sim_pf_init
+        s
+        (RACEFREE: pf_racefree (Configuration.init s))
+    :
+      sim_pf_all (Configuration.init s) (Configuration.init s)
+  .
+  Proof.
+    econs. instantiate (1:=fun _ _ _ => False). instantiate (1:=fun _ => Memory.init).
+    econs; eauto; ss; i.
+    - econs; i; ss.
+      + unfold Threads.init in *. erewrite UsualFMapPositive.UsualPositiveMap.Facts.map_o in *.
+        unfold option_map in *. des_ifs.
+      + econs.
+        * instantiate (1:= Memory.init). econs; ss; eauto.
+          ii. inv PROMS. ss.
+          exploit init_pf; eauto. i. rewrite x0 in *.
+          inv PROMISED. rewrite Memory.bot_get in *. clarify.
+        * refl.
+    - econs; s.
+      + i. exploit init_pf; try apply TIDTGT; eauto. i.
+        rewrite x0 in *. inv PROM.
+        rewrite Memory.bot_get in *. clarify.
+      + i. clarify.
+    - econs; eauto. refl.
+    - eapply Configuration.init_wf.
+    - eapply Configuration.init_wf.
+    - unfold Threads.init in *. erewrite UsualFMapPositive.UsualPositiveMap.Facts.map_o in *.
+      unfold option_map in *. des_ifs.
+  Qed.
+
+End SIMPF.
+
+
+Section UNUSEDYET.
+
+  Definition no_acq_read_msgs (MSGS : Loc.t -> Time.t -> Prop)
+             (e : ThreadEvent.t) : Prop :=
+    match e with
+    | ThreadEvent.read loc to _ _ ord =>
+      forall (SAT: MSGS loc to), ~ Ordering.le Ordering.acqrel ord
+    | ThreadEvent.update loc from _ _ _ _ _ ordr _ =>
+      forall (SAT: MSGS loc from), ~ Ordering.le Ordering.acqrel ordr
+    | _ => True
+    end
+  .
+
+  Inductive capped_with_max_view mem (CAP: Loc.t -> Time.t -> Prop)
+            (prom: Loc.t -> Time.t -> Prop): Prop :=
+  | capped_with_max_view_intro
+      (GET: forall loc to from val view
+                   (SAT: CAP loc to)
+                   (GET: Memory.get loc to mem = Some (from, Message.full val view)),
+          match view with
+          | None => False
+          | Some view' => ~ promise_view_consistent prom view'.(View.rlx)
+          end)
+  .
+
+  Definition cap (m mcap: Memory.t) (l: Loc.t) (t: Time.t): Prop :=
+    (<<NCOV: ~ covered l t m>>) /\ (<<CAP: ~ covered l t mcap>>).
+
+  Definition cap_write_with_update (CAP : Loc.t -> Time.t -> Prop)
+             (e : ThreadEvent.t) : Prop :=
+    match e with
+    | ThreadEvent.write loc from to _ _ _ =>
+      forall t (IN: Interval.mem (from, to) t), (~ CAP loc t)
+    | _ => True
+    end.
+
+  Inductive capped (mem_src mem_tgt: Memory.t): Prop :=
+  | capped_intro
+      (COVERLE: forall l t (COVER: covered l t mem_src), covered l t mem_tgt)
+      (MLE: forall loc to from val released
+                   (GET: Memory.get loc to mem_tgt = Some (from, Message.full val released)),
+          exists to_src from_src released_src,
+            (<<GET: Memory.get loc to_src mem_src =
+                    Some (from_src, Message.full val released_src)>>) /\
+            (<<EMPTY: forall l t (IN: Interval.mem (to_src, to) t), ~ covered l t mem_src>>) /\
+            (<<TOLE: Time.le to_src to>>) /\
+            (<<VIEWLE: View.opt_le released_src released>>))
+  .
+
+End UNUSEDYET.
